
{
    "@context": {
        "unece": "https://service.unece.org/trade/uncefact/vocabulary/unece#",
        "rdf": "http://www.w3.org/1999/02/22-rdf-syntax-ns#",
        "rdfs": "http://www.w3.org/2000/01/rdf-schema#",
        "schema": "http://schema.org/",
        "tourism": "https://service.unece.org/trade/uncefact/vocabulary/unece/tourism#",
        "cefact": "https://service.unece.org/trade/uncefact/vocabulary/cefact#",
        "xsd": "http://www.w3.org/2001/XMLSchema#"
    },
    "@graph": [
        {
            "@id": "tourism:BasicPrice",
            "@type": "rdfs:Class",
            "rdfs:comment": "A sum of money for which something is or may be bought or sold without any discount or surcharge being applied.",
            "rdfs:label": "BasicPrice",
            "unece:cefactElementMetadata": [
                {
                    "@id": "cefact:Basic_Price.Details",
                    "@type": "unece:AggregateBIE",
                    "unece:cefactUNId": "UN01004999",
                    "rdfs:comment": "A sum of money for which something is or may be bought or sold without any discount or surcharge being applied."
                }
            ]
        },
        {
            "@id": "tourism:BathingFacility",
            "@type": "rdfs:Class",
            "rdfs:comment": "A space or structure for immersing the body in water, such as a swimming pool.",
            "rdfs:label": "BathingFacility",
            "unece:cefactElementMetadata": [
                {
                    "@id": "cefact:Bathing_Facility.Details",
                    "@type": "unece:AggregateBIE",
                    "unece:cefactUNId": "UN01001061",
                    "rdfs:comment": "A space or structure for immersing the body in water, such as a swimming pool."
                }
            ]
        },
        {
            "@id": "tourism:BusinessSupportRoomFacility",
            "@type": "rdfs:Class",
            "rdfs:comment": "A room to support business activities, which may include office equipment and secretarial services.",
            "rdfs:label": "BusinessSupportRoomFacility",
            "unece:cefactElementMetadata": [
                {
                    "@id": "cefact:BusinessSupportRoom_Facility.Details",
                    "@type": "unece:AggregateBIE",
                    "unece:cefactUNId": "UN01001105",
                    "rdfs:comment": "A room to support business activities, which may include office equipment and secretarial services."
                }
            ]
        },
        {
            "@id": "tourism:CancellationPrice",
            "@type": "rdfs:Class",
            "rdfs:comment": "A sum of money for cancelling something which is or may be bought or sold.",
            "rdfs:label": "CancellationPrice",
            "unece:cefactElementMetadata": [
                {
                    "@id": "cefact:Cancellation_Price.Details",
                    "@type": "unece:AggregateBIE",
                    "unece:cefactUNId": "UN01005074",
                    "rdfs:comment": "A sum of money for cancelling something which is or may be bought or sold."
                }
            ]
        },
        {
            "@id": "tourism:CustomerClass",
            "@type": "rdfs:Class",
            "rdfs:comment": "The conditions and requirements of the type of person who may use or purchase a product.",
            "rdfs:label": "CustomerClass",
            "unece:cefactElementMetadata": [
                {
                    "@id": "cefact:CustomerClass.Details",
                    "@type": "unece:AggregateBIE",
                    "unece:cefactUNId": "UN01004945",
                    "rdfs:comment": "The conditions and requirements of the type of person who may use or purchase a product."
                }
            ]
        },
        {
            "@id": "tourism:DailyPrice",
            "@type": "rdfs:Class",
            "rdfs:comment": "A daily sum of money for which this lodging house travel product may be or is sold.",
            "rdfs:label": "DailyPrice",
            "unece:cefactElementMetadata": [
                {
                    "@id": "cefact:Daily_Price.Details",
                    "@type": "unece:AggregateBIE",
                    "unece:cefactUNId": "UN01009685",
                    "rdfs:comment": "A daily sum of money for which this lodging house travel product may be or is sold."
                }
            ]
        },
        {
            "@id": "tourism:DiscountPrice",
            "@type": "rdfs:Class",
            "rdfs:comment": "A sum of money which is discount against a price for which something may be bought or sold.",
            "rdfs:label": "DiscountPrice",
            "unece:cefactElementMetadata": [
                {
                    "@id": "cefact:Discount_Price.Details",
                    "@type": "unece:AggregateBIE",
                    "unece:cefactUNId": "UN01005034",
                    "rdfs:comment": "A sum of money which is discount against a price for which something may be bought or sold."
                }
            ]
        },
        {
            "@id": "tourism:ExperienceEvent",
            "@type": "rdfs:Class",
            "rdfs:comment": "An involvement in an experience program in which some thing happens, such as a nature watching, woodware manufacturing, meditation, holiday trip, dinner, theme park visit, could be experienced.",
            "rdfs:label": "ExperienceEvent",
            "unece:cefactElementMetadata": [
                {
                    "@id": "cefact:Experience_Event.Details",
                    "@type": "unece:AggregateBIE",
                    "unece:cefactUNId": "UN01015115",
                    "rdfs:comment": "An involvement in an experience program in which some thing happens, such as a nature watching, woodware manufacturing, meditation, holiday trip, dinner, theme park visit, could be experienced."
                }
            ]
        },
        {
            "@id": "tourism:ExperienceFacility",
            "@type": "rdfs:Class",
            "rdfs:comment": "A structure or place, such as a restaurant, hotel, theme park, hot spring bathing pool, parking lot, or meeting room, that provides a particular experience.",
            "rdfs:label": "ExperienceFacility",
            "unece:cefactElementMetadata": [
                {
                    "@id": "cefact:Experience_Facility.Details",
                    "@type": "unece:AggregateBIE",
                    "unece:cefactUNId": "UN01015137",
                    "rdfs:comment": "A structure or place, such as a restaurant, hotel, theme park, hot spring bathing pool, parking lot, or meeting room, that provides a particular experience."
                }
            ]
        },
        {
            "@id": "tourism:ExperienceItemPreference",
            "@type": "rdfs:Class",
            "rdfs:comment": "An involvement in a happening, such as a theme park, a guided tour that is liked or wanted more than another item.",
            "rdfs:label": "ExperienceItemPreference",
            "unece:cefactElementMetadata": [
                {
                    "@id": "cefact:ExperienceItem_Preference.Details",
                    "@type": "unece:AggregateBIE",
                    "unece:cefactUNId": "UN01015150",
                    "rdfs:comment": "An involvement in a happening, such as a theme park, a guided tour that is liked or wanted more than another item."
                }
            ]
        },
        {
            "@id": "tourism:ExperienceItemVoucher",
            "@type": "rdfs:Class",
            "rdfs:comment": "A printed piece of paper or an electronic document that can be used instead of money to pay for an experience, such as a tour, a trip or a meal in a restaurant.",
            "rdfs:label": "ExperienceItemVoucher",
            "unece:cefactElementMetadata": [
                {
                    "@id": "cefact:ExperienceItem_Voucher.Details",
                    "@type": "unece:AggregateBIE",
                    "unece:cefactUNId": "UN01015241",
                    "rdfs:comment": "A printed piece of paper or an electronic document that can be used instead of money to pay for an experience, such as a tour, a trip or a meal in a restaurant."
                }
            ]
        },
        {
            "@id": "tourism:ExperienceProduct",
            "@type": "rdfs:Class",
            "rdfs:comment": "Any service that provides an involvement, such as an adventure experience, wellness experience, social or business activity experience.",
            "rdfs:label": "ExperienceProduct",
            "unece:cefactElementMetadata": [
                {
                    "@id": "cefact:Experience_Product.Details",
                    "@type": "unece:AggregateBIE",
                    "unece:cefactUNId": "UN01015155",
                    "rdfs:comment": "Any service that provides an involvement, such as an adventure experience, wellness experience, social or business activity experience."
                }
            ]
        },
        {
            "@id": "tourism:ExperienceProgramAction",
            "@type": "rdfs:Class",
            "rdfs:comment": "Any type of action, such as searching, reserving, or paying, necessary for an experience program, such as an adventure experience, a business experience, or a wellness experience.",
            "rdfs:label": "ExperienceProgramAction",
            "unece:cefactElementMetadata": [
                {
                    "@id": "cefact:ExperienceProgram_Action.Details",
                    "@type": "unece:AggregateBIE",
                    "unece:cefactUNId": "UN01015183",
                    "rdfs:comment": "Any type of action, such as searching, reserving, or paying, necessary for an experience program, such as an adventure experience, a business experience, or a wellness experience."
                }
            ]
        },
        {
            "@id": "tourism:ExtraPrice",
            "@type": "rdfs:Class",
            "rdfs:comment": "A sum of money which is an addition to the price for which something is or may be bought or sold, such as for a special meal.",
            "rdfs:label": "ExtraPrice",
            "unece:cefactElementMetadata": [
                {
                    "@id": "cefact:Extra_Price.Details",
                    "@type": "unece:AggregateBIE",
                    "unece:cefactUNId": "UN01005015",
                    "rdfs:comment": "A sum of money which is an addition to the price for which something is or may be bought or sold, such as for a special meal."
                }
            ]
        },
        {
            "@id": "tourism:GuestAllergy",
            "@type": "rdfs:Class",
            "rdfs:comment": "A guest condition of the abnormal reaction of the body to a previously encountered substance introduced by inhalation, ingestion, injection, or skin contact.",
            "rdfs:label": "GuestAllergy",
            "unece:cefactElementMetadata": [
                {
                    "@id": "cefact:Guest_Allergy.Details",
                    "@type": "unece:AggregateBIE",
                    "unece:cefactUNId": "UN01015189",
                    "rdfs:comment": "A guest condition of the abnormal reaction of the body to a previously encountered substance introduced by inhalation, ingestion, injection, or skin contact."
                }
            ]
        },
        {
            "@id": "tourism:GuestCarriedEquipment",
            "@type": "rdfs:Class",
            "rdfs:comment": "A tool or device carried by a guest for an activity.",
            "rdfs:label": "GuestCarriedEquipment",
            "unece:cefactElementMetadata": [
                {
                    "@id": "cefact:Guest_CarriedEquipment.Details",
                    "@type": "unece:AggregateBIE",
                    "unece:cefactUNId": "UN01015194",
                    "rdfs:comment": "A tool or device carried by a guest for an activity."
                }
            ]
        },
        {
            "@id": "tourism:GuestDisability",
            "@type": "rdfs:Class",
            "rdfs:comment": "A physical or mental condition that limits a guest's movements, senses, or activities.",
            "rdfs:label": "GuestDisability",
            "unece:cefactElementMetadata": [
                {
                    "@id": "cefact:Guest_Disability.Details",
                    "@type": "unece:AggregateBIE",
                    "unece:cefactUNId": "UN01015200",
                    "rdfs:comment": "A physical or mental condition that limits a guest's movements, senses, or activities."
                }
            ]
        },
        {
            "@id": "tourism:GuestFoodChoice",
            "@type": "rdfs:Class",
            "rdfs:comment": "A guest's decision which food to buy or eat.",
            "rdfs:label": "GuestFoodChoice",
            "unece:cefactElementMetadata": [
                {
                    "@id": "cefact:Guest_FoodChoice.Details",
                    "@type": "unece:AggregateBIE",
                    "unece:cefactUNId": "UN01015207",
                    "rdfs:comment": "A guest's decision which food to buy or eat."
                }
            ]
        },
        {
            "@id": "tourism:GuestHealthIndication",
            "@type": "rdfs:Class",
            "rdfs:comment": "A guest's physical or mental condition.",
            "rdfs:label": "GuestHealthIndication",
            "unece:cefactElementMetadata": [
                {
                    "@id": "cefact:Guest_HealthIndication.Details",
                    "@type": "unece:AggregateBIE",
                    "unece:cefactUNId": "UN01015212",
                    "rdfs:comment": "A guest's physical or mental condition."
                }
            ]
        },
        {
            "@id": "tourism:GuestPerson",
            "@type": "rdfs:Class",
            "rdfs:comment": "An individual guest.",
            "rdfs:label": "GuestPerson",
            "unece:cefactElementMetadata": [
                {
                    "@id": "cefact:Guest_Person.Details",
                    "@type": "unece:AggregateBIE",
                    "unece:cefactUNId": "UN01009708",
                    "rdfs:comment": "An individual guest."
                }
            ]
        },
        {
            "@id": "tourism:GuestRoomFacility",
            "@type": "rdfs:Class",
            "rdfs:comment": "A place that provides lodging for a guest.",
            "rdfs:label": "GuestRoomFacility",
            "unece:cefactElementMetadata": [
                {
                    "@id": "cefact:GuestRoom_Facility.Details",
                    "@type": "unece:AggregateBIE",
                    "unece:cefactUNId": "UN01001047",
                    "rdfs:comment": "A place that provides lodging for a guest."
                }
            ]
        },
        {
            "@id": "tourism:LodgingHouseBuilding",
            "@type": "rdfs:Class",
            "rdfs:comment": "A permanent fixed structure of the lodging house.",
            "rdfs:label": "LodgingHouseBuilding",
            "unece:cefactElementMetadata": [
                {
                    "@id": "cefact:LodgingHouse_Building.Details",
                    "@type": "unece:AggregateBIE",
                    "unece:cefactUNId": "UN01001037",
                    "rdfs:comment": "A permanent fixed structure of the lodging house."
                }
            ]
        },
        {
            "@id": "tourism:LodgingHouseContact",
            "@type": "rdfs:Class",
            "rdfs:comment": "A person or department that acts as a point of contact with another person or department for this lodging house.",
            "rdfs:label": "LodgingHouseContact",
            "unece:cefactElementMetadata": [
                {
                    "@id": "cefact:LodgingHouse_Contact.Details",
                    "@type": "unece:AggregateBIE",
                    "unece:cefactUNId": "UN01001221",
                    "rdfs:comment": "A person or department that acts as a point of contact with another person or department for this lodging house."
                }
            ]
        },
        {
            "@id": "tourism:LodgingHouseContract",
            "@type": "rdfs:Class",
            "rdfs:comment": "An agreement, written or spoken and enforceable by law, between a lodging house and another party.",
            "rdfs:label": "LodgingHouseContract",
            "unece:cefactElementMetadata": [
                {
                    "@id": "cefact:LodgingHouse_Contract.Details",
                    "@type": "unece:AggregateBIE",
                    "unece:cefactUNId": "UN01001210",
                    "rdfs:comment": "An agreement, written or spoken and enforceable by law, between a lodging house and another party."
                }
            ]
        },
        {
            "@id": "tourism:LodgingHouseCustomerClass",
            "@type": "rdfs:Class",
            "rdfs:comment": "The conditions and requirements of the type of person who may use or purchase a lodging house product.",
            "rdfs:label": "LodgingHouseCustomerClass",
            "unece:cefactElementMetadata": [
                {
                    "@id": "cefact:LodgingHouse_CustomerClass.Details",
                    "@type": "unece:AggregateBIE",
                    "unece:cefactUNId": "UN01010029",
                    "rdfs:comment": "The conditions and requirements of the type of person who may use or purchase a lodging house product."
                }
            ]
        },
        {
            "@id": "tourism:LodgingHouseFeature",
            "@type": "rdfs:Class",
            "rdfs:comment": "Distinctive or characteristic parts of a lodging house.",
            "rdfs:label": "LodgingHouseFeature",
            "unece:cefactElementMetadata": [
                {
                    "@id": "cefact:LodgingHouse_Feature.Details",
                    "@type": "unece:AggregateBIE",
                    "unece:cefactUNId": "UN01001183",
                    "rdfs:comment": "Distinctive or characteristic parts of a lodging house."
                }
            ]
        },
        {
            "@id": "tourism:LodgingHouseLocation",
            "@type": "rdfs:Class",
            "rdfs:comment": "The physical location or place of this lodging house.",
            "rdfs:label": "LodgingHouseLocation",
            "unece:cefactElementMetadata": [
                {
                    "@id": "cefact:LodgingHouse_Location.Details",
                    "@type": "unece:AggregateBIE",
                    "unece:cefactUNId": "UN01001217",
                    "rdfs:comment": "The physical location or place of this lodging house."
                }
            ]
        },
        {
            "@id": "tourism:LodgingHouseOrganization",
            "@type": "rdfs:Class",
            "rdfs:comment": "An organization set up for the purpose of providing temporary accommodation.",
            "rdfs:label": "LodgingHouseOrganization",
            "unece:cefactElementMetadata": [
                {
                    "@id": "cefact:LodgingHouse_Organization.Details",
                    "@type": "unece:AggregateBIE",
                    "unece:cefactUNId": "UN01001027",
                    "rdfs:comment": "An organization set up for the purpose of providing temporary accommodation."
                }
            ]
        },
        {
            "@id": "tourism:LodgingHouseParty",
            "@type": "rdfs:Class",
            "rdfs:comment": "An individual, a group, or a body having a role in the lodging house business.",
            "rdfs:label": "LodgingHouseParty",
            "unece:cefactElementMetadata": [
                {
                    "@id": "cefact:LodgingHouse_Party.Details",
                    "@type": "unece:AggregateBIE",
                    "unece:cefactUNId": "UN01001280",
                    "rdfs:comment": "An individual, a group, or a body having a role in the lodging house business."
                }
            ]
        },
        {
            "@id": "tourism:LodgingHousePicture",
            "@type": "rdfs:Class",
            "rdfs:comment": "A digital image of a painting, drawing, or photograph for this lodging house.",
            "rdfs:label": "LodgingHousePicture",
            "unece:cefactElementMetadata": [
                {
                    "@id": "cefact:LodgingHouse_Picture.Details",
                    "@type": "unece:AggregateBIE",
                    "unece:cefactUNId": "UN01001241",
                    "rdfs:comment": "A digital image of a painting, drawing, or photograph for this lodging house."
                }
            ]
        },
        {
            "@id": "tourism:LodgingHouseReservation",
            "@type": "rdfs:Class",
            "rdfs:comment": "The action or fact of booking a travel product of this lodging house in advance.",
            "rdfs:label": "LodgingHouseReservation",
            "unece:cefactElementMetadata": [
                {
                    "@id": "cefact:LodgingHouse_Reservation.Details",
                    "@type": "unece:AggregateBIE",
                    "unece:cefactUNId": "UN01009789",
                    "rdfs:comment": "The action or fact of booking a travel product of this lodging house in advance."
                }
            ]
        },
        {
            "@id": "tourism:LodgingHouseReservationRestriction",
            "@type": "rdfs:Class",
            "rdfs:comment": "A limitation for the booking of a lodging house product or service.",
            "rdfs:label": "LodgingHouseReservationRestriction",
            "unece:cefactElementMetadata": [
                {
                    "@id": "cefact:LodgingHouse_ReservationRestriction.Details",
                    "@type": "unece:AggregateBIE",
                    "unece:cefactUNId": "UN01010046",
                    "rdfs:comment": "A limitation for the booking of a lodging house product or service."
                }
            ]
        },
        {
            "@id": "tourism:LodgingHouseRoute",
            "@type": "rdfs:Class",
            "rdfs:comment": "Way of approach to a lodging house.",
            "rdfs:label": "LodgingHouseRoute",
            "unece:cefactElementMetadata": [
                {
                    "@id": "cefact:LodgingHouse_Route.Details",
                    "@type": "unece:AggregateBIE",
                    "unece:cefactUNId": "UN01001235",
                    "rdfs:comment": "Way of approach to a lodging house."
                }
            ]
        },
        {
            "@id": "tourism:LodgingHouseTravelProduct",
            "@type": "rdfs:Class",
            "rdfs:comment": "A lodging house travel item which may be purchased by a customer.",
            "rdfs:label": "LodgingHouseTravelProduct",
            "unece:cefactElementMetadata": [
                {
                    "@id": "cefact:LodgingHouse_TravelProduct.Details",
                    "@type": "unece:AggregateBIE",
                    "unece:cefactUNId": "UN01004916",
                    "rdfs:comment": "A lodging house travel item which may be purchased by a customer."
                }
            ]
        },
        {
            "@id": "tourism:LodgingHouseTravelProductComponent",
            "@type": "rdfs:Class",
            "rdfs:comment": "An item that is included in a lodging house travel product for which there is no additional charge.",
            "rdfs:label": "LodgingHouseTravelProductComponent",
            "unece:cefactElementMetadata": [
                {
                    "@id": "cefact:LodgingHouse_TravelProductComponent.Details",
                    "@type": "unece:AggregateBIE",
                    "unece:cefactUNId": "UN01004971",
                    "rdfs:comment": "An item that is included in a lodging house travel product for which there is no additional charge."
                }
            ]
        },
        {
            "@id": "tourism:LodgingHouseTravelProductSubComponent",
            "@type": "rdfs:Class",
            "rdfs:comment": "An item which is included in a lodging house travel product component.",
            "rdfs:label": "LodgingHouseTravelProductSubComponent",
            "unece:cefactElementMetadata": [
                {
                    "@id": "cefact:LodgingHouse_TravelProductSub-Component.Details",
                    "@type": "unece:AggregateBIE",
                    "unece:cefactUNId": "UN01004985",
                    "rdfs:comment": "An item which is included in a lodging house travel product component."
                }
            ]
        },
        {
            "@id": "tourism:LodgingHouseTraveller",
            "@type": "rdfs:Class",
            "rdfs:comment": "A person or group which is travelling or on a journey and staying at this lodging house.",
            "rdfs:label": "LodgingHouseTraveller",
            "unece:cefactElementMetadata": [
                {
                    "@id": "cefact:LodgingHouse_Traveller.Details",
                    "@type": "unece:AggregateBIE",
                    "unece:cefactUNId": "UN01009810",
                    "rdfs:comment": "A person or group which is travelling or on a journey and staying at this lodging house."
                }
            ]
        },
        {
            "@id": "tourism:LodgingHouseUsageCondition",
            "@type": "rdfs:Class",
            "rdfs:comment": "A usage condition for this lodging house.",
            "rdfs:label": "LodgingHouseUsageCondition",
            "unece:cefactElementMetadata": [
                {
                    "@id": "cefact:LodgingHouse_UsageCondition.Details",
                    "@type": "unece:AggregateBIE",
                    "unece:cefactUNId": "UN01001199",
                    "rdfs:comment": "A usage condition for this lodging house."
                }
            ]
        },
        {
            "@id": "tourism:ProductComponentItinerary",
            "@type": "rdfs:Class",
            "rdfs:comment": "Schedule and location information for travel for a product component.",
            "rdfs:label": "ProductComponentItinerary",
            "unece:cefactElementMetadata": [
                {
                    "@id": "cefact:ProductComponent_Itinerary.Details",
                    "@type": "unece:AggregateBIE",
                    "unece:cefactUNId": "UN01004979",
                    "rdfs:comment": "Schedule and location information for travel for a product component."
                }
            ]
        },
        {
            "@id": "tourism:ReservationRestriction",
            "@type": "rdfs:Class",
            "rdfs:comment": "A limitation for the booking of a product or service.",
            "rdfs:label": "ReservationRestriction",
            "unece:cefactElementMetadata": [
                {
                    "@id": "cefact:ReservationRestriction.Details",
                    "@type": "unece:AggregateBIE",
                    "unece:cefactUNId": "UN01004954",
                    "rdfs:comment": "A limitation for the booking of a product or service."
                }
            ]
        },
        {
            "@id": "tourism:TravelProductReservationItem",
            "@type": "rdfs:Class",
            "rdfs:comment": "An item of the travel products or services which is specified in the reservation.",
            "rdfs:label": "TravelProductReservationItem",
            "unece:cefactElementMetadata": [
                {
                    "@id": "cefact:TravelProduct_ReservationItem.Details",
                    "@type": "unece:AggregateBIE",
                    "unece:cefactUNId": "UN01009972",
                    "rdfs:comment": "An item of the travel products or services which is specified in the reservation."
                }
            ]
        },
        {
            "@id": "tourism:acceptedDateTime",
            "@type": "rdf:Property",
            "schema:rangeIncludes": {
                "@id": "xsd:dateTime"
            },
            "schema:domainIncludes": {
                "@id": "tourism:LodgingHouseReservation"
            },
            "rdfs:comment": "The date, time, date time or other date time value that this reservation is accepted for the lodging house.",
            "rdfs:label": "acceptedDateTime",
            "unece:cefactElementMetadata": [
                {
                    "@id": "cefact:LodgingHouse_Reservation.Accepted.DateTime",
                    "@type": "unece:BasicBIE",
                    "unece:cefactUNId": "UN01009792",
                    "unece:cefactBieDomainClass": "cefact:LodgingHouse_Reservation.Details",
                    "rdfs:comment": "The date, time, date time or other date time value that this reservation is accepted for the lodging house."
                }
            ]
        },
        {
            "@id": "tourism:accessRightsCode",
            "@type": "rdf:Property",
            "schema:rangeIncludes": {
                "@id": "xsd:token"
            },
            "schema:domainIncludes": {
                "@id": "tourism:LodgingHouseParty"
            },
            "rdfs:comment": "The code specifying this lodging house party's access rights.",
            "rdfs:label": "accessRightsCode",
            "unece:cefactElementMetadata": [
                {
                    "@id": "cefact:LodgingHouse_Party.AccessRights.Code",
                    "@type": "unece:BasicBIE",
                    "unece:cefactUNId": "UN01001285",
                    "unece:cefactBieDomainClass": "cefact:LodgingHouse_Party.Details",
                    "rdfs:comment": "The code specifying this lodging house party's access rights."
                }
            ]
        },
        {
            "@id": "tourism:accompanyingAnimal",
            "@type": "rdf:Property",
            "schema:rangeIncludes": {
                "@id": "tourism:Animal"
            },
            "schema:domainIncludes": {
                "@id": "tourism:GuestPerson"
            },
            "rdfs:comment": "A pet animal accompanying this guest person.",
            "rdfs:label": "accompanyingAnimal",
            "unece:cefactElementMetadata": [
                {
                    "@id": "cefact:Guest_Person.Accompanying.Pet_Animal",
                    "@type": "unece:AssociationBIE",
                    "unece:cefactUNId": "UN01015224",
                    "unece:cefactBieDomainClass": "cefact:Guest_Person.Details",
                    "rdfs:comment": "A pet animal accompanying this guest person."
                }
            ]
        },
        {
            "@id": "tourism:actualPicture",
            "@type": "rdf:Property",
            "schema:rangeIncludes": {
                "@id": "tourism:Picture"
            },
            "schema:domainIncludes": [
                {
                    "@id": "tourism:BathingFacility"
                },
                {
                    "@id": "tourism:BusinessSupportRoomFacility"
                },
                {
                    "@id": "tourism:GuestRoomFacility"
                },
                {
                    "@id": "tourism:LodgingHouseBuilding"
                },
                {
                    "@id": "tourism:LodgingHouseTravelProductSubComponent"
                }
            ],
            "rdfs:comment": [
                "An actual picture of this bathing facility at this lodging house.",
                "An actual picture of this business support room at this lodging house.",
                "An actual picture of this guest room at this lodging house.",
                "An actual picture of this lodging house building.",
                "An actual picture of this lodging house travel product sub-component."
            ],
            "rdfs:label": "actualPicture",
            "unece:cefactElementMetadata": [
                {
                    "@id": "cefact:LodgingHouse_TravelProductSub-Component.Actual.LodgingHouse_Picture",
                    "@type": "unece:AssociationBIE",
                    "unece:cefactUNId": "UN01010194",
                    "unece:cefactBieDomainClass": "cefact:LodgingHouse_TravelProductSubComponent.Details",
                    "rdfs:comment": "An actual picture of this lodging house travel product sub-component."
                },
                {
                    "@id": "cefact:Bathing_Facility.Actual.LodgingHouse_Picture",
                    "@type": "unece:AssociationBIE",
                    "unece:cefactUNId": "UN01001073",
                    "unece:cefactBieDomainClass": "cefact:Bathing_Facility.Details",
                    "rdfs:comment": "An actual picture of this bathing facility at this lodging house."
                },
                {
                    "@id": "cefact:BusinessSupportRoom_Facility.Actual.LodgingHouse_Picture",
                    "@type": "unece:AssociationBIE",
                    "unece:cefactUNId": "UN01001115",
                    "unece:cefactBieDomainClass": "cefact:BusinessSupportRoom_Facility.Details",
                    "rdfs:comment": "An actual picture of this business support room at this lodging house."
                },
                {
                    "@id": "cefact:LodgingHouse_TravelProductSub-Component.Actual.Picture",
                    "@type": "unece:AssociationBIE",
                    "unece:cefactUNId": "UN01004996",
                    "unece:cefactBieDomainClass": "cefact:LodgingHouse_TravelProductSubComponent.Details",
                    "rdfs:comment": "An actual picture of this lodging house travel product sub-component."
                },
                {
                    "@id": "cefact:LodgingHouse_Building.Actual.LodgingHouse_Picture",
                    "@type": "unece:AssociationBIE",
                    "unece:cefactUNId": "UN01001045",
                    "unece:cefactBieDomainClass": "cefact:LodgingHouse_Building.Details",
                    "rdfs:comment": "An actual picture of this lodging house building."
                },
                {
                    "@id": "cefact:GuestRoom_Facility.Actual.LodgingHouse_Picture",
                    "@type": "unece:AssociationBIE",
                    "unece:cefactUNId": "UN01001058",
                    "unece:cefactBieDomainClass": "cefact:GuestRoom_Facility.Details",
                    "rdfs:comment": "An actual picture of this guest room at this lodging house."
                }
            ]
        },
        {
            "@id": "tourism:additionalInformationNote",
            "@type": "rdf:Property",
            "schema:rangeIncludes": {
                "@id": "tourism:Note"
            },
            "schema:domainIncludes": [
                {
                    "@id": "tourism:BasicPrice"
                },
                {
                    "@id": "tourism:CancellationPrice"
                },
                {
                    "@id": "tourism:DiscountPrice"
                },
                {
                    "@id": "tourism:ExtraPrice"
                }
            ],
            "rdfs:comment": [
                "Additional information about the travel cancellation price.",
                "Additional travel product information for a basic price.",
                "Additional travel product information for a discount price.",
                "Additional travel product information for an extra price."
            ],
            "rdfs:label": "additionalInformationNote",
            "unece:cefactElementMetadata": [
                {
                    "@id": "cefact:Discount_Price.AdditionalInformation.TravelProduct_Note",
                    "@type": "unece:AssociationBIE",
                    "unece:cefactUNId": "UN01005051",
                    "unece:cefactBieDomainClass": "cefact:Discount_Price.Details",
                    "rdfs:comment": "Additional travel product information for a discount price."
                },
                {
                    "@id": "cefact:Basic_Price.AdditionalInformation.TravelProduct_Note",
                    "@type": "unece:AssociationBIE",
                    "unece:cefactUNId": "UN01005013",
                    "unece:cefactBieDomainClass": "cefact:Basic_Price.Details",
                    "rdfs:comment": "Additional travel product information for a basic price."
                },
                {
                    "@id": "cefact:Extra_Price.AdditionalInformation.TravelProduct_Note",
                    "@type": "unece:AssociationBIE",
                    "unece:cefactUNId": "UN01005032",
                    "unece:cefactBieDomainClass": "cefact:Extra_Price.Details",
                    "rdfs:comment": "Additional travel product information for an extra price."
                },
                {
                    "@id": "cefact:Cancellation_Price.AdditionalInformation.TravelProduct_Note",
                    "@type": "unece:AssociationBIE",
                    "unece:cefactUNId": "UN01005083",
                    "unece:cefactBieDomainClass": "cefact:Cancellation_Price.Details",
                    "rdfs:comment": "Additional information about the travel cancellation price."
                }
            ]
        },
        {
            "@id": "tourism:additionalNote",
            "@type": "rdf:Property",
            "schema:rangeIncludes": {
                "@id": "tourism:Note"
            },
            "schema:domainIncludes": {
                "@id": "tourism:GuestPerson"
            },
            "rdfs:comment": "An additional personal note for this guest.",
            "rdfs:label": "additionalNote",
            "unece:cefactElementMetadata": [
                {
                    "@id": "cefact:Guest_Person.Additional.Person_Note",
                    "@type": "unece:AssociationBIE",
                    "unece:cefactUNId": "UN01009721",
                    "unece:cefactBieDomainClass": "cefact:Guest_Person.Details",
                    "rdfs:comment": "An additional personal note for this guest."
                }
            ]
        },
        {
            "@id": "tourism:ageLimitation",
            "@type": "rdf:Property",
            "schema:rangeIncludes": {
                "@id": "xsd:string"
            },
            "schema:domainIncludes": {
                "@id": "tourism:LodgingHouseUsageCondition"
            },
            "rdfs:comment": "The age limitation, expressed as text, applicable to this lodging house usage condition.",
            "rdfs:label": "ageLimitation",
            "unece:cefactElementMetadata": [
                {
                    "@id": "cefact:LodgingHouse_UsageCondition.AgeLimitation.Text",
                    "@type": "unece:BasicBIE",
                    "unece:cefactUNId": "UN01001206",
                    "unece:cefactBieDomainClass": "cefact:LodgingHouse_UsageCondition.Details",
                    "rdfs:comment": "The age limitation, expressed as text, applicable to this lodging house usage condition."
                }
            ]
        },
        {
            "@id": "tourism:ageMeasure",
            "@type": "rdf:Property",
            "schema:rangeIncludes": {
                "@id": "xsd:decimal"
            },
            "schema:domainIncludes": {
                "@id": "tourism:GuestPerson"
            },
            "rdfs:comment": "The measure of the age of this guest person.",
            "rdfs:label": "ageMeasure",
            "unece:cefactElementMetadata": [
                {
                    "@id": "cefact:Guest_Person.Age.Measure",
                    "@type": "unece:BasicBIE",
                    "unece:TDED": "2018",
                    "unece:cefactUNId": "UN01015219",
                    "unece:cefactBieDomainClass": "cefact:Guest_Person.Details",
                    "rdfs:comment": "The measure of the age of this guest person."
                }
            ]
        },
        {
            "@id": "tourism:allianceName",
            "@type": "rdf:Property",
            "schema:rangeIncludes": {
                "@id": "xsd:string"
            },
            "schema:domainIncludes": {
                "@id": "tourism:LodgingHouseOrganization"
            },
            "rdfs:comment": "A name of an alliance, expressed as text, in which this lodging house organization participates, such as JTB Accredited Hotels and Ryokans Group, Accredited Hotel Group, STAR ALLIANCE Member Hotel Group.",
            "rdfs:label": "allianceName",
            "unece:cefactElementMetadata": [
                {
                    "@id": "cefact:LodgingHouse_Organization.Alliance_Name.Text",
                    "@type": "unece:BasicBIE",
                    "unece:cefactUNId": "UN01001034",
                    "unece:cefactBieDomainClass": "cefact:LodgingHouse_Organization.Details",
                    "rdfs:comment": "A name of an alliance, expressed as text, in which this lodging house organization participates, such as JTB Accredited Hotels and Ryokans Group, Accredited Hotel Group, STAR ALLIANCE Member Hotel Group."
                }
            ]
        },
        {
            "@id": "tourism:applicableAvailability",
            "@type": "rdf:Property",
            "schema:rangeIncludes": {
                "@id": "tourism:Availability"
            },
            "schema:domainIncludes": {
                "@id": "tourism:LodgingHouseTravelProduct"
            },
            "rdfs:comment": "Product availability applicable to this lodging house travel product.",
            "rdfs:label": "applicableAvailability",
            "unece:cefactElementMetadata": [
                {
                    "@id": "cefact:LodgingHouse_TravelProduct.Applicable.Product_Availability",
                    "@type": "unece:AssociationBIE",
                    "unece:cefactUNId": "UN01004938",
                    "unece:cefactBieDomainClass": "cefact:LodgingHouse_TravelProduct.Details",
                    "rdfs:comment": "Product availability applicable to this lodging house travel product."
                }
            ]
        },
        {
            "@id": "tourism:applicableCustomerClass",
            "@type": "rdf:Property",
            "schema:rangeIncludes": {
                "@id": "tourism:CustomerClass"
            },
            "schema:domainIncludes": [
                {
                    "@id": "tourism:BasicPrice"
                },
                {
                    "@id": "tourism:CancellationPrice"
                },
                {
                    "@id": "tourism:DiscountPrice"
                },
                {
                    "@id": "tourism:ExtraPrice"
                },
                {
                    "@id": "tourism:LodgingHouseTravelProduct"
                }
            ],
            "rdfs:comment": [
                "A customer class applicable to a discount price.",
                "A customer class applicable to the basic price.",
                "A customer class applicable to the cancellation price.",
                "A customer class applicable to the extra price.",
                "A customer class applicable to this lodging house travel product.",
                "A lodging house customer class applicable to this basic price.",
                "A lodging house customer class applicable to this cancellation price.",
                "A lodging house customer class applicable to this discount price.",
                "A lodging house customer class applicable to this extra price."
            ],
            "rdfs:label": "applicableCustomerClass",
            "unece:cefactElementMetadata": [
                {
                    "@id": "cefact:Cancellation_Price.Applicable.CustomerClass",
                    "@type": "unece:AssociationBIE",
                    "unece:cefactUNId": "UN01005084",
                    "unece:cefactBieDomainClass": "cefact:Cancellation_Price.Details",
                    "rdfs:comment": "A customer class applicable to the cancellation price."
                },
                {
                    "@id": "cefact:Discount_Price.Applicable.CustomerClass",
                    "@type": "unece:AssociationBIE",
                    "unece:cefactUNId": "UN01005052",
                    "unece:cefactBieDomainClass": "cefact:Discount_Price.Details",
                    "rdfs:comment": "A customer class applicable to a discount price."
                },
                {
                    "@id": "cefact:Discount_Price.Applicable.LodgingHouse_CustomerClass",
                    "@type": "unece:AssociationBIE",
                    "unece:cefactUNId": "UN01010192",
                    "unece:cefactBieDomainClass": "cefact:Discount_Price.Details",
                    "rdfs:comment": "A lodging house customer class applicable to this discount price."
                },
                {
                    "@id": "cefact:LodgingHouse_TravelProduct.Applicable.CustomerClass",
                    "@type": "unece:AssociationBIE",
                    "unece:cefactUNId": "UN01004932",
                    "unece:cefactBieDomainClass": "cefact:LodgingHouse_TravelProduct.Details",
                    "rdfs:comment": "A customer class applicable to this lodging house travel product."
                },
                {
                    "@id": "cefact:Extra_Price.Applicable.CustomerClass",
                    "@type": "unece:AssociationBIE",
                    "unece:cefactUNId": "UN01005033",
                    "unece:cefactBieDomainClass": "cefact:Extra_Price.Details",
                    "rdfs:comment": "A customer class applicable to the extra price."
                },
                {
                    "@id": "cefact:LodgingHouse_TravelProduct.Applicable.LodgingHouse_CustomerClass",
                    "@type": "unece:AssociationBIE",
                    "unece:cefactUNId": "UN01010196",
                    "unece:cefactBieDomainClass": "cefact:LodgingHouse_TravelProduct.Details",
                    "rdfs:comment": "A customer class applicable to this lodging house travel product."
                },
                {
                    "@id": "cefact:Basic_Price.Applicable.CustomerClass",
                    "@type": "unece:AssociationBIE",
                    "unece:cefactUNId": "UN01005014",
                    "unece:cefactBieDomainClass": "cefact:Basic_Price.Details",
                    "rdfs:comment": "A customer class applicable to the basic price."
                },
                {
                    "@id": "cefact:Extra_Price.Applicable.LodgingHouse_CustomerClass",
                    "@type": "unece:AssociationBIE",
                    "unece:cefactUNId": "UN01010193",
                    "unece:cefactBieDomainClass": "cefact:Extra_Price.Details",
                    "rdfs:comment": "A lodging house customer class applicable to this extra price."
                },
                {
                    "@id": "cefact:Basic_Price.Applicable.LodgingHouse_CustomerClass",
                    "@type": "unece:AssociationBIE",
                    "unece:cefactUNId": "UN01010190",
                    "unece:cefactBieDomainClass": "cefact:Basic_Price.Details",
                    "rdfs:comment": "A lodging house customer class applicable to this basic price."
                },
                {
                    "@id": "cefact:Cancellation_Price.Applicable.LodgingHouse_CustomerClass",
                    "@type": "unece:AssociationBIE",
                    "unece:cefactUNId": "UN01010191",
                    "unece:cefactBieDomainClass": "cefact:Cancellation_Price.Details",
                    "rdfs:comment": "A lodging house customer class applicable to this cancellation price."
                }
            ]
        },
        {
            "@id": "tourism:applicableIndicator",
            "@type": "rdf:Property",
            "schema:rangeIncludes": {
                "@id": "xsd:boolean"
            },
            "schema:domainIncludes": {
                "@id": "tourism:ExperienceItemVoucher"
            },
            "rdfs:comment": "The indication of whether or not this experience item voucher is applicable.",
            "rdfs:label": "applicableIndicator",
            "unece:cefactElementMetadata": [
                {
                    "@id": "cefact:ExperienceItem_Voucher.Applicable.Indicator",
                    "@type": "unece:BasicBIE",
                    "unece:cefactUNId": "UN01015248",
                    "unece:cefactBieDomainClass": "cefact:ExperienceItem_Voucher.Details",
                    "rdfs:comment": "The indication of whether or not this experience item voucher is applicable."
                }
            ]
        },
        {
            "@id": "tourism:applicableNote",
            "@type": "rdf:Property",
            "schema:rangeIncludes": {
                "@id": "tourism:Note"
            },
            "schema:domainIncludes": [
                {
                    "@id": "tourism:ExperienceEvent"
                },
                {
                    "@id": "tourism:ExperienceProduct"
                },
                {
                    "@id": "tourism:GuestPerson"
                }
            ],
            "rdfs:comment": [
                "A note applicable for this experience product.",
                "A note applicable to this guest person.",
                "A specified note applicable for this experience event."
            ],
            "rdfs:label": "applicableNote",
            "unece:cefactElementMetadata": [
                {
                    "@id": "cefact:Guest_Person.Applicable.Specified_Note",
                    "@type": "unece:AssociationBIE",
                    "unece:cefactUNId": "UN01015223",
                    "unece:cefactBieDomainClass": "cefact:Guest_Person.Details",
                    "rdfs:comment": "A note applicable to this guest person."
                },
                {
                    "@id": "cefact:Experience_Product.Applicable.Specified_Note",
                    "@type": "unece:AssociationBIE",
                    "unece:cefactUNId": "UN01015180",
                    "unece:cefactBieDomainClass": "cefact:Experience_Product.Details",
                    "rdfs:comment": "A note applicable for this experience product."
                },
                {
                    "@id": "cefact:Experience_Event.Applicable.Specified_Note",
                    "@type": "unece:AssociationBIE",
                    "unece:cefactUNId": "UN01015136",
                    "unece:cefactBieDomainClass": "cefact:Experience_Event.Details",
                    "rdfs:comment": "A specified note applicable for this experience event."
                }
            ]
        },
        {
            "@id": "tourism:applicablePayment",
            "@type": "rdf:Property",
            "schema:rangeIncludes": {
                "@id": "tourism:Payment"
            },
            "schema:domainIncludes": {
                "@id": "tourism:LodgingHouseReservation"
            },
            "rdfs:comment": "A payment applicable for this lodging house reservation.",
            "rdfs:label": "applicablePayment",
            "unece:cefactElementMetadata": [
                {
                    "@id": "cefact:LodgingHouse_Reservation.Applicable.Travel_Payment",
                    "@type": "unece:AssociationBIE",
                    "unece:cefactUNId": "UN01009804",
                    "unece:cefactBieDomainClass": "cefact:LodgingHouse_Reservation.Details",
                    "rdfs:comment": "A payment applicable for this lodging house reservation."
                }
            ]
        },
        {
            "@id": "tourism:applicablePeriod",
            "@type": "rdf:Property",
            "schema:rangeIncludes": {
                "@id": "tourism:Period"
            },
            "schema:domainIncludes": {
                "@id": "tourism:LodgingHouseTravelProduct"
            },
            "rdfs:comment": "A period applicable to this lodging house travel product.",
            "rdfs:label": "applicablePeriod",
            "unece:cefactElementMetadata": [
                {
                    "@id": "cefact:LodgingHouse_TravelProduct.Applicable.TravelProduct_Period",
                    "@type": "unece:AssociationBIE",
                    "unece:cefactUNId": "UN01004936",
                    "unece:cefactBieDomainClass": "cefact:LodgingHouse_TravelProduct.Details",
                    "rdfs:comment": "A period applicable to this lodging house travel product."
                }
            ]
        },
        {
            "@id": "tourism:applicablePrice",
            "@type": "rdf:Property",
            "schema:rangeIncludes": {
                "@id": "tourism:Price"
            },
            "schema:domainIncludes": {
                "@id": "tourism:LodgingHouseTravelProduct"
            },
            "rdfs:comment": [
                "A basic price applicable to this lodging house travel product.",
                "A cancellation price applicable to this lodging house travel product.",
                "A discount price applicable to this lodging house travel product.",
                "A service price applicable to this lodging house travel product.",
                "An extra price applicable to this lodging house travel product."
            ],
            "rdfs:label": "applicablePrice",
            "unece:cefactElementMetadata": [
                {
                    "@id": "cefact:LodgingHouse_TravelProduct.Applicable.Discount_Price",
                    "@type": "unece:AssociationBIE",
                    "unece:cefactUNId": "UN01004941",
                    "unece:cefactBieDomainClass": "cefact:LodgingHouse_TravelProduct.Details",
                    "rdfs:comment": "A discount price applicable to this lodging house travel product."
                },
                {
                    "@id": "cefact:LodgingHouse_TravelProduct.Applicable.Cancellation_Price",
                    "@type": "unece:AssociationBIE",
                    "unece:cefactUNId": "UN01004944",
                    "unece:cefactBieDomainClass": "cefact:LodgingHouse_TravelProduct.Details",
                    "rdfs:comment": "A cancellation price applicable to this lodging house travel product."
                },
                {
                    "@id": "cefact:LodgingHouse_TravelProduct.Applicable.Basic_Price",
                    "@type": "unece:AssociationBIE",
                    "unece:cefactUNId": "UN01004939",
                    "unece:cefactBieDomainClass": "cefact:LodgingHouse_TravelProduct.Details",
                    "rdfs:comment": "A basic price applicable to this lodging house travel product."
                },
                {
                    "@id": "cefact:LodgingHouse_TravelProduct.Applicable.Service_Price",
                    "@type": "unece:AssociationBIE",
                    "unece:cefactUNId": "UN01004942",
                    "unece:cefactBieDomainClass": "cefact:LodgingHouse_TravelProduct.Details",
                    "rdfs:comment": "A service price applicable to this lodging house travel product."
                },
                {
                    "@id": "cefact:LodgingHouse_TravelProduct.Applicable.Extra_Price",
                    "@type": "unece:AssociationBIE",
                    "unece:cefactUNId": "UN01004940",
                    "unece:cefactBieDomainClass": "cefact:LodgingHouse_TravelProduct.Details",
                    "rdfs:comment": "An extra price applicable to this lodging house travel product."
                }
            ]
        },
        {
            "@id": "tourism:applicableQuantityUnitTypeCode",
            "@type": "rdf:Property",
            "schema:rangeIncludes": {
                "@id": "xsd:token"
            },
            "schema:domainIncludes": {
                "@id": "tourism:ExperienceProduct"
            },
            "rdfs:comment": "The code specifying the type of quantity unit applicable for this experience product.",
            "rdfs:label": "applicableQuantityUnitTypeCode",
            "unece:cefactElementMetadata": [
                {
                    "@id": "cefact:Experience_Product.ApplicableQuantityUnit_Type.Code",
                    "@type": "unece:BasicBIE",
                    "unece:cefactUNId": "UN01015171",
                    "unece:cefactBieDomainClass": "cefact:Experience_Product.Details",
                    "rdfs:comment": "The code specifying the type of quantity unit applicable for this experience product."
                }
            ]
        },
        {
            "@id": "tourism:applicableTax",
            "@type": "rdf:Property",
            "schema:rangeIncludes": {
                "@id": "tourism:Tax"
            },
            "schema:domainIncludes": {
                "@id": "tourism:LodgingHouseTravelProduct"
            },
            "rdfs:comment": "A tax applicable to this lodging house travel product.",
            "rdfs:label": "applicableTax",
            "unece:cefactElementMetadata": [
                {
                    "@id": "cefact:LodgingHouse_TravelProduct.Applicable.TravelProduct_Tax",
                    "@type": "unece:AssociationBIE",
                    "unece:cefactUNId": "UN01004943",
                    "unece:cefactBieDomainClass": "cefact:LodgingHouse_TravelProduct.Details",
                    "rdfs:comment": "A tax applicable to this lodging house travel product."
                }
            ]
        },
        {
            "@id": "tourism:applicableUnitQuantity",
            "@type": "rdf:Property",
            "schema:rangeIncludes": {
                "@id": "xsd:decimal"
            },
            "schema:domainIncludes": {
                "@id": "tourism:LodgingHouseTravelProductSubComponent"
            },
            "rdfs:comment": "The number of units applicable to this lodging house travel product sub-component.",
            "rdfs:label": "applicableUnitQuantity",
            "unece:cefactElementMetadata": [
                {
                    "@id": "cefact:LodgingHouse_TravelProductSub-Component.ApplicableUnit.Quantity",
                    "@type": "unece:BasicBIE",
                    "unece:cefactUNId": "UN01004992",
                    "unece:cefactBieDomainClass": "cefact:LodgingHouse_TravelProductSubComponent.Details",
                    "rdfs:comment": "The number of units applicable to this lodging house travel product sub-component."
                }
            ]
        },
        {
            "@id": "tourism:applicableUsageCondition",
            "@type": "rdf:Property",
            "schema:rangeIncludes": {
                "@id": "tourism:UsageCondition"
            },
            "schema:domainIncludes": {
                "@id": "tourism:LodgingHouseTravelProductSubComponent"
            },
            "rdfs:comment": [
                "A usage condition applicable to this lodging house travel product sub-component.",
                "An applicable usage condition for this lodging house travel product sub-component."
            ],
            "rdfs:label": "applicableUsageCondition",
            "unece:cefactElementMetadata": [
                {
                    "@id": "cefact:LodgingHouse_TravelProductSub-Component.Applicable.UsageCondition",
                    "@type": "unece:AssociationBIE",
                    "unece:cefactUNId": "UN01004997",
                    "unece:cefactBieDomainClass": "cefact:LodgingHouse_TravelProductSubComponent.Details",
                    "rdfs:comment": "A usage condition applicable to this lodging house travel product sub-component."
                },
                {
                    "@id": "cefact:LodgingHouse_TravelProductSub-Component.Applicable.LodgingHouse_UsageCondition",
                    "@type": "unece:AssociationBIE",
                    "unece:cefactUNId": "UN01010195",
                    "unece:cefactBieDomainClass": "cefact:LodgingHouse_TravelProductSubComponent.Details",
                    "rdfs:comment": "An applicable usage condition for this lodging house travel product sub-component."
                }
            ]
        },
        {
            "@id": "tourism:appropriateClothing",
            "@type": "rdf:Property",
            "schema:rangeIncludes": {
                "@id": "xsd:string"
            },
            "schema:domainIncludes": {
                "@id": "tourism:LodgingHouseUsageCondition"
            },
            "rdfs:comment": "The appropriate clothing, expressed as text, applicable to this lodging house usage condition.",
            "rdfs:label": "appropriateClothing",
            "unece:cefactElementMetadata": [
                {
                    "@id": "cefact:LodgingHouse_UsageCondition.AppropriateClothing.Text",
                    "@type": "unece:BasicBIE",
                    "unece:cefactUNId": "UN01001208",
                    "unece:cefactBieDomainClass": "cefact:LodgingHouse_UsageCondition.Details",
                    "rdfs:comment": "The appropriate clothing, expressed as text, applicable to this lodging house usage condition."
                }
            ]
        },
        {
            "@id": "tourism:architecturalStyle",
            "@type": "rdf:Property",
            "schema:rangeIncludes": {
                "@id": "xsd:string"
            },
            "schema:domainIncludes": [
                {
                    "@id": "tourism:BathingFacility"
                },
                {
                    "@id": "tourism:BusinessSupportRoomFacility"
                },
                {
                    "@id": "tourism:ExperienceFacility"
                },
                {
                    "@id": "tourism:GuestRoomFacility"
                },
                {
                    "@id": "tourism:LodgingHouseBuilding"
                }
            ],
            "rdfs:comment": [
                "An architectural style, expressed as text, of this experience facility.",
                "The architectural style, expressed as text, of this bathing facility.",
                "The architectural style, expressed as text, of this business support room.",
                "The architectural style, expressed as text, of this guest room.",
                "The architectural style, expressed as text, of this lodging house building."
            ],
            "rdfs:label": "architecturalStyle",
            "unece:cefactElementMetadata": [
                {
                    "@id": "cefact:Bathing_Facility.Architectural_Style.Text",
                    "@type": "unece:BasicBIE",
                    "unece:cefactUNId": "UN01001064",
                    "unece:cefactBieDomainClass": "cefact:Bathing_Facility.Details",
                    "rdfs:comment": "The architectural style, expressed as text, of this bathing facility."
                },
                {
                    "@id": "cefact:Experience_Facility.Architectural_Style.Text",
                    "@type": "unece:BasicBIE",
                    "unece:cefactUNId": "UN01015142",
                    "unece:cefactBieDomainClass": "cefact:Experience_Facility.Details",
                    "rdfs:comment": "An architectural style, expressed as text, of this experience facility."
                },
                {
                    "@id": "cefact:GuestRoom_Facility.Architectural_Style.Text",
                    "@type": "unece:BasicBIE",
                    "unece:cefactUNId": "UN01001050",
                    "unece:cefactBieDomainClass": "cefact:GuestRoom_Facility.Details",
                    "rdfs:comment": "The architectural style, expressed as text, of this guest room."
                },
                {
                    "@id": "cefact:BusinessSupportRoom_Facility.Architectural_Style.Text",
                    "@type": "unece:BasicBIE",
                    "unece:cefactUNId": "UN01001108",
                    "unece:cefactBieDomainClass": "cefact:BusinessSupportRoom_Facility.Details",
                    "rdfs:comment": "The architectural style, expressed as text, of this business support room."
                },
                {
                    "@id": "cefact:LodgingHouse_Building.Architectural_Style.Text",
                    "@type": "unece:BasicBIE",
                    "unece:cefactUNId": "UN01001041",
                    "unece:cefactBieDomainClass": "cefact:LodgingHouse_Building.Details",
                    "rdfs:comment": "The architectural style, expressed as text, of this lodging house building."
                }
            ]
        },
        {
            "@id": "tourism:areaIncluded",
            "@type": "rdf:Property",
            "schema:rangeIncludes": {
                "@id": "xsd:string"
            },
            "schema:domainIncludes": {
                "@id": "tourism:LodgingHousePicture"
            },
            "rdfs:comment": "The area or location, expressed as text, that is included for this lodging house picture.",
            "rdfs:label": "areaIncluded",
            "unece:cefactElementMetadata": [
                {
                    "@id": "cefact:LodgingHouse_Picture.AreaIncluded.Text",
                    "@type": "unece:BasicBIE",
                    "unece:cefactUNId": "UN01001250",
                    "unece:cefactBieDomainClass": "cefact:LodgingHouse_Picture.Details",
                    "rdfs:comment": "The area or location, expressed as text, that is included for this lodging house picture."
                }
            ]
        },
        {
            "@id": "tourism:associationMembershipName",
            "@type": "rdf:Property",
            "schema:rangeIncludes": {
                "@id": "xsd:string"
            },
            "schema:domainIncludes": {
                "@id": "tourism:LodgingHouseOrganization"
            },
            "rdfs:comment": "A name, expressed as text, of an association membership held by this lodging house organization, such as the Japan Ryokan Association or the Hotel Electronic Distribution Network Association.",
            "rdfs:label": "associationMembershipName",
            "unece:cefactElementMetadata": [
                {
                    "@id": "cefact:LodgingHouse_Organization.AssociationMembership_Name.Text",
                    "@type": "unece:BasicBIE",
                    "unece:cefactUNId": "UN01001033",
                    "unece:cefactBieDomainClass": "cefact:LodgingHouse_Organization.Details",
                    "rdfs:comment": "A name, expressed as text, of an association membership held by this lodging house organization, such as the Japan Ryokan Association or the Hotel Electronic Distribution Network Association."
                }
            ]
        },
        {
            "@id": "tourism:automaticExtensionIndicator",
            "@type": "rdf:Property",
            "schema:rangeIncludes": {
                "@id": "xsd:boolean"
            },
            "schema:domainIncludes": {
                "@id": "tourism:LodgingHouseContract"
            },
            "rdfs:comment": "The indication of whether or not this lodging house contract can be or has been automatically extended.",
            "rdfs:label": "automaticExtensionIndicator",
            "unece:cefactElementMetadata": [
                {
                    "@id": "cefact:LodgingHouse_Contract.Automatic_Extension.Indicator",
                    "@type": "unece:BasicBIE",
                    "unece:cefactUNId": "UN01001214",
                    "unece:cefactBieDomainClass": "cefact:LodgingHouse_Contract.Details",
                    "rdfs:comment": "The indication of whether or not this lodging house contract can be or has been automatically extended."
                }
            ]
        },
        {
            "@id": "tourism:availablePeriod",
            "@type": "rdf:Property",
            "schema:rangeIncludes": {
                "@id": "tourism:Period"
            },
            "schema:domainIncludes": {
                "@id": "tourism:LodgingHouseContact"
            },
            "rdfs:comment": "A period during which this lodging house contact is available.",
            "rdfs:label": "availablePeriod",
            "unece:cefactElementMetadata": [
                {
                    "@id": "cefact:LodgingHouse_Contact.Available.Specified_Period",
                    "@type": "unece:AssociationBIE",
                    "unece:cefactUNId": "UN01001232",
                    "unece:cefactBieDomainClass": "cefact:LodgingHouse_Contact.Details",
                    "rdfs:comment": "A period during which this lodging house contact is available."
                }
            ]
        },
        {
            "@id": "tourism:availableRoute",
            "@type": "rdf:Property",
            "schema:rangeIncludes": {
                "@id": "tourism:Route"
            },
            "schema:domainIncludes": {
                "@id": "tourism:ExperienceFacility"
            },
            "rdfs:comment": "An available route specified for this experience facility.",
            "rdfs:label": "availableRoute",
            "unece:cefactElementMetadata": [
                {
                    "@id": "cefact:Experience_Facility.Available.Specified_Route",
                    "@type": "unece:AssociationBIE",
                    "unece:cefactUNId": "UN01015147",
                    "unece:cefactBieDomainClass": "cefact:Experience_Facility.Details",
                    "rdfs:comment": "An available route specified for this experience facility."
                }
            ]
        },
        {
            "@id": "tourism:basicChargeAmount",
            "@type": "rdf:Property",
            "schema:rangeIncludes": {
                "@id": "xsd:decimal"
            },
            "schema:domainIncludes": {
                "@id": "tourism:DailyPrice"
            },
            "rdfs:comment": "The monetary value of the basic price charged on which this daily price is calculated.",
            "rdfs:label": "basicChargeAmount",
            "unece:cefactElementMetadata": [
                {
                    "@id": "cefact:Daily_Price.Basic_Charge.Amount",
                    "@type": "unece:BasicBIE",
                    "unece:cefactUNId": "UN01009689",
                    "unece:cefactBieDomainClass": "cefact:Daily_Price.Details",
                    "rdfs:comment": "The monetary value of the basic price charged on which this daily price is calculated."
                }
            ]
        },
        {
            "@id": "tourism:basicObjective",
            "@type": "rdf:Property",
            "schema:rangeIncludes": {
                "@id": "xsd:string"
            },
            "schema:domainIncludes": {
                "@id": "tourism:ExperienceEvent"
            },
            "rdfs:comment": "A basic objective, expressed as text, for this experience event.",
            "rdfs:label": "basicObjective",
            "unece:cefactElementMetadata": [
                {
                    "@id": "cefact:Experience_Event.Basic_Objective.Text",
                    "@type": "unece:BasicBIE",
                    "unece:cefactUNId": "UN01015118",
                    "unece:cefactBieDomainClass": "cefact:Experience_Event.Details",
                    "rdfs:comment": "A basic objective, expressed as text, for this experience event."
                }
            ]
        },
        {
            "@id": "tourism:basicPriceBracketTypeCode",
            "@type": "rdf:Property",
            "schema:rangeIncludes": {
                "@id": "unece:UNECECL5375Code"
            },
            "schema:domainIncludes": {
                "@id": "tourism:BasicPrice"
            },
            "rdfs:comment": "The code specifying the bracket type of this basic price.",
            "rdfs:label": "basicPriceBracketTypeCode",
            "unece:cefactElementMetadata": [
                {
                    "@id": "cefact:Basic_Price.Bracket_Type.Code",
                    "@type": "unece:BasicBIE",
                    "unece:TDED": "5375",
                    "unece:cefactUNId": "UN01005003",
                    "unece:cefactBieDomainClass": "cefact:Basic_Price.Details",
                    "rdfs:comment": "The code specifying the bracket type of this basic price."
                }
            ]
        },
        {
            "@id": "tourism:basicPriceTypeCode",
            "@type": "rdf:Property",
            "schema:rangeIncludes": {
                "@id": "unece:UNECECL5375Code"
            },
            "schema:domainIncludes": {
                "@id": "tourism:BasicPrice"
            },
            "rdfs:comment": "The code specifying the type of basic price.",
            "rdfs:label": "basicPriceTypeCode",
            "unece:cefactElementMetadata": [
                {
                    "@id": "cefact:Basic_Price.Type.Code",
                    "@type": "unece:BasicBIE",
                    "unece:TDED": "5375",
                    "unece:cefactUNId": "UN01005000",
                    "unece:cefactBieDomainClass": "cefact:Basic_Price.Details",
                    "rdfs:comment": "The code specifying the type of basic price."
                }
            ]
        },
        {
            "@id": "tourism:basisQuantity",
            "@type": "rdf:Property",
            "schema:rangeIncludes": {
                "@id": "xsd:decimal"
            },
            "schema:domainIncludes": [
                {
                    "@id": "tourism:BasicPrice"
                },
                {
                    "@id": "tourism:CancellationPrice"
                },
                {
                    "@id": "tourism:DiscountPrice"
                },
                {
                    "@id": "tourism:ExtraPrice"
                }
            ],
            "rdfs:comment": [
                "The quantity on which the basic price is based.",
                "The quantity on which the cancellation price is based.",
                "The quantity on which the discount price is based.",
                "The quantity on which the extra price is based."
            ],
            "rdfs:label": "basisQuantity",
            "unece:cefactElementMetadata": [
                {
                    "@id": "cefact:Discount_Price.Basis.Quantity",
                    "@type": "unece:BasicBIE",
                    "unece:TDED": "5310",
                    "unece:cefactUNId": "UN01005038",
                    "unece:cefactBieDomainClass": "cefact:Discount_Price.Details",
                    "rdfs:comment": "The quantity on which the discount price is based."
                },
                {
                    "@id": "cefact:Cancellation_Price.Basis.Quantity",
                    "@type": "unece:BasicBIE",
                    "unece:TDED": "5310",
                    "unece:cefactUNId": "UN01005077",
                    "unece:cefactBieDomainClass": "cefact:Cancellation_Price.Details",
                    "rdfs:comment": "The quantity on which the cancellation price is based."
                },
                {
                    "@id": "cefact:Extra_Price.Basis.Quantity",
                    "@type": "unece:BasicBIE",
                    "unece:TDED": "5310",
                    "unece:cefactUNId": "UN01005019",
                    "unece:cefactBieDomainClass": "cefact:Extra_Price.Details",
                    "rdfs:comment": "The quantity on which the extra price is based."
                },
                {
                    "@id": "cefact:Basic_Price.Basis.Quantity",
                    "@type": "unece:BasicBIE",
                    "unece:TDED": "5310",
                    "unece:cefactUNId": "UN01005004",
                    "unece:cefactBieDomainClass": "cefact:Basic_Price.Details",
                    "rdfs:comment": "The quantity on which the basic price is based."
                }
            ]
        },
        {
            "@id": "tourism:birthDateTime",
            "@type": "rdf:Property",
            "schema:rangeIncludes": {
                "@id": "xsd:dateTime"
            },
            "schema:domainIncludes": {
                "@id": "tourism:GuestPerson"
            },
            "rdfs:comment": "The date, time, date time, or other date time value which specifies the birth date for this guest.",
            "rdfs:label": "birthDateTime",
            "unece:cefactElementMetadata": [
                {
                    "@id": "cefact:Guest_Person.Birth.DateTime",
                    "@type": "unece:BasicBIE",
                    "unece:TDED": "2491",
                    "unece:cefactUNId": "UN01009713",
                    "unece:cefactBieDomainClass": "cefact:Guest_Person.Details",
                    "rdfs:comment": "The date, time, date time, or other date time value which specifies the birth date for this guest."
                }
            ]
        },
        {
            "@id": "tourism:brandName",
            "@type": "rdf:Property",
            "schema:rangeIncludes": {
                "@id": "xsd:string"
            },
            "schema:domainIncludes": [
                {
                    "@id": "tourism:ExperienceProduct"
                },
                {
                    "@id": "tourism:LodgingHouseOrganization"
                },
                {
                    "@id": "tourism:LodgingHouseTravelProduct"
                }
            ],
            "rdfs:comment": [
                "A brand name, expressed as text, for this experience product.",
                "A brand name, expressed as text, for this lodging house organization.",
                "The brand name, expressed as text, of this lodging house travel product."
            ],
            "rdfs:label": "brandName",
            "unece:cefactElementMetadata": [
                {
                    "@id": "cefact:LodgingHouse_Organization.Brand_Name.Text",
                    "@type": "unece:BasicBIE",
                    "unece:cefactUNId": "UN01001030",
                    "unece:cefactBieDomainClass": "cefact:LodgingHouse_Organization.Details",
                    "rdfs:comment": "A brand name, expressed as text, for this lodging house organization."
                },
                {
                    "@id": "cefact:LodgingHouse_TravelProduct.Brand_Name.Text",
                    "@type": "unece:BasicBIE",
                    "unece:cefactUNId": "UN01004920",
                    "unece:cefactBieDomainClass": "cefact:LodgingHouse_TravelProduct.Details",
                    "rdfs:comment": "The brand name, expressed as text, of this lodging house travel product."
                },
                {
                    "@id": "cefact:Experience_Product.Brand_Name.Text",
                    "@type": "unece:BasicBIE",
                    "unece:TDED": "7134",
                    "unece:cefactUNId": "UN01015161",
                    "unece:cefactBieDomainClass": "cefact:Experience_Product.Details",
                    "rdfs:comment": "A brand name, expressed as text, for this experience product."
                }
            ]
        },
        {
            "@id": "tourism:breakUpDateTime",
            "@type": "rdf:Property",
            "schema:rangeIncludes": {
                "@id": "xsd:dateTime"
            },
            "schema:domainIncludes": {
                "@id": "tourism:ExperienceEvent"
            },
            "rdfs:comment": "The break up date, time, date time, or other date time value for this experience event.",
            "rdfs:label": "breakUpDateTime",
            "unece:cefactElementMetadata": [
                {
                    "@id": "cefact:Experience_Event.BreakUp.DateTime",
                    "@type": "unece:BasicBIE",
                    "unece:cefactUNId": "UN01015124",
                    "unece:cefactBieDomainClass": "cefact:Experience_Event.Details",
                    "rdfs:comment": "The break up date, time, date time, or other date time value for this experience event."
                }
            ]
        },
        {
            "@id": "tourism:businessTypeCode",
            "@type": "rdf:Property",
            "schema:rangeIncludes": {
                "@id": "xsd:token"
            },
            "schema:domainIncludes": {
                "@id": "tourism:LodgingHouseOrganization"
            },
            "rdfs:comment": "A code specifying the business type of this lodging house organization.",
            "rdfs:label": "businessTypeCode",
            "unece:cefactElementMetadata": [
                {
                    "@id": "cefact:LodgingHouse_Organization.BusinessType.Code",
                    "@type": "unece:BasicBIE",
                    "unece:cefactUNId": "UN01001032",
                    "unece:cefactBieDomainClass": "cefact:LodgingHouse_Organization.Details",
                    "rdfs:comment": "A code specifying the business type of this lodging house organization."
                }
            ]
        },
        {
            "@id": "tourism:calculatedPrice",
            "@type": "rdf:Property",
            "schema:rangeIncludes": {
                "@id": "tourism:Price"
            },
            "schema:domainIncludes": [
                {
                    "@id": "tourism:ExperienceEvent"
                },
                {
                    "@id": "tourism:ExperienceProduct"
                }
            ],
            "rdfs:comment": [
                "A calculated price for this experience event.",
                "A calculated price for this experience product."
            ],
            "rdfs:label": "calculatedPrice",
            "unece:cefactElementMetadata": [
                {
                    "@id": "cefact:Experience_Product.Calculated.Trade_Price",
                    "@type": "unece:AssociationBIE",
                    "unece:cefactUNId": "UN01015181",
                    "unece:cefactBieDomainClass": "cefact:Experience_Product.Details",
                    "rdfs:comment": "A calculated price for this experience product."
                },
                {
                    "@id": "cefact:Experience_Event.Calculated.Trade_Price",
                    "@type": "unece:AssociationBIE",
                    "unece:cefactUNId": "UN01015134",
                    "unece:cefactBieDomainClass": "cefact:Experience_Event.Details",
                    "rdfs:comment": "A calculated price for this experience event."
                }
            ]
        },
        {
            "@id": "tourism:calculationPercent",
            "@type": "rdf:Property",
            "schema:rangeIncludes": {
                "@id": "xsd:decimal"
            },
            "schema:domainIncludes": [
                {
                    "@id": "tourism:CancellationPrice"
                },
                {
                    "@id": "tourism:DiscountPrice"
                },
                {
                    "@id": "tourism:ExtraPrice"
                }
            ],
            "rdfs:comment": [
                "The percentage applied to calculate the cancellation price.",
                "The percentage applied to calculate the discount price.",
                "The percentage applied to calculate the extra price."
            ],
            "rdfs:label": "calculationPercent",
            "unece:cefactElementMetadata": [
                {
                    "@id": "cefact:Discount_Price.Calculation.Percent",
                    "@type": "unece:BasicBIE",
                    "unece:cefactUNId": "UN01005041",
                    "unece:cefactBieDomainClass": "cefact:Discount_Price.Details",
                    "rdfs:comment": "The percentage applied to calculate the discount price."
                },
                {
                    "@id": "cefact:Cancellation_Price.Calculation.Percent",
                    "@type": "unece:BasicBIE",
                    "unece:cefactUNId": "UN01005080",
                    "unece:cefactBieDomainClass": "cefact:Cancellation_Price.Details",
                    "rdfs:comment": "The percentage applied to calculate the cancellation price."
                },
                {
                    "@id": "cefact:Extra_Price.Calculation.Percent",
                    "@type": "unece:BasicBIE",
                    "unece:cefactUNId": "UN01005022",
                    "unece:cefactBieDomainClass": "cefact:Extra_Price.Details",
                    "rdfs:comment": "The percentage applied to calculate the extra price."
                }
            ]
        },
        {
            "@id": "tourism:cancellationAcceptedDateTime",
            "@type": "rdf:Property",
            "schema:rangeIncludes": {
                "@id": "xsd:dateTime"
            },
            "schema:domainIncludes": {
                "@id": "tourism:LodgingHouseReservation"
            },
            "rdfs:comment": "The date, time, date time, or other date time value when the cancellation was accepted for this lodging house reservation.",
            "rdfs:label": "cancellationAcceptedDateTime",
            "unece:cefactElementMetadata": [
                {
                    "@id": "cefact:LodgingHouse_Reservation.CancellationAccepted.DateTime",
                    "@type": "unece:BasicBIE",
                    "unece:cefactUNId": "UN01009799",
                    "unece:cefactBieDomainClass": "cefact:LodgingHouse_Reservation.Details",
                    "rdfs:comment": "The date, time, date time, or other date time value when the cancellation was accepted for this lodging house reservation."
                }
            ]
        },
        {
            "@id": "tourism:cancellationChargeAmount",
            "@type": "rdf:Property",
            "schema:rangeIncludes": {
                "@id": "xsd:decimal"
            },
            "schema:domainIncludes": {
                "@id": "tourism:DailyPrice"
            },
            "rdfs:comment": "The monetary value of the cancellation price charged on which this daily price is calculated.",
            "rdfs:label": "cancellationChargeAmount",
            "unece:cefactElementMetadata": [
                {
                    "@id": "cefact:Daily_Price.Cancellation_Charge.Amount",
                    "@type": "unece:BasicBIE",
                    "unece:cefactUNId": "UN01009697",
                    "unece:cefactBieDomainClass": "cefact:Daily_Price.Details",
                    "rdfs:comment": "The monetary value of the cancellation price charged on which this daily price is calculated."
                }
            ]
        },
        {
            "@id": "tourism:cancellationChargeApplicableIndicator",
            "@type": "rdf:Property",
            "schema:rangeIncludes": {
                "@id": "xsd:boolean"
            },
            "schema:domainIncludes": [
                {
                    "@id": "tourism:BasicPrice"
                },
                {
                    "@id": "tourism:DiscountPrice"
                },
                {
                    "@id": "tourism:ExtraPrice"
                }
            ],
            "rdfs:comment": [
                "The indication of whether or not a cancellation charge is applicable to the discount price.",
                "The indication of whether or not a cancellation charge is applicable to the extra price.",
                "The indication of whether or not the cancellation charge is applicable to the basic price."
            ],
            "rdfs:label": "cancellationChargeApplicableIndicator",
            "unece:cefactElementMetadata": [
                {
                    "@id": "cefact:Discount_Price.Cancellation_ChargeApplicable.Indicator",
                    "@type": "unece:BasicBIE",
                    "unece:cefactUNId": "UN01005044",
                    "unece:cefactBieDomainClass": "cefact:Discount_Price.Details",
                    "rdfs:comment": "The indication of whether or not a cancellation charge is applicable to the discount price."
                },
                {
                    "@id": "cefact:Extra_Price.Cancellation_ChargeApplicable.Indicator",
                    "@type": "unece:BasicBIE",
                    "unece:cefactUNId": "UN01005025",
                    "unece:cefactBieDomainClass": "cefact:Extra_Price.Details",
                    "rdfs:comment": "The indication of whether or not a cancellation charge is applicable to the extra price."
                },
                {
                    "@id": "cefact:Basic_Price.Cancellation_ChargeApplicable.Indicator",
                    "@type": "unece:BasicBIE",
                    "unece:cefactUNId": "UN01005009",
                    "unece:cefactBieDomainClass": "cefact:Basic_Price.Details",
                    "rdfs:comment": "The indication of whether or not the cancellation charge is applicable to the basic price."
                }
            ]
        },
        {
            "@id": "tourism:cancellationId",
            "@type": "rdf:Property",
            "schema:rangeIncludes": {
                "@id": "xsd:token"
            },
            "schema:domainIncludes": {
                "@id": "tourism:LodgingHouseReservation"
            },
            "rdfs:comment": "The identifier of the cancellation for this lodging house reservation.",
            "rdfs:label": "cancellationId",
            "unece:cefactElementMetadata": [
                {
                    "@id": "cefact:LodgingHouse_Reservation.Cancellation.Identifier",
                    "@type": "unece:BasicBIE",
                    "unece:cefactUNId": "UN01009798",
                    "unece:cefactBieDomainClass": "cefact:LodgingHouse_Reservation.Details",
                    "rdfs:comment": "The identifier of the cancellation for this lodging house reservation."
                }
            ]
        },
        {
            "@id": "tourism:cancellationPolicy",
            "@type": "rdf:Property",
            "schema:rangeIncludes": {
                "@id": "xsd:string"
            },
            "schema:domainIncludes": {
                "@id": "tourism:LodgingHouseTravelProduct"
            },
            "rdfs:comment": "The cancellation policy, expressed as text, for this lodging house travel product.",
            "rdfs:label": "cancellationPolicy",
            "unece:cefactElementMetadata": [
                {
                    "@id": "cefact:LodgingHouse_TravelProduct.CancellationPolicy.Text",
                    "@type": "unece:BasicBIE",
                    "unece:cefactUNId": "UN01004929",
                    "unece:cefactBieDomainClass": "cefact:LodgingHouse_TravelProduct.Details",
                    "rdfs:comment": "The cancellation policy, expressed as text, for this lodging house travel product."
                }
            ]
        },
        {
            "@id": "tourism:carriedCertificate",
            "@type": "rdf:Property",
            "schema:rangeIncludes": {
                "@id": "tourism:Certificate"
            },
            "schema:domainIncludes": {
                "@id": "tourism:GuestPerson"
            },
            "rdfs:comment": "A certificate carried by this guest person.",
            "rdfs:label": "carriedCertificate",
            "unece:cefactElementMetadata": [
                {
                    "@id": "cefact:Guest_Person.Carried.Specified_Certificate",
                    "@type": "unece:AssociationBIE",
                    "unece:cefactUNId": "UN01015233",
                    "unece:cefactBieDomainClass": "cefact:Guest_Person.Details",
                    "rdfs:comment": "A certificate carried by this guest person."
                }
            ]
        },
        {
            "@id": "tourism:categoryCode",
            "@type": "rdf:Property",
            "schema:rangeIncludes": {
                "@id": "xsd:token"
            },
            "schema:domainIncludes": [
                {
                    "@id": "tourism:CustomerClass"
                },
                {
                    "@id": "tourism:ExperienceProduct"
                },
                {
                    "@id": "tourism:LodgingHouseCustomerClass"
                },
                {
                    "@id": "tourism:LodgingHouseTravelProduct"
                },
                {
                    "@id": "tourism:LodgingHouseTravelProductComponent"
                },
                {
                    "@id": "tourism:LodgingHouseTravelProductSubComponent"
                },
                {
                    "@id": "tourism:LodgingHouseTraveller"
                }
            ],
            "rdfs:comment": [
                "The code specifying the category for this lodging house travel product sub-component.",
                "The code specifying the category of a customer class, such as adult or child.",
                "The code specifying the category of lodging house travel product.",
                "The code specifying the category of this experience product.",
                "The code specifying the category of this lodging house customer class, such as adult or child.",
                "The code specifying the category of this lodging house traveller.",
                "The code specifying the category of this travel product component."
            ],
            "rdfs:label": "categoryCode",
            "unece:cefactElementMetadata": [
                {
                    "@id": "cefact:LodgingHouse_TravelProductComponent.Category.Code",
                    "@type": "unece:BasicBIE",
                    "unece:cefactUNId": "UN01004972",
                    "unece:cefactBieDomainClass": "cefact:LodgingHouse_TravelProductComponent.Details",
                    "rdfs:comment": "The code specifying the category of this travel product component."
                },
                {
                    "@id": "cefact:LodgingHouse_TravelProduct.Category.Code",
                    "@type": "unece:BasicBIE",
                    "unece:cefactUNId": "UN01004918",
                    "unece:cefactBieDomainClass": "cefact:LodgingHouse_TravelProduct.Details",
                    "rdfs:comment": "The code specifying the category of lodging house travel product."
                },
                {
                    "@id": "cefact:LodgingHouse_TravelProductSub-Component.Category.Code",
                    "@type": "unece:BasicBIE",
                    "unece:cefactUNId": "UN01004986",
                    "unece:cefactBieDomainClass": "cefact:LodgingHouse_TravelProductSubComponent.Details",
                    "rdfs:comment": "The code specifying the category for this lodging house travel product sub-component."
                },
                {
                    "@id": "cefact:CustomerClass.Category.Code",
                    "@type": "unece:BasicBIE",
                    "unece:cefactUNId": "UN01004946",
                    "unece:cefactBieDomainClass": "cefact:CustomerClass.Details",
                    "rdfs:comment": "The code specifying the category of a customer class, such as adult or child."
                },
                {
                    "@id": "cefact:Experience_Product.Category.Code",
                    "@type": "unece:BasicBIE",
                    "unece:cefactUNId": "UN01015159",
                    "unece:cefactBieDomainClass": "cefact:Experience_Product.Details",
                    "rdfs:comment": "The code specifying the category of this experience product."
                },
                {
                    "@id": "cefact:LodgingHouse_CustomerClass.Category.Code",
                    "@type": "unece:BasicBIE",
                    "unece:cefactUNId": "UN01010030",
                    "unece:cefactBieDomainClass": "cefact:LodgingHouse_CustomerClass.Details",
                    "rdfs:comment": "The code specifying the category of this lodging house customer class, such as adult or child."
                },
                {
                    "@id": "cefact:LodgingHouse_Traveller.Category.Code",
                    "@type": "unece:BasicBIE",
                    "unece:cefactUNId": "UN01009812",
                    "unece:cefactBieDomainClass": "cefact:LodgingHouse_Traveller.Details",
                    "rdfs:comment": "The code specifying the category of this lodging house traveller."
                }
            ]
        },
        {
            "@id": "tourism:categoryName",
            "@type": "rdf:Property",
            "schema:rangeIncludes": {
                "@id": "xsd:string"
            },
            "schema:domainIncludes": [
                {
                    "@id": "tourism:CustomerClass"
                },
                {
                    "@id": "tourism:LodgingHouseCustomerClass"
                },
                {
                    "@id": "tourism:LodgingHouseTravelProductComponent"
                }
            ],
            "rdfs:comment": [
                "The category name, expressed as text, of a customer class.",
                "The category name, expressed as text, of this lodging house customer class.",
                "The category name, expressed as text, of this lodging house travel product component."
            ],
            "rdfs:label": "categoryName",
            "unece:cefactElementMetadata": [
                {
                    "@id": "cefact:LodgingHouse_CustomerClass.CategoryName.Text",
                    "@type": "unece:BasicBIE",
                    "unece:cefactUNId": "UN01010031",
                    "unece:cefactBieDomainClass": "cefact:LodgingHouse_CustomerClass.Details",
                    "rdfs:comment": "The category name, expressed as text, of this lodging house customer class."
                },
                {
                    "@id": "cefact:CustomerClass.CategoryName.Text",
                    "@type": "unece:BasicBIE",
                    "unece:cefactUNId": "UN01004947",
                    "unece:cefactBieDomainClass": "cefact:CustomerClass.Details",
                    "rdfs:comment": "The category name, expressed as text, of a customer class."
                },
                {
                    "@id": "cefact:LodgingHouse_TravelProductComponent.Category_Name.Text",
                    "@type": "unece:BasicBIE",
                    "unece:cefactUNId": "UN01004973",
                    "unece:cefactBieDomainClass": "cefact:LodgingHouse_TravelProductComponent.Details",
                    "rdfs:comment": "The category name, expressed as text, of this lodging house travel product component."
                }
            ]
        },
        {
            "@id": "tourism:categoryTypeCode",
            "@type": "rdf:Property",
            "schema:rangeIncludes": {
                "@id": "xsd:token"
            },
            "schema:domainIncludes": {
                "@id": "tourism:LodgingHouseTravelProductSubComponent"
            },
            "rdfs:comment": "The code specifying the type of category for this lodging house travel product sub-component.",
            "rdfs:label": "categoryTypeCode",
            "unece:cefactElementMetadata": [
                {
                    "@id": "cefact:LodgingHouse_TravelProductSub-Component.CategoryType.Code",
                    "@type": "unece:BasicBIE",
                    "unece:cefactUNId": "UN01004987",
                    "unece:cefactBieDomainClass": "cefact:LodgingHouse_TravelProductSubComponent.Details",
                    "rdfs:comment": "The code specifying the type of category for this lodging house travel product sub-component."
                }
            ]
        },
        {
            "@id": "tourism:certifiedPersonArrangementIndicator",
            "@type": "rdf:Property",
            "schema:rangeIncludes": {
                "@id": "xsd:boolean"
            },
            "schema:domainIncludes": {
                "@id": "tourism:ExperienceProduct"
            },
            "rdfs:comment": "The indication of whether or not a certified person arrangement is made for this experience product.",
            "rdfs:label": "certifiedPersonArrangementIndicator",
            "unece:cefactElementMetadata": [
                {
                    "@id": "cefact:Experience_Product.CertifiedPerson_Arrangement.Indicator",
                    "@type": "unece:BasicBIE",
                    "unece:cefactUNId": "UN01015168",
                    "unece:cefactBieDomainClass": "cefact:Experience_Product.Details",
                    "rdfs:comment": "The indication of whether or not a certified person arrangement is made for this experience product."
                }
            ]
        },
        {
            "@id": "tourism:chainName",
            "@type": "rdf:Property",
            "schema:rangeIncludes": {
                "@id": "xsd:string"
            },
            "schema:domainIncludes": {
                "@id": "tourism:LodgingHouseOrganization"
            },
            "rdfs:comment": "A name of the chain, expressed as text, to which this lodging house organization belongs.",
            "rdfs:label": "chainName",
            "unece:cefactElementMetadata": [
                {
                    "@id": "cefact:LodgingHouse_Organization.Chain_Name.Text",
                    "@type": "unece:BasicBIE",
                    "unece:cefactUNId": "UN01001029",
                    "unece:cefactBieDomainClass": "cefact:LodgingHouse_Organization.Details",
                    "rdfs:comment": "A name of the chain, expressed as text, to which this lodging house organization belongs."
                }
            ]
        },
        {
            "@id": "tourism:chargeAmount",
            "@type": "rdf:Property",
            "schema:rangeIncludes": {
                "@id": "xsd:decimal"
            },
            "schema:domainIncludes": [
                {
                    "@id": "tourism:BasicPrice"
                },
                {
                    "@id": "tourism:CancellationPrice"
                },
                {
                    "@id": "tourism:DiscountPrice"
                },
                {
                    "@id": "tourism:ExtraPrice"
                }
            ],
            "rdfs:comment": [
                "The monetary value of the basic price charged.",
                "The monetary value of the cancellation price charged.",
                "The monetary value of the discount price charged.",
                "The monetary value of the extra price charged."
            ],
            "rdfs:label": "chargeAmount",
            "unece:cefactElementMetadata": [
                {
                    "@id": "cefact:Cancellation_Price.Charge.Amount",
                    "@type": "unece:BasicBIE",
                    "unece:cefactUNId": "UN01005079",
                    "unece:cefactBieDomainClass": "cefact:Cancellation_Price.Details",
                    "rdfs:comment": "The monetary value of the cancellation price charged."
                },
                {
                    "@id": "cefact:Basic_Price.Charge.Amount",
                    "@type": "unece:BasicBIE",
                    "unece:cefactUNId": "UN01005006",
                    "unece:cefactBieDomainClass": "cefact:Basic_Price.Details",
                    "rdfs:comment": "The monetary value of the basic price charged."
                },
                {
                    "@id": "cefact:Discount_Price.Charge.Amount",
                    "@type": "unece:BasicBIE",
                    "unece:cefactUNId": "UN01005040",
                    "unece:cefactBieDomainClass": "cefact:Discount_Price.Details",
                    "rdfs:comment": "The monetary value of the discount price charged."
                },
                {
                    "@id": "cefact:Extra_Price.Charge.Amount",
                    "@type": "unece:BasicBIE",
                    "unece:cefactUNId": "UN01005021",
                    "unece:cefactBieDomainClass": "cefact:Extra_Price.Details",
                    "rdfs:comment": "The monetary value of the extra price charged."
                }
            ]
        },
        {
            "@id": "tourism:chargeDateTime",
            "@type": "rdf:Property",
            "schema:rangeIncludes": {
                "@id": "xsd:dateTime"
            },
            "schema:domainIncludes": {
                "@id": "tourism:DailyPrice"
            },
            "rdfs:comment": "The date, time, date time, or other date time value when this daily price was or will be charged.",
            "rdfs:label": "chargeDateTime",
            "unece:cefactElementMetadata": [
                {
                    "@id": "cefact:Daily_Price.Charge.DateTime",
                    "@type": "unece:BasicBIE",
                    "unece:TDED": "2379",
                    "unece:cefactUNId": "UN01009688",
                    "unece:cefactBieDomainClass": "cefact:Daily_Price.Details",
                    "rdfs:comment": "The date, time, date time, or other date time value when this daily price was or will be charged."
                }
            ]
        },
        {
            "@id": "tourism:chargedPrice",
            "@type": "rdf:Property",
            "schema:rangeIncludes": {
                "@id": "tourism:Price"
            },
            "schema:domainIncludes": [
                {
                    "@id": "tourism:DailyPrice"
                },
                {
                    "@id": "tourism:LodgingHouseTravelProduct"
                }
            ],
            "rdfs:comment": [
                "A cancellation price charged for this daily price.",
                "A daily price charged for this lodging house travel product.",
                "A discount price charged for this daily price.",
                "An additional price charged for this daily price.",
                "The basic price charged for this daily price.",
                "The service price charged for this daily price."
            ],
            "rdfs:label": "chargedPrice",
            "unece:cefactElementMetadata": [
                {
                    "@id": "cefact:LodgingHouse_TravelProduct.Charged.Daily_Price",
                    "@type": "unece:AssociationBIE",
                    "unece:cefactUNId": "UN01009809",
                    "unece:cefactBieDomainClass": "cefact:LodgingHouse_TravelProduct.Details",
                    "rdfs:comment": "A daily price charged for this lodging house travel product."
                },
                {
                    "@id": "cefact:Daily_Price.Charged.Basic_Price",
                    "@type": "unece:AssociationBIE",
                    "unece:cefactUNId": "UN01009699",
                    "unece:cefactBieDomainClass": "cefact:Daily_Price.Details",
                    "rdfs:comment": "The basic price charged for this daily price."
                },
                {
                    "@id": "cefact:Daily_Price.Charged.Service_Price",
                    "@type": "unece:AssociationBIE",
                    "unece:cefactUNId": "UN01009702",
                    "unece:cefactBieDomainClass": "cefact:Daily_Price.Details",
                    "rdfs:comment": "The service price charged for this daily price."
                },
                {
                    "@id": "cefact:Daily_Price.Charged.Discount_Price",
                    "@type": "unece:AssociationBIE",
                    "unece:cefactUNId": "UN01009701",
                    "unece:cefactBieDomainClass": "cefact:Daily_Price.Details",
                    "rdfs:comment": "A discount price charged for this daily price."
                },
                {
                    "@id": "cefact:Daily_Price.Charged.Cancellation_Price",
                    "@type": "unece:AssociationBIE",
                    "unece:cefactUNId": "UN01009704",
                    "unece:cefactBieDomainClass": "cefact:Daily_Price.Details",
                    "rdfs:comment": "A cancellation price charged for this daily price."
                },
                {
                    "@id": "cefact:Daily_Price.Charged.Extra_Price",
                    "@type": "unece:AssociationBIE",
                    "unece:cefactUNId": "UN01009700",
                    "unece:cefactBieDomainClass": "cefact:Daily_Price.Details",
                    "rdfs:comment": "An additional price charged for this daily price."
                }
            ]
        },
        {
            "@id": "tourism:chargedTax",
            "@type": "rdf:Property",
            "schema:rangeIncludes": {
                "@id": "tourism:Tax"
            },
            "schema:domainIncludes": {
                "@id": "tourism:DailyPrice"
            },
            "rdfs:comment": "A travel product tax charged for this daily price.",
            "rdfs:label": "chargedTax",
            "unece:cefactElementMetadata": [
                {
                    "@id": "cefact:Daily_Price.Charged.TravelProduct_Tax",
                    "@type": "unece:AssociationBIE",
                    "unece:cefactUNId": "UN01009703",
                    "unece:cefactBieDomainClass": "cefact:Daily_Price.Details",
                    "rdfs:comment": "A travel product tax charged for this daily price."
                }
            ]
        },
        {
            "@id": "tourism:choiceAllowedIndicator",
            "@type": "rdf:Property",
            "schema:rangeIncludes": {
                "@id": "xsd:boolean"
            },
            "schema:domainIncludes": [
                {
                    "@id": "tourism:ExperienceEvent"
                },
                {
                    "@id": "tourism:LodgingHouseTravelProductComponent"
                }
            ],
            "rdfs:comment": [
                "The indication of whether or not a choice is allowed for this experience event.",
                "The indication of whether or not a choice is allowed within this lodging house travel product component."
            ],
            "rdfs:label": "choiceAllowedIndicator",
            "unece:cefactElementMetadata": [
                {
                    "@id": "cefact:LodgingHouse_TravelProductComponent.ChoiceAllowed.Indicator",
                    "@type": "unece:BasicBIE",
                    "unece:cefactUNId": "UN01004975",
                    "unece:cefactBieDomainClass": "cefact:LodgingHouse_TravelProductComponent.Details",
                    "rdfs:comment": "The indication of whether or not a choice is allowed within this lodging house travel product component."
                },
                {
                    "@id": "cefact:Experience_Event.Choice_Allowed.Indicator",
                    "@type": "unece:BasicBIE",
                    "unece:cefactUNId": "UN01015120",
                    "unece:cefactBieDomainClass": "cefact:Experience_Event.Details",
                    "rdfs:comment": "The indication of whether or not a choice is allowed for this experience event."
                }
            ]
        },
        {
            "@id": "tourism:claimedLanguageProficiency",
            "@type": "rdf:Property",
            "schema:rangeIncludes": {
                "@id": "tourism:LanguageProficiency"
            },
            "schema:domainIncludes": {
                "@id": "tourism:GuestPerson"
            },
            "rdfs:comment": "Personal language proficiency skills claimed by this guest person.",
            "rdfs:label": "claimedLanguageProficiency",
            "unece:cefactElementMetadata": [
                {
                    "@id": "cefact:Guest_Person.Claimed.Personal_LanguageProficiency",
                    "@type": "unece:AssociationBIE",
                    "unece:cefactUNId": "UN01015234",
                    "unece:cefactBieDomainClass": "cefact:Guest_Person.Details",
                    "rdfs:comment": "Personal language proficiency skills claimed by this guest person."
                }
            ]
        },
        {
            "@id": "tourism:classificationCode",
            "@type": "rdf:Property",
            "schema:rangeIncludes": {
                "@id": "xsd:token"
            },
            "schema:domainIncludes": {
                "@id": "tourism:LodgingHouseParty"
            },
            "rdfs:comment": "The code specifying the classification of this lodging house party.",
            "rdfs:label": "classificationCode",
            "unece:cefactElementMetadata": [
                {
                    "@id": "cefact:LodgingHouse_Party.Classification.Code",
                    "@type": "unece:BasicBIE",
                    "unece:cefactUNId": "UN01001286",
                    "unece:cefactBieDomainClass": "cefact:LodgingHouse_Party.Details",
                    "rdfs:comment": "The code specifying the classification of this lodging house party."
                }
            ]
        },
        {
            "@id": "tourism:commissionChargeAmount",
            "@type": "rdf:Property",
            "schema:rangeIncludes": {
                "@id": "xsd:decimal"
            },
            "schema:domainIncludes": {
                "@id": "tourism:DailyPrice"
            },
            "rdfs:comment": "The monetary value of the commission charged on which this daily price is calculated.",
            "rdfs:label": "commissionChargeAmount",
            "unece:cefactElementMetadata": [
                {
                    "@id": "cefact:Daily_Price.Commission_Charge.Amount",
                    "@type": "unece:BasicBIE",
                    "unece:cefactUNId": "UN01009695",
                    "unece:cefactBieDomainClass": "cefact:Daily_Price.Details",
                    "rdfs:comment": "The monetary value of the commission charged on which this daily price is calculated."
                }
            ]
        },
        {
            "@id": "tourism:commissionPaidIndicator",
            "@type": "rdf:Property",
            "schema:rangeIncludes": {
                "@id": "xsd:boolean"
            },
            "schema:domainIncludes": [
                {
                    "@id": "tourism:BasicPrice"
                },
                {
                    "@id": "tourism:DiscountPrice"
                },
                {
                    "@id": "tourism:ExtraPrice"
                }
            ],
            "rdfs:comment": [
                "The indication of whether or not a commission will be paid for this basic price.",
                "The indication of whether or not a commission will be paid for this discount price.",
                "The indication of whether or not a commission will be paid for this extra price."
            ],
            "rdfs:label": "commissionPaidIndicator",
            "unece:cefactElementMetadata": [
                {
                    "@id": "cefact:Discount_Price.CommissionPaid.Indicator",
                    "@type": "unece:BasicBIE",
                    "unece:cefactUNId": "UN01005045",
                    "unece:cefactBieDomainClass": "cefact:Discount_Price.Details",
                    "rdfs:comment": "The indication of whether or not a commission will be paid for this discount price."
                },
                {
                    "@id": "cefact:Basic_Price.CommissionPaid.Indicator",
                    "@type": "unece:BasicBIE",
                    "unece:cefactUNId": "UN01005010",
                    "unece:cefactBieDomainClass": "cefact:Basic_Price.Details",
                    "rdfs:comment": "The indication of whether or not a commission will be paid for this basic price."
                },
                {
                    "@id": "cefact:Extra_Price.CommissionPaid.Indicator",
                    "@type": "unece:BasicBIE",
                    "unece:cefactUNId": "UN01005026",
                    "unece:cefactBieDomainClass": "cefact:Extra_Price.Details",
                    "rdfs:comment": "The indication of whether or not a commission will be paid for this extra price."
                }
            ]
        },
        {
            "@id": "tourism:completionDateTime",
            "@type": "rdf:Property",
            "schema:rangeIncludes": {
                "@id": "xsd:dateTime"
            },
            "schema:domainIncludes": {
                "@id": "tourism:ExperienceFacility"
            },
            "rdfs:comment": "The date of the completion of this experience facility.",
            "rdfs:label": "completionDateTime",
            "unece:cefactElementMetadata": [
                {
                    "@id": "cefact:Experience_Facility.Completion.DateTime",
                    "@type": "unece:BasicBIE",
                    "unece:cefactUNId": "UN01015143",
                    "unece:cefactBieDomainClass": "cefact:Experience_Facility.Details",
                    "rdfs:comment": "The date of the completion of this experience facility."
                }
            ]
        },
        {
            "@id": "tourism:condition",
            "@type": "rdf:Property",
            "schema:rangeIncludes": {
                "@id": "xsd:string"
            },
            "schema:domainIncludes": {
                "@id": ":FinancialGuarantee"
            },
            "rdfs:comment": "The condition, expressed as text, for this financial guarantee.",
            "rdfs:label": "condition",
            "unece:cefactElementMetadata": [
                {
                    "@id": "cefact:Financial_Guarantee.Condition.Text",
                    "@type": "unece:BasicBIE",
                    "unece:cefactUNId": "UN01009707",
                    "unece:cefactBieDomainClass": "cefact:Financial_Guarantee.Details",
                    "rdfs:comment": "The condition, expressed as text, for this financial guarantee."
                }
            ]
        },
        {
            "@id": "tourism:constructionDate",
            "@type": "rdf:Property",
            "schema:rangeIncludes": {
                "@id": "xsd:base64Binary"
            },
            "schema:domainIncludes": [
                {
                    "@id": "tourism:BathingFacility"
                },
                {
                    "@id": "tourism:BusinessSupportRoomFacility"
                },
                {
                    "@id": "tourism:GuestRoomFacility"
                }
            ],
            "rdfs:comment": [
                "The date of the construction of this bathing facility.",
                "The date of the construction of this business support room.",
                "The date of the construction of this guest room."
            ],
            "rdfs:label": "constructionDate",
            "unece:cefactElementMetadata": [
                {
                    "@id": "cefact:BusinessSupportRoom_Facility.Construction.Date",
                    "@type": "unece:BasicBIE",
                    "unece:cefactUNId": "UN01001110",
                    "unece:cefactBieDomainClass": "cefact:BusinessSupportRoom_Facility.Details",
                    "rdfs:comment": "The date of the construction of this business support room."
                },
                {
                    "@id": "cefact:Bathing_Facility.Construction.Date",
                    "@type": "unece:BasicBIE",
                    "unece:cefactUNId": "UN01001066",
                    "unece:cefactBieDomainClass": "cefact:Bathing_Facility.Details",
                    "rdfs:comment": "The date of the construction of this bathing facility."
                },
                {
                    "@id": "cefact:GuestRoom_Facility.Construction.Date",
                    "@type": "unece:BasicBIE",
                    "unece:cefactUNId": "UN01001052",
                    "unece:cefactBieDomainClass": "cefact:GuestRoom_Facility.Details",
                    "rdfs:comment": "The date of the construction of this guest room."
                }
            ]
        },
        {
            "@id": "tourism:copyrightOwnerName",
            "@type": "rdf:Property",
            "schema:rangeIncludes": {
                "@id": "xsd:string"
            },
            "schema:domainIncludes": {
                "@id": "tourism:LodgingHousePicture"
            },
            "rdfs:comment": "The name of the company or individual person, expressed as text, that owns the copyright for this lodging house picture.",
            "rdfs:label": "copyrightOwnerName",
            "unece:cefactElementMetadata": [
                {
                    "@id": "cefact:LodgingHouse_Picture.CopyrightOwnerName.Text",
                    "@type": "unece:BasicBIE",
                    "unece:cefactUNId": "UN01001244",
                    "unece:cefactBieDomainClass": "cefact:LodgingHouse_Picture.Details",
                    "rdfs:comment": "The name of the company or individual person, expressed as text, that owns the copyright for this lodging house picture."
                }
            ]
        },
        {
            "@id": "tourism:copyrightRegisteredId",
            "@type": "rdf:Property",
            "schema:rangeIncludes": {
                "@id": "xsd:token"
            },
            "schema:domainIncludes": {
                "@id": "tourism:LodgingHousePicture"
            },
            "rdfs:comment": "The unique identifier under which the copyright is registered for this lodging house picture.",
            "rdfs:label": "copyrightRegisteredId",
            "unece:cefactElementMetadata": [
                {
                    "@id": "cefact:LodgingHouse_Picture.CopyrightRegistered_Identification.Identifier",
                    "@type": "unece:BasicBIE",
                    "unece:cefactUNId": "UN01001247",
                    "unece:cefactBieDomainClass": "cefact:LodgingHouse_Picture.Details",
                    "rdfs:comment": "The unique identifier under which the copyright is registered for this lodging house picture."
                }
            ]
        },
        {
            "@id": "tourism:customerServicePointQuantity",
            "@type": "rdf:Property",
            "schema:rangeIncludes": {
                "@id": "xsd:decimal"
            },
            "schema:domainIncludes": {
                "@id": "tourism:DailyPrice"
            },
            "rdfs:comment": "The number of customer service points for this daily price.",
            "rdfs:label": "customerServicePointQuantity",
            "unece:cefactElementMetadata": [
                {
                    "@id": "cefact:Daily_Price.CustomerServicePoint.Quantity",
                    "@type": "unece:BasicBIE",
                    "unece:cefactUNId": "UN01009692",
                    "unece:cefactBieDomainClass": "cefact:Daily_Price.Details",
                    "rdfs:comment": "The number of customer service points for this daily price."
                }
            ]
        },
        {
            "@id": "tourism:dailyPriceTypeCode",
            "@type": "rdf:Property",
            "schema:rangeIncludes": {
                "@id": "unece:UNECECL5375Code"
            },
            "schema:domainIncludes": {
                "@id": "tourism:DailyPrice"
            },
            "rdfs:comment": "The code specifying the type of this daily price, such as tax inclusive, tax and service charge inclusive.",
            "rdfs:label": "dailyPriceTypeCode",
            "unece:cefactElementMetadata": [
                {
                    "@id": "cefact:Daily_Price.Type.Code",
                    "@type": "unece:BasicBIE",
                    "unece:TDED": "5375",
                    "unece:cefactUNId": "UN01009686",
                    "unece:cefactBieDomainClass": "cefact:Daily_Price.Details",
                    "rdfs:comment": "The code specifying the type of this daily price, such as tax inclusive, tax and service charge inclusive."
                }
            ]
        },
        {
            "@id": "tourism:dateSequenceNumeric",
            "@type": "rdf:Property",
            "schema:rangeIncludes": {
                "@id": "xsd:decimal"
            },
            "schema:domainIncludes": {
                "@id": "tourism:ExperienceEvent"
            },
            "rdfs:comment": "The date sequence number for this experience event.",
            "rdfs:label": "dateSequenceNumeric",
            "unece:cefactElementMetadata": [
                {
                    "@id": "cefact:Experience_Event.Date_Sequence.Numeric",
                    "@type": "unece:BasicBIE",
                    "unece:cefactUNId": "UN01015116",
                    "unece:cefactBieDomainClass": "cefact:Experience_Event.Details",
                    "rdfs:comment": "The date sequence number for this experience event."
                }
            ]
        },
        {
            "@id": "tourism:dayNumeric",
            "@type": "rdf:Property",
            "schema:rangeIncludes": {
                "@id": "xsd:decimal"
            },
            "schema:domainIncludes": {
                "@id": "tourism:ProductComponentItinerary"
            },
            "rdfs:comment": "The number of the day in this product component itinerary, such as day 1, day 2, or day 3.",
            "rdfs:label": "dayNumeric",
            "unece:cefactElementMetadata": [
                {
                    "@id": "cefact:ProductComponent_Itinerary.Day.Numeric",
                    "@type": "unece:BasicBIE",
                    "unece:cefactUNId": "UN01004980",
                    "unece:cefactBieDomainClass": "cefact:ProductComponent_Itinerary.Details",
                    "rdfs:comment": "The number of the day in this product component itinerary, such as day 1, day 2, or day 3."
                }
            ]
        },
        {
            "@id": "tourism:definedContact",
            "@type": "rdf:Property",
            "schema:rangeIncludes": {
                "@id": "tourism:Contact"
            },
            "schema:domainIncludes": {
                "@id": "tourism:LodgingHouseParty"
            },
            "rdfs:comment": "The defined contact for this lodging house party.",
            "rdfs:label": "definedContact",
            "unece:cefactElementMetadata": [
                {
                    "@id": "cefact:LodgingHouse_Party.Defined.LodgingHouse_Contact",
                    "@type": "unece:AssociationBIE",
                    "unece:cefactUNId": "UN01001289",
                    "unece:cefactBieDomainClass": "cefact:LodgingHouse_Party.Details",
                    "rdfs:comment": "The defined contact for this lodging house party."
                }
            ]
        },
        {
            "@id": "tourism:definedFeature",
            "@type": "rdf:Property",
            "schema:rangeIncludes": {
                "@id": "tourism:Feature"
            },
            "schema:domainIncludes": {
                "@id": "tourism:LodgingHouseTravelProduct"
            },
            "rdfs:comment": "A feature defined for this lodging house travel product.",
            "rdfs:label": "definedFeature",
            "unece:cefactElementMetadata": [
                {
                    "@id": "cefact:LodgingHouse_TravelProduct.Defined.TravelProduct_Feature",
                    "@type": "unece:AssociationBIE",
                    "unece:cefactUNId": "UN01004935",
                    "unece:cefactBieDomainClass": "cefact:LodgingHouse_TravelProduct.Details",
                    "rdfs:comment": "A feature defined for this lodging house travel product."
                }
            ]
        },
        {
            "@id": "tourism:departmentName",
            "@type": "rdf:Property",
            "schema:rangeIncludes": {
                "@id": "xsd:string"
            },
            "schema:domainIncludes": {
                "@id": "tourism:LodgingHouseContact"
            },
            "rdfs:comment": "The department name, expressed as text, to which this contact belongs within this lodging house.",
            "rdfs:label": "departmentName",
            "unece:cefactElementMetadata": [
                {
                    "@id": "cefact:LodgingHouse_Contact.DepartmentName.Text",
                    "@type": "unece:BasicBIE",
                    "unece:TDED": "3412",
                    "unece:cefactUNId": "UN01001225",
                    "unece:cefactBieDomainClass": "cefact:LodgingHouse_Contact.Details",
                    "rdfs:comment": "The department name, expressed as text, to which this contact belongs within this lodging house."
                }
            ]
        },
        {
            "@id": "tourism:departurePoint",
            "@type": "rdf:Property",
            "schema:rangeIncludes": {
                "@id": "xsd:string"
            },
            "schema:domainIncludes": {
                "@id": "tourism:LodgingHouseRoute"
            },
            "rdfs:comment": "The departure point, expressed as text, for this route to this lodging house.",
            "rdfs:label": "departurePoint",
            "unece:cefactElementMetadata": [
                {
                    "@id": "cefact:LodgingHouse_Route.DeparturePoint.Text",
                    "@type": "unece:BasicBIE",
                    "unece:cefactUNId": "UN01001239",
                    "unece:cefactBieDomainClass": "cefact:LodgingHouse_Route.Details",
                    "rdfs:comment": "The departure point, expressed as text, for this route to this lodging house."
                }
            ]
        },
        {
            "@id": "tourism:description",
            "@type": "rdf:Property",
            "schema:rangeIncludes": {
                "@id": "xsd:string"
            },
            "schema:domainIncludes": [
                {
                    "@id": "tourism:BathingFacility"
                },
                {
                    "@id": "tourism:BusinessSupportRoomFacility"
                },
                {
                    "@id": "tourism:CustomerClass"
                },
                {
                    "@id": "tourism:ExperienceEvent"
                },
                {
                    "@id": "tourism:ExperienceFacility"
                },
                {
                    "@id": "tourism:ExperienceItemPreference"
                },
                {
                    "@id": "tourism:ExperienceItemVoucher"
                },
                {
                    "@id": "tourism:ExperienceProduct"
                },
                {
                    "@id": "tourism:ExperienceProgramAction"
                },
                {
                    "@id": "tourism:GuestAllergy"
                },
                {
                    "@id": "tourism:GuestCarriedEquipment"
                },
                {
                    "@id": "tourism:GuestDisability"
                },
                {
                    "@id": "tourism:GuestFoodChoice"
                },
                {
                    "@id": "tourism:GuestHealthIndication"
                },
                {
                    "@id": "tourism:GuestPerson"
                },
                {
                    "@id": "tourism:GuestRoomFacility"
                },
                {
                    "@id": "tourism:LodgingHouseBuilding"
                },
                {
                    "@id": "tourism:LodgingHouseContact"
                },
                {
                    "@id": "tourism:LodgingHouseCustomerClass"
                },
                {
                    "@id": "tourism:LodgingHouseFeature"
                },
                {
                    "@id": "tourism:LodgingHouseOrganization"
                },
                {
                    "@id": "tourism:LodgingHouseParty"
                },
                {
                    "@id": "tourism:LodgingHousePicture"
                },
                {
                    "@id": "tourism:LodgingHouseReservation"
                },
                {
                    "@id": "tourism:LodgingHouseReservationRestriction"
                },
                {
                    "@id": "tourism:LodgingHouseRoute"
                },
                {
                    "@id": "tourism:LodgingHouseTravelProduct"
                },
                {
                    "@id": "tourism:LodgingHouseTravelProductComponent"
                },
                {
                    "@id": "tourism:LodgingHouseTravelProductSubComponent"
                },
                {
                    "@id": "tourism:LodgingHouseTraveller"
                },
                {
                    "@id": "tourism:LodgingHouseUsageCondition"
                },
                {
                    "@id": "tourism:ReservationRestriction"
                },
                {
                    "@id": "tourism:TravelProductReservationItem"
                }
            ],
            "rdfs:comment": [
                "A textual description of this experience event.",
                "A textual description of this experience facility.",
                "A textual description of this experience item preference.",
                "A textual description of this experience item voucher.",
                "A textual description of this experience product.",
                "A textual description of this experience program action.",
                "A textual description of this guest allergy.",
                "A textual description of this guest carried equipment.",
                "A textual description of this guest disability.",
                "A textual description of this guest food choice.",
                "A textual description of this guest health indication.",
                "A textual description of this lodging house party.",
                "The textual description for this lodging house picture.",
                "The textual description of a customer class.",
                "The textual description of the contact for this lodging house.",
                "The textual description of the lodging house usage condition.",
                "The textual description of the route to this lodging house.",
                "The textual description of this bathing facility.",
                "The textual description of this business support room.",
                "The textual description of this guest room.",
                "The textual description of this guest.",
                "The textual description of this lodging house building.",
                "The textual description of this lodging house customer class.",
                "The textual description of this lodging house feature.",
                "The textual description of this lodging house organization.",
                "The textual description of this lodging house reservation restriction.",
                "The textual description of this lodging house reservation.",
                "The textual description of this lodging house travel product component.",
                "The textual description of this lodging house travel product sub-component.",
                "The textual description of this lodging house travel product.",
                "The textual description of this lodging house traveller.",
                "The textual description of this reservation restriction.",
                "The textual description of this travel product reservation item."
            ],
            "rdfs:label": "description",
            "unece:cefactElementMetadata": [
                {
                    "@id": "cefact:Guest_Allergy.Description.Text",
                    "@type": "unece:BasicBIE",
                    "unece:cefactUNId": "UN01015193",
                    "unece:cefactBieDomainClass": "cefact:Guest_Allergy.Details",
                    "rdfs:comment": "A textual description of this guest allergy."
                },
                {
                    "@id": "cefact:LodgingHouse_TravelProductSub-Component.Description.Text",
                    "@type": "unece:BasicBIE",
                    "unece:cefactUNId": "UN01004993",
                    "unece:cefactBieDomainClass": "cefact:LodgingHouse_TravelProductSubComponent.Details",
                    "rdfs:comment": "The textual description of this lodging house travel product sub-component."
                },
                {
                    "@id": "cefact:CustomerClass.Description.Text",
                    "@type": "unece:BasicBIE",
                    "unece:cefactUNId": "UN01004953",
                    "unece:cefactBieDomainClass": "cefact:CustomerClass.Details",
                    "rdfs:comment": "The textual description of a customer class."
                },
                {
                    "@id": "cefact:ExperienceItem_Preference.Description.Text",
                    "@type": "unece:BasicBIE",
                    "unece:cefactUNId": "UN01015154",
                    "unece:cefactBieDomainClass": "cefact:ExperienceItem_Preference.Details",
                    "rdfs:comment": "A textual description of this experience item preference."
                },
                {
                    "@id": "cefact:Bathing_Facility.Description.Text",
                    "@type": "unece:BasicBIE",
                    "unece:cefactUNId": "UN01001063",
                    "unece:cefactBieDomainClass": "cefact:Bathing_Facility.Details",
                    "rdfs:comment": "The textual description of this bathing facility."
                },
                {
                    "@id": "cefact:LodgingHouse_ReservationRestriction.Description.Text",
                    "@type": "unece:BasicBIE",
                    "unece:cefactUNId": "UN01010050",
                    "unece:cefactBieDomainClass": "cefact:LodgingHouse_ReservationRestriction.Details",
                    "rdfs:comment": "The textual description of this lodging house reservation restriction."
                },
                {
                    "@id": "cefact:LodgingHouse_TravelProduct.Description.Text",
                    "@type": "unece:BasicBIE",
                    "unece:cefactUNId": "UN01004931",
                    "unece:cefactBieDomainClass": "cefact:LodgingHouse_TravelProduct.Details",
                    "rdfs:comment": "The textual description of this lodging house travel product."
                },
                {
                    "@id": "cefact:ExperienceProgram_Action.Description.Text",
                    "@type": "unece:BasicBIE",
                    "unece:cefactUNId": "UN01015187",
                    "unece:cefactBieDomainClass": "cefact:ExperienceProgram_Action.Details",
                    "rdfs:comment": "A textual description of this experience program action."
                },
                {
                    "@id": "cefact:Guest_Disability.Description.Text",
                    "@type": "unece:BasicBIE",
                    "unece:cefactUNId": "UN01015206",
                    "unece:cefactBieDomainClass": "cefact:Guest_Disability.Details",
                    "rdfs:comment": "A textual description of this guest disability."
                },
                {
                    "@id": "cefact:LodgingHouse_Traveller.Description.Text",
                    "@type": "unece:BasicBIE",
                    "unece:cefactUNId": "UN01009816",
                    "unece:cefactBieDomainClass": "cefact:LodgingHouse_Traveller.Details",
                    "rdfs:comment": "The textual description of this lodging house traveller."
                },
                {
                    "@id": "cefact:TravelProduct_ReservationItem.Description.Text",
                    "@type": "unece:BasicBIE",
                    "unece:cefactUNId": "UN01009975",
                    "unece:cefactBieDomainClass": "cefact:TravelProduct_ReservationItem.Details",
                    "rdfs:comment": "The textual description of this travel product reservation item."
                },
                {
                    "@id": "cefact:Guest_FoodChoice.Description.Text",
                    "@type": "unece:BasicBIE",
                    "unece:cefactUNId": "UN01015211",
                    "unece:cefactBieDomainClass": "cefact:Guest_FoodChoice.Details",
                    "rdfs:comment": "A textual description of this guest food choice."
                },
                {
                    "@id": "cefact:Experience_Event.Description.Text",
                    "@type": "unece:BasicBIE",
                    "unece:cefactUNId": "UN01015128",
                    "unece:cefactBieDomainClass": "cefact:Experience_Event.Details",
                    "rdfs:comment": "A textual description of this experience event."
                },
                {
                    "@id": "cefact:LodgingHouse_Organization.Description.Text",
                    "@type": "unece:BasicBIE",
                    "unece:cefactUNId": "UN01001036",
                    "unece:cefactBieDomainClass": "cefact:LodgingHouse_Organization.Details",
                    "rdfs:comment": "The textual description of this lodging house organization."
                },
                {
                    "@id": "cefact:LodgingHouse_Building.Description.Text",
                    "@type": "unece:BasicBIE",
                    "unece:cefactUNId": "UN01001044",
                    "unece:cefactBieDomainClass": "cefact:LodgingHouse_Building.Details",
                    "rdfs:comment": "The textual description of this lodging house building."
                },
                {
                    "@id": "cefact:LodgingHouse_Party.Description.Text",
                    "@type": "unece:BasicBIE",
                    "unece:cefactUNId": "UN01001284",
                    "unece:cefactBieDomainClass": "cefact:LodgingHouse_Party.Details",
                    "rdfs:comment": "A textual description of this lodging house party."
                },
                {
                    "@id": "cefact:LodgingHouse_CustomerClass.Description.Text",
                    "@type": "unece:BasicBIE",
                    "unece:cefactUNId": "UN01010037",
                    "unece:cefactBieDomainClass": "cefact:LodgingHouse_CustomerClass.Details",
                    "rdfs:comment": "The textual description of this lodging house customer class."
                },
                {
                    "@id": "cefact:LodgingHouse_UsageCondition.Description.Text",
                    "@type": "unece:BasicBIE",
                    "unece:cefactUNId": "UN01001203",
                    "unece:cefactBieDomainClass": "cefact:LodgingHouse_UsageCondition.Details",
                    "rdfs:comment": "The textual description of the lodging house usage condition."
                },
                {
                    "@id": "cefact:GuestRoom_Facility.Description.Text",
                    "@type": "unece:BasicBIE",
                    "unece:cefactUNId": "UN01001049",
                    "unece:cefactBieDomainClass": "cefact:GuestRoom_Facility.Details",
                    "rdfs:comment": "The textual description of this guest room."
                },
                {
                    "@id": "cefact:Guest_HealthIndication.Description.Text",
                    "@type": "unece:BasicBIE",
                    "unece:cefactUNId": "UN01015216",
                    "unece:cefactBieDomainClass": "cefact:Guest_HealthIndication.Details",
                    "rdfs:comment": "A textual description of this guest health indication."
                },
                {
                    "@id": "cefact:Guest_CarriedEquipment.Description.Text",
                    "@type": "unece:BasicBIE",
                    "unece:cefactUNId": "UN01015198",
                    "unece:cefactBieDomainClass": "cefact:Guest_CarriedEquipment.Details",
                    "rdfs:comment": "A textual description of this guest carried equipment."
                },
                {
                    "@id": "cefact:LodgingHouse_Feature.Description.Text",
                    "@type": "unece:BasicBIE",
                    "unece:cefactUNId": "UN01001188",
                    "unece:cefactBieDomainClass": "cefact:LodgingHouse_Feature.Details",
                    "rdfs:comment": "The textual description of this lodging house feature."
                },
                {
                    "@id": "cefact:LodgingHouse_Picture.Description.Text",
                    "@type": "unece:BasicBIE",
                    "unece:cefactUNId": "UN01001251",
                    "unece:cefactBieDomainClass": "cefact:LodgingHouse_Picture.Details",
                    "rdfs:comment": "The textual description for this lodging house picture."
                },
                {
                    "@id": "cefact:BusinessSupportRoom_Facility.Description.Text",
                    "@type": "unece:BasicBIE",
                    "unece:cefactUNId": "UN01001107",
                    "unece:cefactBieDomainClass": "cefact:BusinessSupportRoom_Facility.Details",
                    "rdfs:comment": "The textual description of this business support room."
                },
                {
                    "@id": "cefact:ReservationRestriction.Description.Text",
                    "@type": "unece:BasicBIE",
                    "unece:cefactUNId": "UN01004958",
                    "unece:cefactBieDomainClass": "cefact:ReservationRestriction.Details",
                    "rdfs:comment": "The textual description of this reservation restriction."
                },
                {
                    "@id": "cefact:ExperienceItem_Voucher.Description.Text",
                    "@type": "unece:BasicBIE",
                    "unece:cefactUNId": "UN01015247",
                    "unece:cefactBieDomainClass": "cefact:ExperienceItem_Voucher.Details",
                    "rdfs:comment": "A textual description of this experience item voucher."
                },
                {
                    "@id": "cefact:LodgingHouse_Reservation.Description.Text",
                    "@type": "unece:BasicBIE",
                    "unece:cefactUNId": "UN01009800",
                    "unece:cefactBieDomainClass": "cefact:LodgingHouse_Reservation.Details",
                    "rdfs:comment": "The textual description of this lodging house reservation."
                },
                {
                    "@id": "cefact:Guest_Person.Description.Text",
                    "@type": "unece:BasicBIE",
                    "unece:cefactUNId": "UN01009715",
                    "unece:cefactBieDomainClass": "cefact:Guest_Person.Details",
                    "rdfs:comment": "The textual description of this guest."
                },
                {
                    "@id": "cefact:Experience_Facility.Description.Text",
                    "@type": "unece:BasicBIE",
                    "unece:cefactUNId": "UN01015145",
                    "unece:cefactBieDomainClass": "cefact:Experience_Facility.Details",
                    "rdfs:comment": "A textual description of this experience facility."
                },
                {
                    "@id": "cefact:LodgingHouse_Contact.Description.Text",
                    "@type": "unece:BasicBIE",
                    "unece:cefactUNId": "UN01001229",
                    "unece:cefactBieDomainClass": "cefact:LodgingHouse_Contact.Details",
                    "rdfs:comment": "The textual description of the contact for this lodging house."
                },
                {
                    "@id": "cefact:LodgingHouse_TravelProductComponent.Description.Text",
                    "@type": "unece:BasicBIE",
                    "unece:cefactUNId": "UN01004977",
                    "unece:cefactBieDomainClass": "cefact:LodgingHouse_TravelProductComponent.Details",
                    "rdfs:comment": "The textual description of this lodging house travel product component."
                },
                {
                    "@id": "cefact:LodgingHouse_Route.Description.Text",
                    "@type": "unece:BasicBIE",
                    "unece:cefactUNId": "UN01001237",
                    "unece:cefactBieDomainClass": "cefact:LodgingHouse_Route.Details",
                    "rdfs:comment": "The textual description of the route to this lodging house."
                },
                {
                    "@id": "cefact:Experience_Product.Description.Text",
                    "@type": "unece:BasicBIE",
                    "unece:cefactUNId": "UN01015167",
                    "unece:cefactBieDomainClass": "cefact:Experience_Product.Details",
                    "rdfs:comment": "A textual description of this experience product."
                }
            ]
        },
        {
            "@id": "tourism:determinationCode",
            "@type": "rdf:Property",
            "schema:rangeIncludes": {
                "@id": "xsd:token"
            },
            "schema:domainIncludes": {
                "@id": "tourism:CancellationPrice"
            },
            "rdfs:comment": "The code specifying how the cancellation price is determined.",
            "rdfs:label": "determinationCode",
            "unece:cefactElementMetadata": [
                {
                    "@id": "cefact:Cancellation_Price.Determination.Code",
                    "@type": "unece:BasicBIE",
                    "unece:cefactUNId": "UN01005076",
                    "unece:cefactBieDomainClass": "cefact:Cancellation_Price.Details",
                    "rdfs:comment": "The code specifying how the cancellation price is determined."
                }
            ]
        },
        {
            "@id": "tourism:digitalImageBinaryObject",
            "@type": "rdf:Property",
            "schema:rangeIncludes": {
                "@id": "xsd:base64Binary"
            },
            "schema:domainIncludes": {
                "@id": "tourism:LodgingHousePicture"
            },
            "rdfs:comment": "The binary object data that is a digital image for this lodging house picture.",
            "rdfs:label": "digitalImageBinaryObject",
            "unece:cefactElementMetadata": [
                {
                    "@id": "cefact:LodgingHouse_Picture.DigitalImage.BinaryObject",
                    "@type": "unece:BasicBIE",
                    "unece:cefactUNId": "UN01001248",
                    "unece:cefactBieDomainClass": "cefact:LodgingHouse_Picture.Details",
                    "rdfs:comment": "The binary object data that is a digital image for this lodging house picture."
                }
            ]
        },
        {
            "@id": "tourism:directions",
            "@type": "rdf:Property",
            "schema:rangeIncludes": {
                "@id": "xsd:string"
            },
            "schema:domainIncludes": {
                "@id": "tourism:LodgingHouseLocation"
            },
            "rdfs:comment": "A textual description of how to reach this lodging house location.",
            "rdfs:label": "directions",
            "unece:cefactElementMetadata": [
                {
                    "@id": "cefact:LodgingHouse_Location.Directions.Text",
                    "@type": "unece:BasicBIE",
                    "unece:cefactUNId": "UN01001220",
                    "unece:cefactBieDomainClass": "cefact:LodgingHouse_Location.Details",
                    "rdfs:comment": "A textual description of how to reach this lodging house location."
                }
            ]
        },
        {
            "@id": "tourism:discountChargeAmount",
            "@type": "rdf:Property",
            "schema:rangeIncludes": {
                "@id": "xsd:decimal"
            },
            "schema:domainIncludes": {
                "@id": "tourism:DailyPrice"
            },
            "rdfs:comment": "The monetary value of the discount price charged on which this daily price is calculated.",
            "rdfs:label": "discountChargeAmount",
            "unece:cefactElementMetadata": [
                {
                    "@id": "cefact:Daily_Price.Discount_Charge.Amount",
                    "@type": "unece:BasicBIE",
                    "unece:cefactUNId": "UN01009691",
                    "unece:cefactBieDomainClass": "cefact:Daily_Price.Details",
                    "rdfs:comment": "The monetary value of the discount price charged on which this daily price is calculated."
                }
            ]
        },
        {
            "@id": "tourism:discountPriceTypeCode",
            "@type": "rdf:Property",
            "schema:rangeIncludes": {
                "@id": "unece:UNECECL5375Code"
            },
            "schema:domainIncludes": {
                "@id": "tourism:DiscountPrice"
            },
            "rdfs:comment": "The code specifying the type of discount price.",
            "rdfs:label": "discountPriceTypeCode",
            "unece:cefactElementMetadata": [
                {
                    "@id": "cefact:Discount_Price.Type.Code",
                    "@type": "unece:BasicBIE",
                    "unece:TDED": "5375",
                    "unece:cefactUNId": "UN01005035",
                    "unece:cefactBieDomainClass": "cefact:Discount_Price.Details",
                    "rdfs:comment": "The code specifying the type of discount price."
                }
            ]
        },
        {
            "@id": "tourism:dislikedItem",
            "@type": "rdf:Property",
            "schema:rangeIncludes": {
                "@id": "xsd:string"
            },
            "schema:domainIncludes": {
                "@id": "tourism:ExperienceItemPreference"
            },
            "rdfs:comment": "A disliked item, expressed as text, for this experience item preference.",
            "rdfs:label": "dislikedItem",
            "unece:cefactElementMetadata": [
                {
                    "@id": "cefact:ExperienceItem_Preference.Disliked_Item.Text",
                    "@type": "unece:BasicBIE",
                    "unece:cefactUNId": "UN01015152",
                    "unece:cefactBieDomainClass": "cefact:ExperienceItem_Preference.Details",
                    "rdfs:comment": "A disliked item, expressed as text, for this experience item preference."
                }
            ]
        },
        {
            "@id": "tourism:distinctiveFeature",
            "@type": "rdf:Property",
            "schema:rangeIncludes": {
                "@id": "tourism:Feature"
            },
            "schema:domainIncludes": [
                {
                    "@id": "tourism:BathingFacility"
                },
                {
                    "@id": "tourism:BusinessSupportRoomFacility"
                },
                {
                    "@id": "tourism:ExperienceEvent"
                },
                {
                    "@id": "tourism:ExperienceProduct"
                },
                {
                    "@id": "tourism:GuestRoomFacility"
                },
                {
                    "@id": "tourism:LodgingHouseBuilding"
                },
                {
                    "@id": "tourism:LodgingHouseTravelProductSubComponent"
                }
            ],
            "rdfs:comment": [
                "A distinctive feature of this experience product.",
                "A distinctive feature specified for this experience event.",
                "A distinctive lodging house travel product feature for this travel product sub-component.",
                "A feature that is a distinctive characteristic of this bathing facility at this lodging house.",
                "A feature that is a distinctive characteristic of this business support room at this lodging house.",
                "A feature that is a distinctive characteristic of this guest room at this lodging house.",
                "A feature that is a distinctive characteristic of this lodging house building."
            ],
            "rdfs:label": "distinctiveFeature",
            "unece:cefactElementMetadata": [
                {
                    "@id": "cefact:Experience_Product.Distinctive.Specified_Feature",
                    "@type": "unece:AssociationBIE",
                    "unece:cefactUNId": "UN01015177",
                    "unece:cefactBieDomainClass": "cefact:Experience_Product.Details",
                    "rdfs:comment": "A distinctive feature of this experience product."
                },
                {
                    "@id": "cefact:LodgingHouse_TravelProductSub-Component.Distinctive.TravelProduct_Feature",
                    "@type": "unece:AssociationBIE",
                    "unece:cefactUNId": "UN01004994",
                    "unece:cefactBieDomainClass": "cefact:LodgingHouse_TravelProductSubComponent.Details",
                    "rdfs:comment": "A distinctive lodging house travel product feature for this travel product sub-component."
                },
                {
                    "@id": "cefact:BusinessSupportRoom_Facility.Distinctive.LodgingHouse_Feature",
                    "@type": "unece:AssociationBIE",
                    "unece:cefactUNId": "UN01001116",
                    "unece:cefactBieDomainClass": "cefact:BusinessSupportRoom_Facility.Details",
                    "rdfs:comment": "A feature that is a distinctive characteristic of this business support room at this lodging house."
                },
                {
                    "@id": "cefact:LodgingHouse_Building.Distinctive.LodgingHouse_Feature",
                    "@type": "unece:AssociationBIE",
                    "unece:cefactUNId": "UN01001046",
                    "unece:cefactBieDomainClass": "cefact:LodgingHouse_Building.Details",
                    "rdfs:comment": "A feature that is a distinctive characteristic of this lodging house building."
                },
                {
                    "@id": "cefact:GuestRoom_Facility.Distinctive.LodgingHouse_Feature",
                    "@type": "unece:AssociationBIE",
                    "unece:cefactUNId": "UN01001059",
                    "unece:cefactBieDomainClass": "cefact:GuestRoom_Facility.Details",
                    "rdfs:comment": "A feature that is a distinctive characteristic of this guest room at this lodging house."
                },
                {
                    "@id": "cefact:Bathing_Facility.Distinctive.LodgingHouse_Feature",
                    "@type": "unece:AssociationBIE",
                    "unece:cefactUNId": "UN01001074",
                    "unece:cefactBieDomainClass": "cefact:Bathing_Facility.Details",
                    "rdfs:comment": "A feature that is a distinctive characteristic of this bathing facility at this lodging house."
                },
                {
                    "@id": "cefact:Experience_Event.Distinctive.Specified_Feature",
                    "@type": "unece:AssociationBIE",
                    "unece:cefactUNId": "UN01015132",
                    "unece:cefactBieDomainClass": "cefact:Experience_Event.Details",
                    "rdfs:comment": "A distinctive feature specified for this experience event."
                }
            ]
        },
        {
            "@id": "tourism:effectivePeriod",
            "@type": "rdf:Property",
            "schema:rangeIncludes": {
                "@id": "tourism:Period"
            },
            "schema:domainIncludes": {
                "@id": "tourism:LodgingHouseContract"
            },
            "rdfs:comment": "The specified period for which this lodging house contract is effective.",
            "rdfs:label": "effectivePeriod",
            "unece:cefactElementMetadata": [
                {
                    "@id": "cefact:LodgingHouse_Contract.Effective.Specified_Period",
                    "@type": "unece:AssociationBIE",
                    "unece:cefactUNId": "UN01001215",
                    "unece:cefactBieDomainClass": "cefact:LodgingHouse_Contract.Details",
                    "rdfs:comment": "The specified period for which this lodging house contract is effective."
                }
            ]
        },
        {
            "@id": "tourism:endDateTime",
            "@type": "rdf:Property",
            "schema:rangeIncludes": {
                "@id": "xsd:dateTime"
            },
            "schema:domainIncludes": {
                "@id": ":AvailablePeriod"
            },
            "rdfs:comment": "The date, time, date time or other date time value for the end of this available period of time.",
            "rdfs:label": "endDateTime",
            "unece:cefactElementMetadata": [
                {
                    "@id": "cefact:Available_Period.End.DateTime",
                    "@type": "unece:BasicBIE",
                    "unece:cefactUNId": "UN01005110",
                    "unece:cefactBieDomainClass": "cefact:Available_Period.Details",
                    "rdfs:comment": "The date, time, date time or other date time value for the end of this available period of time."
                }
            ]
        },
        {
            "@id": "tourism:experienceFacilityTypeCode",
            "@type": "rdf:Property",
            "schema:rangeIncludes": {
                "@id": "unece:UNECECL9039Code"
            },
            "schema:domainIncludes": {
                "@id": "tourism:ExperienceFacility"
            },
            "rdfs:comment": "The code specifying the type of experience facility.",
            "rdfs:label": "experienceFacilityTypeCode",
            "unece:cefactElementMetadata": [
                {
                    "@id": "cefact:Experience_Facility.Type.Code",
                    "@type": "unece:BasicBIE",
                    "unece:TDED": "9039",
                    "unece:cefactUNId": "UN01015140",
                    "unece:cefactBieDomainClass": "cefact:Experience_Facility.Details",
                    "rdfs:comment": "The code specifying the type of experience facility."
                }
            ]
        },
        {
            "@id": "tourism:extraChargeAmount",
            "@type": "rdf:Property",
            "schema:rangeIncludes": {
                "@id": "xsd:decimal"
            },
            "schema:domainIncludes": {
                "@id": "tourism:DailyPrice"
            },
            "rdfs:comment": "The monetary value of the additional price charged on which this daily price is calculated.",
            "rdfs:label": "extraChargeAmount",
            "unece:cefactElementMetadata": [
                {
                    "@id": "cefact:Daily_Price.Extra_Charge.Amount",
                    "@type": "unece:BasicBIE",
                    "unece:cefactUNId": "UN01009690",
                    "unece:cefactBieDomainClass": "cefact:Daily_Price.Details",
                    "rdfs:comment": "The monetary value of the additional price charged on which this daily price is calculated."
                }
            ]
        },
        {
            "@id": "tourism:extraPriceTypeCode",
            "@type": "rdf:Property",
            "schema:rangeIncludes": {
                "@id": "unece:UNECECL5375Code"
            },
            "schema:domainIncludes": {
                "@id": "tourism:ExtraPrice"
            },
            "rdfs:comment": "The code specifying the type of extra price.",
            "rdfs:label": "extraPriceTypeCode",
            "unece:cefactElementMetadata": [
                {
                    "@id": "cefact:Extra_Price.Type.Code",
                    "@type": "unece:BasicBIE",
                    "unece:TDED": "5375",
                    "unece:cefactUNId": "UN01005016",
                    "unece:cefactBieDomainClass": "cefact:Extra_Price.Details",
                    "rdfs:comment": "The code specifying the type of extra price."
                }
            ]
        },
        {
            "@id": "tourism:faceAmount",
            "@type": "rdf:Property",
            "schema:rangeIncludes": {
                "@id": "xsd:decimal"
            },
            "schema:domainIncludes": {
                "@id": "tourism:ExperienceItemVoucher"
            },
            "rdfs:comment": "A monetary value shown on the face of this experience item voucher.",
            "rdfs:label": "faceAmount",
            "unece:cefactElementMetadata": [
                {
                    "@id": "cefact:ExperienceItem_Voucher.Face.Amount",
                    "@type": "unece:BasicBIE",
                    "unece:cefactUNId": "UN01015242",
                    "unece:cefactBieDomainClass": "cefact:ExperienceItem_Voucher.Details",
                    "rdfs:comment": "A monetary value shown on the face of this experience item voucher."
                }
            ]
        },
        {
            "@id": "tourism:familiarName",
            "@type": "rdf:Property",
            "schema:rangeIncludes": {
                "@id": "xsd:string"
            },
            "schema:domainIncludes": {
                "@id": "tourism:LodgingHouseBuilding"
            },
            "rdfs:comment": "The familiar name such as a nickname, expressed as text, of the lodging house building.",
            "rdfs:label": "familiarName",
            "unece:cefactElementMetadata": [
                {
                    "@id": "cefact:LodgingHouse_Building.Familiar_Name.Text",
                    "@type": "unece:BasicBIE",
                    "unece:cefactUNId": "UN01001040",
                    "unece:cefactBieDomainClass": "cefact:LodgingHouse_Building.Details",
                    "rdfs:comment": "The familiar name such as a nickname, expressed as text, of the lodging house building."
                }
            ]
        },
        {
            "@id": "tourism:formalName",
            "@type": "rdf:Property",
            "schema:rangeIncludes": {
                "@id": "xsd:string"
            },
            "schema:domainIncludes": {
                "@id": "tourism:LodgingHouseBuilding"
            },
            "rdfs:comment": "A formal name, expressed as text, of this lodging house building.",
            "rdfs:label": "formalName",
            "unece:cefactElementMetadata": [
                {
                    "@id": "cefact:LodgingHouse_Building.Formal_Name.Text",
                    "@type": "unece:BasicBIE",
                    "unece:cefactUNId": "UN01001039",
                    "unece:cefactBieDomainClass": "cefact:LodgingHouse_Building.Details",
                    "rdfs:comment": "A formal name, expressed as text, of this lodging house building."
                }
            ]
        },
        {
            "@id": "tourism:genderCode",
            "@type": "rdf:Property",
            "schema:rangeIncludes": {
                "@id": "xsd:token"
            },
            "schema:domainIncludes": [
                {
                    "@id": "tourism:CustomerClass"
                },
                {
                    "@id": "tourism:GuestPerson"
                },
                {
                    "@id": "tourism:LodgingHouseCustomerClass"
                }
            ],
            "rdfs:comment": [
                "The code specifying the gender in a customer class.",
                "The code specifying the gender in this lodging house customer class.",
                "The code specifying the gender of this guest, such as male, female."
            ],
            "rdfs:label": "genderCode",
            "unece:cefactElementMetadata": [
                {
                    "@id": "cefact:Guest_Person.Gender.Code",
                    "@type": "unece:BasicBIE",
                    "unece:TDED": "3499",
                    "unece:cefactUNId": "UN01009712",
                    "unece:cefactBieDomainClass": "cefact:Guest_Person.Details",
                    "rdfs:comment": "The code specifying the gender of this guest, such as male, female."
                },
                {
                    "@id": "cefact:LodgingHouse_CustomerClass.Gender.Code",
                    "@type": "unece:BasicBIE",
                    "unece:cefactUNId": "UN01010034",
                    "unece:cefactBieDomainClass": "cefact:LodgingHouse_CustomerClass.Details",
                    "rdfs:comment": "The code specifying the gender in this lodging house customer class."
                },
                {
                    "@id": "cefact:CustomerClass.Gender.Code",
                    "@type": "unece:BasicBIE",
                    "unece:cefactUNId": "UN01004950",
                    "unece:cefactBieDomainClass": "cefact:CustomerClass.Details",
                    "rdfs:comment": "The code specifying the gender in a customer class."
                }
            ]
        },
        {
            "@id": "tourism:genderLimitation",
            "@type": "rdf:Property",
            "schema:rangeIncludes": {
                "@id": "xsd:string"
            },
            "schema:domainIncludes": {
                "@id": "tourism:LodgingHouseUsageCondition"
            },
            "rdfs:comment": "The gender limitation, expressed as text, applicable to this lodging house usage condition.",
            "rdfs:label": "genderLimitation",
            "unece:cefactElementMetadata": [
                {
                    "@id": "cefact:LodgingHouse_UsageCondition.GenderLimitation.Text",
                    "@type": "unece:BasicBIE",
                    "unece:cefactUNId": "UN01001205",
                    "unece:cefactBieDomainClass": "cefact:LodgingHouse_UsageCondition.Details",
                    "rdfs:comment": "The gender limitation, expressed as text, applicable to this lodging house usage condition."
                }
            ]
        },
        {
            "@id": "tourism:groupAllowedDuration",
            "@type": "rdf:Property",
            "schema:rangeIncludes": {
                "@id": "xsd:string"
            },
            "schema:domainIncludes": {
                "@id": "tourism:LodgingHouseUsageCondition"
            },
            "rdfs:comment": "The duration, expressed as text, allowed for a group, applicable to this lodging house usage condition.",
            "rdfs:label": "groupAllowedDuration",
            "unece:cefactElementMetadata": [
                {
                    "@id": "cefact:LodgingHouse_UsageCondition.GroupAllowed_Duration.Text",
                    "@type": "unece:BasicBIE",
                    "unece:cefactUNId": "UN01001204",
                    "unece:cefactBieDomainClass": "cefact:LodgingHouse_UsageCondition.Details",
                    "rdfs:comment": "The duration, expressed as text, allowed for a group, applicable to this lodging house usage condition."
                }
            ]
        },
        {
            "@id": "tourism:groupApplicableIndicator",
            "@type": "rdf:Property",
            "schema:rangeIncludes": {
                "@id": "xsd:boolean"
            },
            "schema:domainIncludes": {
                "@id": "tourism:LodgingHouseUsageCondition"
            },
            "rdfs:comment": "The indication of whether or not this lodging house usage condition applies to a group.",
            "rdfs:label": "groupApplicableIndicator",
            "unece:cefactElementMetadata": [
                {
                    "@id": "cefact:LodgingHouse_UsageCondition.Group_Applicable.Indicator",
                    "@type": "unece:BasicBIE",
                    "unece:cefactUNId": "UN01001201",
                    "unece:cefactBieDomainClass": "cefact:LodgingHouse_UsageCondition.Details",
                    "rdfs:comment": "The indication of whether or not this lodging house usage condition applies to a group."
                }
            ]
        },
        {
            "@id": "tourism:heldMembership",
            "@type": "rdf:Property",
            "schema:rangeIncludes": {
                "@id": "tourism:Membership"
            },
            "schema:domainIncludes": {
                "@id": "tourism:GuestPerson"
            },
            "rdfs:comment": "A travel related membership held by this guest.",
            "rdfs:label": "heldMembership",
            "unece:cefactElementMetadata": [
                {
                    "@id": "cefact:Guest_Person.Held.Travel_Membership",
                    "@type": "unece:AssociationBIE",
                    "unece:cefactUNId": "UN01009720",
                    "unece:cefactBieDomainClass": "cefact:Guest_Person.Details",
                    "rdfs:comment": "A travel related membership held by this guest."
                }
            ]
        },
        {
            "@id": "tourism:heldReservationItem",
            "@type": "rdf:Property",
            "schema:rangeIncludes": {
                "@id": "tourism:ReservationItem"
            },
            "schema:domainIncludes": {
                "@id": "tourism:LodgingHouseTravelProduct"
            },
            "rdfs:comment": "The reservation item held for this lodging house travel product.",
            "rdfs:label": "heldReservationItem",
            "unece:cefactElementMetadata": [
                {
                    "@id": "cefact:LodgingHouse_TravelProduct.Held.TravelProduct_ReservationItem",
                    "@type": "unece:AssociationBIE",
                    "unece:cefactUNId": "UN01009806",
                    "unece:cefactBieDomainClass": "cefact:LodgingHouse_TravelProduct.Details",
                    "rdfs:comment": "The reservation item held for this lodging house travel product."
                }
            ]
        },
        {
            "@id": "tourism:id",
            "@type": "rdf:Property",
            "schema:rangeIncludes": {
                "@id": "xsd:token"
            },
            "schema:domainIncludes": [
                {
                    "@id": "tourism:BathingFacility"
                },
                {
                    "@id": "tourism:BusinessSupportRoomFacility"
                },
                {
                    "@id": "tourism:ExperienceEvent"
                },
                {
                    "@id": "tourism:ExperienceFacility"
                },
                {
                    "@id": "tourism:ExperienceItemVoucher"
                },
                {
                    "@id": "tourism:ExperienceProduct"
                },
                {
                    "@id": "tourism:GuestPerson"
                },
                {
                    "@id": "tourism:GuestRoomFacility"
                },
                {
                    "@id": "tourism:LodgingHouseBuilding"
                },
                {
                    "@id": "tourism:LodgingHouseContact"
                },
                {
                    "@id": "tourism:LodgingHouseContract"
                },
                {
                    "@id": "tourism:LodgingHouseFeature"
                },
                {
                    "@id": "tourism:LodgingHouseLocation"
                },
                {
                    "@id": "tourism:LodgingHouseOrganization"
                },
                {
                    "@id": "tourism:LodgingHouseParty"
                },
                {
                    "@id": "tourism:LodgingHousePicture"
                },
                {
                    "@id": "tourism:LodgingHouseReservation"
                },
                {
                    "@id": "tourism:LodgingHouseRoute"
                },
                {
                    "@id": "tourism:LodgingHouseTravelProduct"
                },
                {
                    "@id": "tourism:LodgingHouseTravelProductComponent"
                },
                {
                    "@id": "tourism:LodgingHouseTravelProductSubComponent"
                },
                {
                    "@id": "tourism:LodgingHouseUsageCondition"
                }
            ],
            "rdfs:comment": [
                "A unique identifier for this lodging house building.",
                "A unique identifier for this lodging house organization.",
                "The identifier for this experience item voucher.",
                "The identifier for this guest.",
                "The identifier for this lodging house reservation, such as assigned by a central reservation office.",
                "The identifier of this experience event.",
                "The identifier of this experience facility.",
                "The identifier of this experience product.",
                "The unique identifier for the route to this lodging house.",
                "The unique identifier for this bathing facility.",
                "The unique identifier for this business support room.",
                "The unique identifier for this guest room.",
                "The unique identifier for this lodging house contact.",
                "The unique identifier for this lodging house contract.",
                "The unique identifier for this lodging house feature.",
                "The unique identifier for this lodging house location.",
                "The unique identifier for this lodging house party.",
                "The unique identifier for this lodging house picture.",
                "The unique identifier for this lodging house travel product component.",
                "The unique identifier for this lodging house travel product sub-component.",
                "The unique identifier for this lodging house travel product.",
                "The unique identifier for this lodging house usage condition."
            ],
            "rdfs:label": "id",
            "unece:cefactElementMetadata": [
                {
                    "@id": "cefact:ExperienceItem_Voucher.Identification.Identifier",
                    "@type": "unece:BasicBIE",
                    "unece:cefactUNId": "UN01015244",
                    "unece:cefactBieDomainClass": "cefact:ExperienceItem_Voucher.Details",
                    "rdfs:comment": "The identifier for this experience item voucher."
                },
                {
                    "@id": "cefact:GuestRoom_Facility.Identification.Identifier",
                    "@type": "unece:BasicBIE",
                    "unece:cefactUNId": "UN01001048",
                    "unece:cefactBieDomainClass": "cefact:GuestRoom_Facility.Details",
                    "rdfs:comment": "The unique identifier for this guest room."
                },
                {
                    "@id": "cefact:LodgingHouse_TravelProductComponent.Identification.Identifier",
                    "@type": "unece:BasicBIE",
                    "unece:cefactUNId": "UN01004974",
                    "unece:cefactBieDomainClass": "cefact:LodgingHouse_TravelProductComponent.Details",
                    "rdfs:comment": "The unique identifier for this lodging house travel product component."
                },
                {
                    "@id": "cefact:LodgingHouse_Reservation.Identification.Identifier",
                    "@type": "unece:BasicBIE",
                    "unece:TDED": "9040",
                    "unece:cefactUNId": "UN01009791",
                    "unece:cefactBieDomainClass": "cefact:LodgingHouse_Reservation.Details",
                    "rdfs:comment": "The identifier for this lodging house reservation, such as assigned by a central reservation office."
                },
                {
                    "@id": "cefact:LodgingHouse_Feature.Identification.Identifier",
                    "@type": "unece:BasicBIE",
                    "unece:cefactUNId": "UN01001184",
                    "unece:cefactBieDomainClass": "cefact:LodgingHouse_Feature.Details",
                    "rdfs:comment": "The unique identifier for this lodging house feature."
                },
                {
                    "@id": "cefact:Experience_Product.Identification.Identifier",
                    "@type": "unece:BasicBIE",
                    "unece:TDED": "7135",
                    "unece:cefactUNId": "UN01015156",
                    "unece:cefactBieDomainClass": "cefact:Experience_Product.Details",
                    "rdfs:comment": "The identifier of this experience product."
                },
                {
                    "@id": "cefact:LodgingHouse_Location.Identification.Identifier",
                    "@type": "unece:BasicBIE",
                    "unece:TDED": "3225",
                    "unece:cefactUNId": "UN01001218",
                    "unece:cefactBieDomainClass": "cefact:LodgingHouse_Location.Details",
                    "rdfs:comment": "The unique identifier for this lodging house location."
                },
                {
                    "@id": "cefact:LodgingHouse_Party.Identification.Identifier",
                    "@type": "unece:BasicBIE",
                    "unece:TDED": "3039",
                    "unece:cefactUNId": "UN01001281",
                    "unece:cefactBieDomainClass": "cefact:LodgingHouse_Party.Details",
                    "rdfs:comment": "The unique identifier for this lodging house party."
                },
                {
                    "@id": "cefact:Guest_Person.Identification.Identifier",
                    "@type": "unece:BasicBIE",
                    "unece:cefactUNId": "UN01009709",
                    "unece:cefactBieDomainClass": "cefact:Guest_Person.Details",
                    "rdfs:comment": "The identifier for this guest."
                },
                {
                    "@id": "cefact:BusinessSupportRoom_Facility.Identification.Identifier",
                    "@type": "unece:BasicBIE",
                    "unece:cefactUNId": "UN01001106",
                    "unece:cefactBieDomainClass": "cefact:BusinessSupportRoom_Facility.Details",
                    "rdfs:comment": "The unique identifier for this business support room."
                },
                {
                    "@id": "cefact:Experience_Event.Identification.Identifier",
                    "@type": "unece:BasicBIE",
                    "unece:TDED": "1007",
                    "unece:cefactUNId": "UN01015119",
                    "unece:cefactBieDomainClass": "cefact:Experience_Event.Details",
                    "rdfs:comment": "The identifier of this experience event."
                },
                {
                    "@id": "cefact:LodgingHouse_TravelProductSub-Component.Identification.Identifier",
                    "@type": "unece:BasicBIE",
                    "unece:cefactUNId": "UN01004988",
                    "unece:cefactBieDomainClass": "cefact:LodgingHouse_TravelProductSubComponent.Details",
                    "rdfs:comment": "The unique identifier for this lodging house travel product sub-component."
                },
                {
                    "@id": "cefact:Experience_Facility.Identification.Identifier",
                    "@type": "unece:BasicBIE",
                    "unece:cefactUNId": "UN01015139",
                    "unece:cefactBieDomainClass": "cefact:Experience_Facility.Details",
                    "rdfs:comment": "The identifier of this experience facility."
                },
                {
                    "@id": "cefact:LodgingHouse_Organization.Identification.Identifier",
                    "@type": "unece:BasicBIE",
                    "unece:cefactUNId": "UN01001028",
                    "unece:cefactBieDomainClass": "cefact:LodgingHouse_Organization.Details",
                    "rdfs:comment": "A unique identifier for this lodging house organization."
                },
                {
                    "@id": "cefact:LodgingHouse_Contact.Identification.Identifier",
                    "@type": "unece:BasicBIE",
                    "unece:TDED": "3413",
                    "unece:cefactUNId": "UN01001222",
                    "unece:cefactBieDomainClass": "cefact:LodgingHouse_Contact.Details",
                    "rdfs:comment": "The unique identifier for this lodging house contact."
                },
                {
                    "@id": "cefact:LodgingHouse_Route.Identification.Identifier",
                    "@type": "unece:BasicBIE",
                    "unece:cefactUNId": "UN01001236",
                    "unece:cefactBieDomainClass": "cefact:LodgingHouse_Route.Details",
                    "rdfs:comment": "The unique identifier for the route to this lodging house."
                },
                {
                    "@id": "cefact:LodgingHouse_TravelProduct.Identification.Identifier",
                    "@type": "unece:BasicBIE",
                    "unece:cefactUNId": "UN01004919",
                    "unece:cefactBieDomainClass": "cefact:LodgingHouse_TravelProduct.Details",
                    "rdfs:comment": "The unique identifier for this lodging house travel product."
                },
                {
                    "@id": "cefact:Bathing_Facility.Identification.Identifier",
                    "@type": "unece:BasicBIE",
                    "unece:cefactUNId": "UN01001062",
                    "unece:cefactBieDomainClass": "cefact:Bathing_Facility.Details",
                    "rdfs:comment": "The unique identifier for this bathing facility."
                },
                {
                    "@id": "cefact:LodgingHouse_Picture.Identification.Identifier",
                    "@type": "unece:BasicBIE",
                    "unece:cefactUNId": "UN01001242",
                    "unece:cefactBieDomainClass": "cefact:LodgingHouse_Picture.Details",
                    "rdfs:comment": "The unique identifier for this lodging house picture."
                },
                {
                    "@id": "cefact:LodgingHouse_Building.Identification.Identifier",
                    "@type": "unece:BasicBIE",
                    "unece:cefactUNId": "UN01001038",
                    "unece:cefactBieDomainClass": "cefact:LodgingHouse_Building.Details",
                    "rdfs:comment": "A unique identifier for this lodging house building."
                },
                {
                    "@id": "cefact:LodgingHouse_Contract.Identification.Identifier",
                    "@type": "unece:BasicBIE",
                    "unece:TDED": "1296",
                    "unece:cefactUNId": "UN01001211",
                    "unece:cefactBieDomainClass": "cefact:LodgingHouse_Contract.Details",
                    "rdfs:comment": "The unique identifier for this lodging house contract."
                },
                {
                    "@id": "cefact:LodgingHouse_UsageCondition.Identification.Identifier",
                    "@type": "unece:BasicBIE",
                    "unece:cefactUNId": "UN01001200",
                    "unece:cefactBieDomainClass": "cefact:LodgingHouse_UsageCondition.Details",
                    "rdfs:comment": "The unique identifier for this lodging house usage condition."
                }
            ]
        },
        {
            "@id": "tourism:identifiedParty",
            "@type": "rdf:Property",
            "schema:rangeIncludes": {
                "@id": "tourism:Party"
            },
            "schema:domainIncludes": {
                "@id": "tourism:LodgingHouseContract"
            },
            "rdfs:comment": "The lodging house party identified in this lodging house contract.",
            "rdfs:label": "identifiedParty",
            "unece:cefactElementMetadata": [
                {
                    "@id": "cefact:LodgingHouse_Contract.Identified.LodgingHouse_Party",
                    "@type": "unece:AssociationBIE",
                    "unece:cefactUNId": "UN01001216",
                    "unece:cefactBieDomainClass": "cefact:LodgingHouse_Contract.Details",
                    "rdfs:comment": "The lodging house party identified in this lodging house contract."
                }
            ]
        },
        {
            "@id": "tourism:includedEvent",
            "@type": "rdf:Property",
            "schema:rangeIncludes": {
                "@id": "tourism:Event"
            },
            "schema:domainIncludes": {
                "@id": "tourism:ExperienceProduct"
            },
            "rdfs:comment": "An event included within this experience product.",
            "rdfs:label": "includedEvent",
            "unece:cefactElementMetadata": [
                {
                    "@id": "cefact:Experience_Product.Included.Experience_Event",
                    "@type": "unece:AssociationBIE",
                    "unece:cefactUNId": "UN01015173",
                    "unece:cefactBieDomainClass": "cefact:Experience_Product.Details",
                    "rdfs:comment": "An event included within this experience product."
                }
            ]
        },
        {
            "@id": "tourism:includedTravelProductComponent",
            "@type": "rdf:Property",
            "schema:rangeIncludes": {
                "@id": "tourism:TravelProductComponent"
            },
            "schema:domainIncludes": {
                "@id": "tourism:LodgingHouseTravelProduct"
            },
            "rdfs:comment": "A lodging house travel product component included in this lodging house travel product.",
            "rdfs:label": "includedTravelProductComponent",
            "unece:cefactElementMetadata": [
                {
                    "@id": "cefact:LodgingHouse_TravelProduct.Included.LodgingHouse_TravelProductComponent",
                    "@type": "unece:AssociationBIE",
                    "unece:cefactUNId": "UN01004937",
                    "unece:cefactBieDomainClass": "cefact:LodgingHouse_TravelProduct.Details",
                    "rdfs:comment": "A lodging house travel product component included in this lodging house travel product."
                }
            ]
        },
        {
            "@id": "tourism:includedTravelProductSub-Component",
            "@type": "rdf:Property",
            "schema:rangeIncludes": {
                "@id": "tourism:TravelProductSub-Component"
            },
            "schema:domainIncludes": {
                "@id": "tourism:ProductComponentItinerary"
            },
            "rdfs:comment": "The lodging house travel product sub-component included in this product component itinerary.",
            "rdfs:label": "includedTravelProductSub-Component",
            "unece:cefactElementMetadata": [
                {
                    "@id": "cefact:ProductComponent_Itinerary.Included.LodgingHouse_TravelProductSub-Component",
                    "@type": "unece:AssociationBIE",
                    "unece:cefactUNId": "UN01004984",
                    "unece:cefactBieDomainClass": "cefact:ProductComponent_Itinerary.Details",
                    "rdfs:comment": "The lodging house travel product sub-component included in this product component itinerary."
                }
            ]
        },
        {
            "@id": "tourism:indemnityClause",
            "@type": "rdf:Property",
            "schema:rangeIncludes": {
                "@id": "xsd:string"
            },
            "schema:domainIncludes": [
                {
                    "@id": "tourism:ExperienceEvent"
                },
                {
                    "@id": "tourism:ExperienceProduct"
                },
                {
                    "@id": "tourism:LodgingHouseTravelProduct"
                }
            ],
            "rdfs:comment": [
                "An indemnity clause, expressed as text, for this experience event.",
                "An indemnity clause, expressed as text, for this experience product.",
                "The indemnity clause, expressed as text, for this lodging house travel product."
            ],
            "rdfs:label": "indemnityClause",
            "unece:cefactElementMetadata": [
                {
                    "@id": "cefact:Experience_Event.Indemnity_Clause.Text",
                    "@type": "unece:BasicBIE",
                    "unece:cefactUNId": "UN01015127",
                    "unece:cefactBieDomainClass": "cefact:Experience_Event.Details",
                    "rdfs:comment": "An indemnity clause, expressed as text, for this experience event."
                },
                {
                    "@id": "cefact:LodgingHouse_TravelProduct.IndemnityClause.Text",
                    "@type": "unece:BasicBIE",
                    "unece:cefactUNId": "UN01004928",
                    "unece:cefactBieDomainClass": "cefact:LodgingHouse_TravelProduct.Details",
                    "rdfs:comment": "The indemnity clause, expressed as text, for this lodging house travel product."
                },
                {
                    "@id": "cefact:Experience_Product.Indemnity_Clause.Text",
                    "@type": "unece:BasicBIE",
                    "unece:cefactUNId": "UN01015166",
                    "unece:cefactBieDomainClass": "cefact:Experience_Product.Details",
                    "rdfs:comment": "An indemnity clause, expressed as text, for this experience product."
                }
            ]
        },
        {
            "@id": "tourism:information",
            "@type": "rdf:Property",
            "schema:rangeIncludes": {
                "@id": "xsd:string"
            },
            "schema:domainIncludes": {
                "@id": "tourism:DailyPrice"
            },
            "rdfs:comment": "Information, expressed as text about this daily price.",
            "rdfs:label": "information",
            "unece:cefactElementMetadata": [
                {
                    "@id": "cefact:Daily_Price.Information.Text",
                    "@type": "unece:BasicBIE",
                    "unece:cefactUNId": "UN01009698",
                    "unece:cefactBieDomainClass": "cefact:Daily_Price.Details",
                    "rdfs:comment": "Information, expressed as text about this daily price."
                }
            ]
        },
        {
            "@id": "tourism:informationAddress",
            "@type": "rdf:Property",
            "schema:rangeIncludes": {
                "@id": "tourism:Address"
            },
            "schema:domainIncludes": {
                "@id": "tourism:GuestPerson"
            },
            "rdfs:comment": "The structured address information of this guest.",
            "rdfs:label": "informationAddress",
            "unece:cefactElementMetadata": [
                {
                    "@id": "cefact:Guest_Person.Information.Structured_Address",
                    "@type": "unece:AssociationBIE",
                    "unece:cefactUNId": "UN01009718",
                    "unece:cefactBieDomainClass": "cefact:Guest_Person.Details",
                    "rdfs:comment": "The structured address information of this guest."
                }
            ]
        },
        {
            "@id": "tourism:informationProvidedPerson",
            "@type": "rdf:Property",
            "schema:rangeIncludes": {
                "@id": "tourism:Person"
            },
            "schema:domainIncludes": {
                "@id": "tourism:LodgingHouseTraveller"
            },
            "rdfs:comment": "The personal information provided for this lodging house traveller.",
            "rdfs:label": "informationProvidedPerson",
            "unece:cefactElementMetadata": [
                {
                    "@id": "cefact:LodgingHouse_Traveller.InformationProvided.Guest_Person",
                    "@type": "unece:AssociationBIE",
                    "unece:cefactUNId": "UN01009820",
                    "unece:cefactBieDomainClass": "cefact:LodgingHouse_Traveller.Details",
                    "rdfs:comment": "The personal information provided for this lodging house traveller."
                }
            ]
        },
        {
            "@id": "tourism:instruction",
            "@type": "rdf:Property",
            "schema:rangeIncludes": {
                "@id": "xsd:string"
            },
            "schema:domainIncludes": [
                {
                    "@id": "tourism:ExperienceEvent"
                },
                {
                    "@id": "tourism:ExperienceProduct"
                }
            ],
            "rdfs:comment": [
                "An instruction, expressed as text, for this experience event.",
                "An instruction, expressed as text, for this experience product."
            ],
            "rdfs:label": "instruction",
            "unece:cefactElementMetadata": [
                {
                    "@id": "cefact:Experience_Product.Instruction.Text",
                    "@type": "unece:BasicBIE",
                    "unece:cefactUNId": "UN01015163",
                    "unece:cefactBieDomainClass": "cefact:Experience_Product.Details",
                    "rdfs:comment": "An instruction, expressed as text, for this experience product."
                },
                {
                    "@id": "cefact:Experience_Event.Instruction.Text",
                    "@type": "unece:BasicBIE",
                    "unece:cefactUNId": "UN01015125",
                    "unece:cefactBieDomainClass": "cefact:Experience_Event.Details",
                    "rdfs:comment": "An instruction, expressed as text, for this experience event."
                }
            ]
        },
        {
            "@id": "tourism:issueDateTime",
            "@type": "rdf:Property",
            "schema:rangeIncludes": {
                "@id": "xsd:dateTime"
            },
            "schema:domainIncludes": {
                "@id": "tourism:ExperienceItemVoucher"
            },
            "rdfs:comment": "The date or date time of the issuance of this experience item voucher.",
            "rdfs:label": "issueDateTime",
            "unece:cefactElementMetadata": [
                {
                    "@id": "cefact:ExperienceItem_Voucher.Issue.DateTime",
                    "@type": "unece:BasicBIE",
                    "unece:cefactUNId": "UN01015245",
                    "unece:cefactBieDomainClass": "cefact:ExperienceItem_Voucher.Details",
                    "rdfs:comment": "The date or date time of the issuance of this experience item voucher."
                }
            ]
        },
        {
            "@id": "tourism:issuingCompanyName",
            "@type": "rdf:Property",
            "schema:rangeIncludes": {
                "@id": "xsd:string"
            },
            "schema:domainIncludes": {
                "@id": "tourism:ExperienceItemVoucher"
            },
            "rdfs:comment": "A name, expressed as text, of the company issuing this experience item voucher.",
            "rdfs:label": "issuingCompanyName",
            "unece:cefactElementMetadata": [
                {
                    "@id": "cefact:ExperienceItem_Voucher.IssuingCompanyName.Text",
                    "@type": "unece:BasicBIE",
                    "unece:cefactUNId": "UN01015246",
                    "unece:cefactBieDomainClass": "cefact:ExperienceItem_Voucher.Details",
                    "rdfs:comment": "A name, expressed as text, of the company issuing this experience item voucher."
                }
            ]
        },
        {
            "@id": "tourism:jobTitle",
            "@type": "rdf:Property",
            "schema:rangeIncludes": {
                "@id": "xsd:string"
            },
            "schema:domainIncludes": {
                "@id": "tourism:LodgingHouseContact"
            },
            "rdfs:comment": "The job title, position or designation, expressed as text, of this contact person for this lodging house.",
            "rdfs:label": "jobTitle",
            "unece:cefactElementMetadata": [
                {
                    "@id": "cefact:LodgingHouse_Contact.JobTitle.Text",
                    "@type": "unece:BasicBIE",
                    "unece:cefactUNId": "UN01001223",
                    "unece:cefactBieDomainClass": "cefact:LodgingHouse_Contact.Details",
                    "rdfs:comment": "The job title, position or designation, expressed as text, of this contact person for this lodging house."
                }
            ]
        },
        {
            "@id": "tourism:keywordMarketingPhrase",
            "@type": "rdf:Property",
            "schema:rangeIncludes": {
                "@id": "xsd:string"
            },
            "schema:domainIncludes": {
                "@id": "tourism:LodgingHouseFeature"
            },
            "rdfs:comment": "A keyword for a catch phrase, expressed as text, for marketing this lodging house feature.",
            "rdfs:label": "keywordMarketingPhrase",
            "unece:cefactElementMetadata": [
                {
                    "@id": "cefact:LodgingHouse_Feature.Keyword_MarketingPhrase.Text",
                    "@type": "unece:BasicBIE",
                    "unece:cefactUNId": "UN01001187",
                    "unece:cefactBieDomainClass": "cefact:LodgingHouse_Feature.Details",
                    "rdfs:comment": "A keyword for a catch phrase, expressed as text, for marketing this lodging house feature."
                }
            ]
        },
        {
            "@id": "tourism:languageCode",
            "@type": "rdf:Property",
            "schema:rangeIncludes": {
                "@id": "xsd:token"
            },
            "schema:domainIncludes": {
                "@id": "tourism:LodgingHouseParty"
            },
            "rdfs:comment": "A code specifying a language for this lodging house party.",
            "rdfs:label": "languageCode",
            "unece:cefactElementMetadata": [
                {
                    "@id": "cefact:LodgingHouse_Party.Language.Code",
                    "@type": "unece:BasicBIE",
                    "unece:TDED": "3453",
                    "unece:cefactUNId": "UN01001288",
                    "unece:cefactBieDomainClass": "cefact:LodgingHouse_Party.Details",
                    "rdfs:comment": "A code specifying a language for this lodging house party."
                }
            ]
        },
        {
            "@id": "tourism:languageId",
            "@type": "rdf:Property",
            "schema:rangeIncludes": {
                "@id": "xsd:token"
            },
            "schema:domainIncludes": {
                "@id": "tourism:GuestPerson"
            },
            "rdfs:comment": "The identifier of the language of this guest.",
            "rdfs:label": "languageId",
            "unece:cefactElementMetadata": [
                {
                    "@id": "cefact:Guest_Person.Language.Identifier",
                    "@type": "unece:BasicBIE",
                    "unece:TDED": "3453",
                    "unece:cefactUNId": "UN01009714",
                    "unece:cefactBieDomainClass": "cefact:Guest_Person.Details",
                    "rdfs:comment": "The identifier of the language of this guest."
                }
            ]
        },
        {
            "@id": "tourism:latestRenovationDate",
            "@type": "rdf:Property",
            "schema:rangeIncludes": {
                "@id": "xsd:base64Binary"
            },
            "schema:domainIncludes": [
                {
                    "@id": "tourism:BathingFacility"
                },
                {
                    "@id": "tourism:BusinessSupportRoomFacility"
                },
                {
                    "@id": "tourism:GuestRoomFacility"
                },
                {
                    "@id": "tourism:LodgingHouseBuilding"
                }
            ],
            "rdfs:comment": [
                "The date of the latest renovation of this bathing facility.",
                "The date of the latest renovation of this business support room.",
                "The date of the latest renovation of this guest room.",
                "The date of the latest renovation of this lodging house building."
            ],
            "rdfs:label": "latestRenovationDate",
            "unece:cefactElementMetadata": [
                {
                    "@id": "cefact:GuestRoom_Facility.Latest_Renovation.Date",
                    "@type": "unece:BasicBIE",
                    "unece:cefactUNId": "UN01001053",
                    "unece:cefactBieDomainClass": "cefact:GuestRoom_Facility.Details",
                    "rdfs:comment": "The date of the latest renovation of this guest room."
                },
                {
                    "@id": "cefact:Bathing_Facility.Latest_Renovation.Date",
                    "@type": "unece:BasicBIE",
                    "unece:cefactUNId": "UN01001067",
                    "unece:cefactBieDomainClass": "cefact:Bathing_Facility.Details",
                    "rdfs:comment": "The date of the latest renovation of this bathing facility."
                },
                {
                    "@id": "cefact:BusinessSupportRoom_Facility.Latest_Renovation.Date",
                    "@type": "unece:BasicBIE",
                    "unece:cefactUNId": "UN01001111",
                    "unece:cefactBieDomainClass": "cefact:BusinessSupportRoom_Facility.Details",
                    "rdfs:comment": "The date of the latest renovation of this business support room."
                },
                {
                    "@id": "cefact:LodgingHouse_Building.Latest_Renovation.Date",
                    "@type": "unece:BasicBIE",
                    "unece:cefactUNId": "UN01001043",
                    "unece:cefactBieDomainClass": "cefact:LodgingHouse_Building.Details",
                    "rdfs:comment": "The date of the latest renovation of this lodging house building."
                }
            ]
        },
        {
            "@id": "tourism:latestRenovationDateTime",
            "@type": "rdf:Property",
            "schema:rangeIncludes": {
                "@id": "xsd:dateTime"
            },
            "schema:domainIncludes": {
                "@id": "tourism:ExperienceFacility"
            },
            "rdfs:comment": "The date of the latest renovation of this experience facility.",
            "rdfs:label": "latestRenovationDateTime",
            "unece:cefactElementMetadata": [
                {
                    "@id": "cefact:Experience_Facility.Latest_Renovation.DateTime",
                    "@type": "unece:BasicBIE",
                    "unece:cefactUNId": "UN01015144",
                    "unece:cefactBieDomainClass": "cefact:Experience_Facility.Details",
                    "rdfs:comment": "The date of the latest renovation of this experience facility."
                }
            ]
        },
        {
            "@id": "tourism:leaderIndicator",
            "@type": "rdf:Property",
            "schema:rangeIncludes": {
                "@id": "xsd:boolean"
            },
            "schema:domainIncludes": {
                "@id": "tourism:LodgingHouseTraveller"
            },
            "rdfs:comment": "The indication of whether or not this lodging house traveller is a leader of a group of travellers.",
            "rdfs:label": "leaderIndicator",
            "unece:cefactElementMetadata": [
                {
                    "@id": "cefact:LodgingHouse_Traveller.Leader.Indicator",
                    "@type": "unece:BasicBIE",
                    "unece:cefactUNId": "UN01009814",
                    "unece:cefactBieDomainClass": "cefact:LodgingHouse_Traveller.Details",
                    "rdfs:comment": "The indication of whether or not this lodging house traveller is a leader of a group of travellers."
                }
            ]
        },
        {
            "@id": "tourism:localeName",
            "@type": "rdf:Property",
            "schema:rangeIncludes": {
                "@id": "xsd:string"
            },
            "schema:domainIncludes": {
                "@id": "tourism:LodgingHouseFeature"
            },
            "rdfs:comment": "The name of the locale, expressed as text, for this lodging house feature.",
            "rdfs:label": "localeName",
            "unece:cefactElementMetadata": [
                {
                    "@id": "cefact:LodgingHouse_Feature.Locale_Name.Text",
                    "@type": "unece:BasicBIE",
                    "unece:cefactUNId": "UN01001185",
                    "unece:cefactBieDomainClass": "cefact:LodgingHouse_Feature.Details",
                    "rdfs:comment": "The name of the locale, expressed as text, for this lodging house feature."
                }
            ]
        },
        {
            "@id": "tourism:location",
            "@type": "rdf:Property",
            "schema:rangeIncludes": {
                "@id": "xsd:string"
            },
            "schema:domainIncludes": [
                {
                    "@id": "tourism:ExperienceEvent"
                },
                {
                    "@id": "tourism:ExperienceProduct"
                }
            ],
            "rdfs:comment": [
                "A location, expressed as text, for this experience event.",
                "A location, expressed as text, specified for this experience product."
            ],
            "rdfs:label": "location",
            "unece:cefactElementMetadata": [
                {
                    "@id": "cefact:Experience_Product.Location.Text",
                    "@type": "unece:BasicBIE",
                    "unece:cefactUNId": "UN01015164",
                    "unece:cefactBieDomainClass": "cefact:Experience_Product.Details",
                    "rdfs:comment": "A location, expressed as text, specified for this experience product."
                },
                {
                    "@id": "cefact:Experience_Event.Location.Text",
                    "@type": "unece:BasicBIE",
                    "unece:cefactUNId": "UN01015122",
                    "unece:cefactBieDomainClass": "cefact:Experience_Event.Details",
                    "rdfs:comment": "A location, expressed as text, for this experience event."
                }
            ]
        },
        {
            "@id": "tourism:lodgingHousePartyRoleCode",
            "@type": "rdf:Property",
            "schema:rangeIncludes": {
                "@id": "unece:UNECECL3035Code"
            },
            "schema:domainIncludes": {
                "@id": "tourism:LodgingHouseParty"
            },
            "rdfs:comment": "The code specifying the role of this lodging house party.",
            "rdfs:label": "lodgingHousePartyRoleCode",
            "unece:cefactElementMetadata": [
                {
                    "@id": "cefact:LodgingHouse_Party.Role.Code",
                    "@type": "unece:BasicBIE",
                    "unece:TDED": "3035",
                    "unece:cefactUNId": "UN01001287",
                    "unece:cefactBieDomainClass": "cefact:LodgingHouse_Party.Details",
                    "rdfs:comment": "The code specifying the role of this lodging house party."
                }
            ]
        },
        {
            "@id": "tourism:lowerAgeLimitNumeric",
            "@type": "rdf:Property",
            "schema:rangeIncludes": {
                "@id": "xsd:decimal"
            },
            "schema:domainIncludes": [
                {
                    "@id": "tourism:CustomerClass"
                },
                {
                    "@id": "tourism:LodgingHouseCustomerClass"
                }
            ],
            "rdfs:comment": [
                "The lower age limit in number of years for the category of a customer class.",
                "The lower age limit in number of years for the category of this lodging house customer class."
            ],
            "rdfs:label": "lowerAgeLimitNumeric",
            "unece:cefactElementMetadata": [
                {
                    "@id": "cefact:LodgingHouse_CustomerClass.LowerAgeLimit.Numeric",
                    "@type": "unece:BasicBIE",
                    "unece:cefactUNId": "UN01010033",
                    "unece:cefactBieDomainClass": "cefact:LodgingHouse_CustomerClass.Details",
                    "rdfs:comment": "The lower age limit in number of years for the category of this lodging house customer class."
                },
                {
                    "@id": "cefact:CustomerClass.LowerAgeLimit.Numeric",
                    "@type": "unece:BasicBIE",
                    "unece:cefactUNId": "UN01004949",
                    "unece:cefactBieDomainClass": "cefact:CustomerClass.Details",
                    "rdfs:comment": "The lower age limit in number of years for the category of a customer class."
                }
            ]
        },
        {
            "@id": "tourism:makingPerson",
            "@type": "rdf:Property",
            "schema:rangeIncludes": {
                "@id": "tourism:Person"
            },
            "schema:domainIncludes": {
                "@id": "tourism:LodgingHouseReservation"
            },
            "rdfs:comment": "The person making this lodging house reservation.",
            "rdfs:label": "makingPerson",
            "unece:cefactElementMetadata": [
                {
                    "@id": "cefact:LodgingHouse_Reservation.Making.Reserving_Person",
                    "@type": "unece:AssociationBIE",
                    "unece:cefactUNId": "UN01009803",
                    "unece:cefactBieDomainClass": "cefact:LodgingHouse_Reservation.Details",
                    "rdfs:comment": "The person making this lodging house reservation."
                }
            ]
        },
        {
            "@id": "tourism:mapBinaryObject",
            "@type": "rdf:Property",
            "schema:rangeIncludes": {
                "@id": "xsd:base64Binary"
            },
            "schema:domainIncludes": {
                "@id": "tourism:LodgingHouseRoute"
            },
            "rdfs:comment": "A binary object data of a map for this route to this lodging house.",
            "rdfs:label": "mapBinaryObject",
            "unece:cefactElementMetadata": [
                {
                    "@id": "cefact:LodgingHouse_Route.Map.BinaryObject",
                    "@type": "unece:BasicBIE",
                    "unece:cefactUNId": "UN01001238",
                    "unece:cefactBieDomainClass": "cefact:LodgingHouse_Route.Details",
                    "rdfs:comment": "A binary object data of a map for this route to this lodging house."
                }
            ]
        },
        {
            "@id": "tourism:marketingPhrase",
            "@type": "rdf:Property",
            "schema:rangeIncludes": {
                "@id": "xsd:string"
            },
            "schema:domainIncludes": [
                {
                    "@id": "tourism:BathingFacility"
                },
                {
                    "@id": "tourism:LodgingHouseFeature"
                }
            ],
            "rdfs:comment": [
                "A catch phrase, expressed as text, for marketing this lodging house feature.",
                "The catch phrase, expressed as text, for marketing of this bathing facility."
            ],
            "rdfs:label": "marketingPhrase",
            "unece:cefactElementMetadata": [
                {
                    "@id": "cefact:Bathing_Facility.MarketingPhrase.Text",
                    "@type": "unece:BasicBIE",
                    "unece:cefactUNId": "UN01001068",
                    "unece:cefactBieDomainClass": "cefact:Bathing_Facility.Details",
                    "rdfs:comment": "The catch phrase, expressed as text, for marketing of this bathing facility."
                },
                {
                    "@id": "cefact:LodgingHouse_Feature.MarketingPhrase.Text",
                    "@type": "unece:BasicBIE",
                    "unece:cefactUNId": "UN01001186",
                    "unece:cefactBieDomainClass": "cefact:LodgingHouse_Feature.Details",
                    "rdfs:comment": "A catch phrase, expressed as text, for marketing this lodging house feature."
                }
            ]
        },
        {
            "@id": "tourism:maximumOccupancy",
            "@type": "rdf:Property",
            "schema:rangeIncludes": {
                "@id": "xsd:string"
            },
            "schema:domainIncludes": {
                "@id": "tourism:LodgingHouseUsageCondition"
            },
            "rdfs:comment": "The maximum occupancy, expressed as text, applicable to the lodging house usage condition.",
            "rdfs:label": "maximumOccupancy",
            "unece:cefactElementMetadata": [
                {
                    "@id": "cefact:LodgingHouse_UsageCondition.Maximum_Occupancy.Text",
                    "@type": "unece:BasicBIE",
                    "unece:cefactUNId": "UN01001209",
                    "unece:cefactBieDomainClass": "cefact:LodgingHouse_UsageCondition.Details",
                    "rdfs:comment": "The maximum occupancy, expressed as text, applicable to the lodging house usage condition."
                }
            ]
        },
        {
            "@id": "tourism:maximumQuantity",
            "@type": "rdf:Property",
            "schema:rangeIncludes": {
                "@id": "xsd:decimal"
            },
            "schema:domainIncludes": [
                {
                    "@id": "tourism:LodgingHouseReservationRestriction"
                },
                {
                    "@id": "tourism:ReservationRestriction"
                }
            ],
            "rdfs:comment": [
                "The maximum quantity for this lodging house reservation restriction.",
                "The maximum quantity for this reservation restriction."
            ],
            "rdfs:label": "maximumQuantity",
            "unece:cefactElementMetadata": [
                {
                    "@id": "cefact:LodgingHouse_ReservationRestriction.Maximum.Quantity",
                    "@type": "unece:BasicBIE",
                    "unece:cefactUNId": "UN01010049",
                    "unece:cefactBieDomainClass": "cefact:LodgingHouse_ReservationRestriction.Details",
                    "rdfs:comment": "The maximum quantity for this lodging house reservation restriction."
                },
                {
                    "@id": "cefact:ReservationRestriction.Maximum.Quantity",
                    "@type": "unece:BasicBIE",
                    "unece:cefactUNId": "UN01004957",
                    "unece:cefactBieDomainClass": "cefact:ReservationRestriction.Details",
                    "rdfs:comment": "The maximum quantity for this reservation restriction."
                }
            ]
        },
        {
            "@id": "tourism:maximumUnitQuantity",
            "@type": "rdf:Property",
            "schema:rangeIncludes": {
                "@id": "xsd:decimal"
            },
            "schema:domainIncludes": {
                "@id": "tourism:ExperienceProduct"
            },
            "rdfs:comment": "The maximum number of units of this experience product.",
            "rdfs:label": "maximumUnitQuantity",
            "unece:cefactElementMetadata": [
                {
                    "@id": "cefact:Experience_Product.Maximum_Unit.Quantity",
                    "@type": "unece:BasicBIE",
                    "unece:cefactUNId": "UN01015169",
                    "unece:cefactBieDomainClass": "cefact:Experience_Product.Details",
                    "rdfs:comment": "The maximum number of units of this experience product."
                }
            ]
        },
        {
            "@id": "tourism:mealServiceCategoryCode",
            "@type": "rdf:Property",
            "schema:rangeIncludes": {
                "@id": "xsd:token"
            },
            "schema:domainIncludes": [
                {
                    "@id": "tourism:CustomerClass"
                },
                {
                    "@id": "tourism:LodgingHouseCustomerClass"
                }
            ],
            "rdfs:comment": [
                "The code specifying the meal service category for a customer class.",
                "The code specifying the meal service category for this lodging house customer class."
            ],
            "rdfs:label": "mealServiceCategoryCode",
            "unece:cefactElementMetadata": [
                {
                    "@id": "cefact:CustomerClass.MealServiceCategory.Code",
                    "@type": "unece:BasicBIE",
                    "unece:cefactUNId": "UN01004951",
                    "unece:cefactBieDomainClass": "cefact:CustomerClass.Details",
                    "rdfs:comment": "The code specifying the meal service category for a customer class."
                },
                {
                    "@id": "cefact:LodgingHouse_CustomerClass.MealServiceCategory.Code",
                    "@type": "unece:BasicBIE",
                    "unece:cefactUNId": "UN01010035",
                    "unece:cefactBieDomainClass": "cefact:LodgingHouse_CustomerClass.Details",
                    "rdfs:comment": "The code specifying the meal service category for this lodging house customer class."
                }
            ]
        },
        {
            "@id": "tourism:meetingDateTime",
            "@type": "rdf:Property",
            "schema:rangeIncludes": {
                "@id": "xsd:dateTime"
            },
            "schema:domainIncludes": {
                "@id": "tourism:ExperienceEvent"
            },
            "rdfs:comment": "The meeting date, time, date time, or other date time value for this experience event.",
            "rdfs:label": "meetingDateTime",
            "unece:cefactElementMetadata": [
                {
                    "@id": "cefact:Experience_Event.Meeting.DateTime",
                    "@type": "unece:BasicBIE",
                    "unece:cefactUNId": "UN01015123",
                    "unece:cefactBieDomainClass": "cefact:Experience_Event.Details",
                    "rdfs:comment": "The meeting date, time, date time, or other date time value for this experience event."
                }
            ]
        },
        {
            "@id": "tourism:messageTypeCode",
            "@type": "rdf:Property",
            "schema:rangeIncludes": {
                "@id": "xsd:token"
            },
            "schema:domainIncludes": {
                "@id": "tourism:LodgingHouseReservation"
            },
            "rdfs:comment": "The code specifying the type of reservation message.for this lodging house.",
            "rdfs:label": "messageTypeCode",
            "unece:cefactElementMetadata": [
                {
                    "@id": "cefact:LodgingHouse_Reservation.MessageType.Code",
                    "@type": "unece:BasicBIE",
                    "unece:cefactUNId": "UN01009790",
                    "unece:cefactBieDomainClass": "cefact:LodgingHouse_Reservation.Details",
                    "rdfs:comment": "The code specifying the type of reservation message.for this lodging house."
                }
            ]
        },
        {
            "@id": "tourism:minimumQuantity",
            "@type": "rdf:Property",
            "schema:rangeIncludes": {
                "@id": "xsd:decimal"
            },
            "schema:domainIncludes": [
                {
                    "@id": "tourism:LodgingHouseReservationRestriction"
                },
                {
                    "@id": "tourism:ReservationRestriction"
                }
            ],
            "rdfs:comment": [
                "The minimum quantity for this lodging house reservation restriction.",
                "The minimum quantity for this reservation restriction."
            ],
            "rdfs:label": "minimumQuantity",
            "unece:cefactElementMetadata": [
                {
                    "@id": "cefact:ReservationRestriction.Minimum.Quantity",
                    "@type": "unece:BasicBIE",
                    "unece:cefactUNId": "UN01004956",
                    "unece:cefactBieDomainClass": "cefact:ReservationRestriction.Details",
                    "rdfs:comment": "The minimum quantity for this reservation restriction."
                },
                {
                    "@id": "cefact:LodgingHouse_ReservationRestriction.Minimum.Quantity",
                    "@type": "unece:BasicBIE",
                    "unece:cefactUNId": "UN01010048",
                    "unece:cefactBieDomainClass": "cefact:LodgingHouse_ReservationRestriction.Details",
                    "rdfs:comment": "The minimum quantity for this lodging house reservation restriction."
                }
            ]
        },
        {
            "@id": "tourism:minimumUnitQuantity",
            "@type": "rdf:Property",
            "schema:rangeIncludes": {
                "@id": "xsd:decimal"
            },
            "schema:domainIncludes": {
                "@id": "tourism:ExperienceProduct"
            },
            "rdfs:comment": "The minimum number of units of this experience product.",
            "rdfs:label": "minimumUnitQuantity",
            "unece:cefactElementMetadata": [
                {
                    "@id": "cefact:Experience_Product.Minimum_Unit.Quantity",
                    "@type": "unece:BasicBIE",
                    "unece:cefactUNId": "UN01015170",
                    "unece:cefactBieDomainClass": "cefact:Experience_Product.Details",
                    "rdfs:comment": "The minimum number of units of this experience product."
                }
            ]
        },
        {
            "@id": "tourism:multipleReasonIndicator",
            "@type": "rdf:Property",
            "schema:rangeIncludes": {
                "@id": "xsd:boolean"
            },
            "schema:domainIncludes": [
                {
                    "@id": "tourism:DiscountPrice"
                },
                {
                    "@id": "tourism:ExtraPrice"
                }
            ],
            "rdfs:comment": [
                "The indication of whether or not multiple reasons affect the extra price.",
                "The indication of whether or not multiple reasons affect this discount price."
            ],
            "rdfs:label": "multipleReasonIndicator",
            "unece:cefactElementMetadata": [
                {
                    "@id": "cefact:Discount_Price.MultipleReason.Indicator",
                    "@type": "unece:BasicBIE",
                    "unece:cefactUNId": "UN01005048",
                    "unece:cefactBieDomainClass": "cefact:Discount_Price.Details",
                    "rdfs:comment": "The indication of whether or not multiple reasons affect this discount price."
                },
                {
                    "@id": "cefact:Extra_Price.MultipleReason.Indicator",
                    "@type": "unece:BasicBIE",
                    "unece:cefactUNId": "UN01005029",
                    "unece:cefactBieDomainClass": "cefact:Extra_Price.Details",
                    "rdfs:comment": "The indication of whether or not multiple reasons affect the extra price."
                }
            ]
        },
        {
            "@id": "tourism:name",
            "@type": "rdf:Property",
            "schema:rangeIncludes": {
                "@id": "xsd:string"
            },
            "schema:domainIncludes": [
                {
                    "@id": "tourism:BathingFacility"
                },
                {
                    "@id": "tourism:BusinessSupportRoomFacility"
                },
                {
                    "@id": "tourism:ExperienceEvent"
                },
                {
                    "@id": "tourism:ExperienceFacility"
                },
                {
                    "@id": "tourism:ExperienceProduct"
                },
                {
                    "@id": "tourism:GuestAllergy"
                },
                {
                    "@id": "tourism:GuestCarriedEquipment"
                },
                {
                    "@id": "tourism:GuestDisability"
                },
                {
                    "@id": "tourism:GuestFoodChoice"
                },
                {
                    "@id": "tourism:GuestPerson"
                },
                {
                    "@id": "tourism:GuestRoomFacility"
                },
                {
                    "@id": "tourism:LodgingHouseLocation"
                },
                {
                    "@id": "tourism:LodgingHouseOrganization"
                },
                {
                    "@id": "tourism:LodgingHouseParty"
                },
                {
                    "@id": "tourism:LodgingHouseTravelProduct"
                },
                {
                    "@id": "tourism:LodgingHouseTravelProductComponent"
                },
                {
                    "@id": "tourism:LodgingHouseTravelProductSubComponent"
                }
            ],
            "rdfs:comment": [
                "A name, expressed as text, for this experience event.",
                "A name, expressed as text, for this experience facility.",
                "A name, expressed as text, for this experience product.",
                "A name, expressed as text, for this guest carried equipment.",
                "A name, expressed as text, for this guest disability.",
                "A name, expressed as text, for this guest food choice.",
                "A name, expressed as text, for this lodging house party.",
                "A name, expressed as text, of this guest allergy.",
                "A name, expressed as text, of this lodging house organization.",
                "The name, expressed as text, by which this guest is known.",
                "The name, expressed as text, for this lodging house location.",
                "The name, expressed as text, for this lodging house travel product component.",
                "The name, expressed as text, of this bathing facility.",
                "The name, expressed as text, of this business support room.",
                "The name, expressed as text, of this guest room.",
                "The name, expressed as text, of this lodging house travel product sub-component.",
                "The name, expressed as text, of this lodging house travel product."
            ],
            "rdfs:label": "name",
            "unece:cefactElementMetadata": [
                {
                    "@id": "cefact:Guest_Disability.Name.Text",
                    "@type": "unece:BasicBIE",
                    "unece:cefactUNId": "UN01015201",
                    "unece:cefactBieDomainClass": "cefact:Guest_Disability.Details",
                    "rdfs:comment": "A name, expressed as text, for this guest disability."
                },
                {
                    "@id": "cefact:Guest_CarriedEquipment.Name.Text",
                    "@type": "unece:BasicBIE",
                    "unece:cefactUNId": "UN01015195",
                    "unece:cefactBieDomainClass": "cefact:Guest_CarriedEquipment.Details",
                    "rdfs:comment": "A name, expressed as text, for this guest carried equipment."
                },
                {
                    "@id": "cefact:Experience_Facility.Name.Text",
                    "@type": "unece:BasicBIE",
                    "unece:cefactUNId": "UN01015138",
                    "unece:cefactBieDomainClass": "cefact:Experience_Facility.Details",
                    "rdfs:comment": "A name, expressed as text, for this experience facility."
                },
                {
                    "@id": "cefact:LodgingHouse_TravelProduct.Name.Text",
                    "@type": "unece:BasicBIE",
                    "unece:cefactUNId": "UN01004921",
                    "unece:cefactBieDomainClass": "cefact:LodgingHouse_TravelProduct.Details",
                    "rdfs:comment": "The name, expressed as text, of this lodging house travel product."
                },
                {
                    "@id": "cefact:Experience_Product.Name.Text",
                    "@type": "unece:BasicBIE",
                    "unece:TDED": "7134",
                    "unece:cefactUNId": "UN01015160",
                    "unece:cefactBieDomainClass": "cefact:Experience_Product.Details",
                    "rdfs:comment": "A name, expressed as text, for this experience product."
                },
                {
                    "@id": "cefact:LodgingHouse_TravelProductComponent.Name.Text",
                    "@type": "unece:BasicBIE",
                    "unece:cefactUNId": "UN01004976",
                    "unece:cefactBieDomainClass": "cefact:LodgingHouse_TravelProductComponent.Details",
                    "rdfs:comment": "The name, expressed as text, for this lodging house travel product component."
                },
                {
                    "@id": "cefact:BusinessSupportRoom_Facility.Name.Text",
                    "@type": "unece:BasicBIE",
                    "unece:cefactUNId": "UN01001109",
                    "unece:cefactBieDomainClass": "cefact:BusinessSupportRoom_Facility.Details",
                    "rdfs:comment": "The name, expressed as text, of this business support room."
                },
                {
                    "@id": "cefact:LodgingHouse_Location.Name.Text",
                    "@type": "unece:BasicBIE",
                    "unece:TDED": "3224",
                    "unece:cefactUNId": "UN01001219",
                    "unece:cefactBieDomainClass": "cefact:LodgingHouse_Location.Details",
                    "rdfs:comment": "The name, expressed as text, for this lodging house location."
                },
                {
                    "@id": "cefact:Experience_Event.Name.Text",
                    "@type": "unece:BasicBIE",
                    "unece:cefactUNId": "UN01015117",
                    "unece:cefactBieDomainClass": "cefact:Experience_Event.Details",
                    "rdfs:comment": "A name, expressed as text, for this experience event."
                },
                {
                    "@id": "cefact:LodgingHouse_Party.Name.Text",
                    "@type": "unece:BasicBIE",
                    "unece:TDED": "3036",
                    "unece:cefactUNId": "UN01001283",
                    "unece:cefactBieDomainClass": "cefact:LodgingHouse_Party.Details",
                    "rdfs:comment": "A name, expressed as text, for this lodging house party."
                },
                {
                    "@id": "cefact:Guest_Person.Name.Text",
                    "@type": "unece:BasicBIE",
                    "unece:TDED": "3404",
                    "unece:cefactUNId": "UN01009710",
                    "unece:cefactBieDomainClass": "cefact:Guest_Person.Details",
                    "rdfs:comment": "The name, expressed as text, by which this guest is known."
                },
                {
                    "@id": "cefact:LodgingHouse_TravelProductSub-Component.Name.Text",
                    "@type": "unece:BasicBIE",
                    "unece:cefactUNId": "UN01004989",
                    "unece:cefactBieDomainClass": "cefact:LodgingHouse_TravelProductSubComponent.Details",
                    "rdfs:comment": "The name, expressed as text, of this lodging house travel product sub-component."
                },
                {
                    "@id": "cefact:Guest_FoodChoice.Name.Text",
                    "@type": "unece:BasicBIE",
                    "unece:cefactUNId": "UN01015208",
                    "unece:cefactBieDomainClass": "cefact:Guest_FoodChoice.Details",
                    "rdfs:comment": "A name, expressed as text, for this guest food choice."
                },
                {
                    "@id": "cefact:Bathing_Facility.Name.Text",
                    "@type": "unece:BasicBIE",
                    "unece:cefactUNId": "UN01001065",
                    "unece:cefactBieDomainClass": "cefact:Bathing_Facility.Details",
                    "rdfs:comment": "The name, expressed as text, of this bathing facility."
                },
                {
                    "@id": "cefact:Guest_Allergy.Name.Text",
                    "@type": "unece:BasicBIE",
                    "unece:cefactUNId": "UN01015190",
                    "unece:cefactBieDomainClass": "cefact:Guest_Allergy.Details",
                    "rdfs:comment": "A name, expressed as text, of this guest allergy."
                },
                {
                    "@id": "cefact:LodgingHouse_Organization.Name.Text",
                    "@type": "unece:BasicBIE",
                    "unece:cefactUNId": "UN01001031",
                    "unece:cefactBieDomainClass": "cefact:LodgingHouse_Organization.Details",
                    "rdfs:comment": "A name, expressed as text, of this lodging house organization."
                },
                {
                    "@id": "cefact:GuestRoom_Facility.Name.Text",
                    "@type": "unece:BasicBIE",
                    "unece:cefactUNId": "UN01001051",
                    "unece:cefactBieDomainClass": "cefact:GuestRoom_Facility.Details",
                    "rdfs:comment": "The name, expressed as text, of this guest room."
                }
            ]
        },
        {
            "@id": "tourism:nationalityCountry",
            "@type": "rdf:Property",
            "schema:rangeIncludes": {
                "@id": "tourism:Country"
            },
            "schema:domainIncludes": {
                "@id": "tourism:GuestPerson"
            },
            "rdfs:comment": "The country of nationality for this guest.",
            "rdfs:label": "nationalityCountry",
            "unece:cefactElementMetadata": [
                {
                    "@id": "cefact:Guest_Person.Nationality.Referenced_Country",
                    "@type": "unece:AssociationBIE",
                    "unece:cefactUNId": "UN01009719",
                    "unece:cefactBieDomainClass": "cefact:Guest_Person.Details",
                    "rdfs:comment": "The country of nationality for this guest."
                }
            ]
        },
        {
            "@id": "tourism:netPriceIndicator",
            "@type": "rdf:Property",
            "schema:rangeIncludes": {
                "@id": "xsd:boolean"
            },
            "schema:domainIncludes": [
                {
                    "@id": "tourism:BasicPrice"
                },
                {
                    "@id": "tourism:CancellationPrice"
                },
                {
                    "@id": "tourism:DiscountPrice"
                },
                {
                    "@id": "tourism:ExtraPrice"
                }
            ],
            "rdfs:comment": [
                "The indication of whether or not the basic price is a net price.",
                "The indication of whether or not the cancellation price is a net price.",
                "The indication of whether or not the discount price is a net price.",
                "The indication of whether or not the extra price is a net price."
            ],
            "rdfs:label": "netPriceIndicator",
            "unece:cefactElementMetadata": [
                {
                    "@id": "cefact:Extra_Price.NetPrice.Indicator",
                    "@type": "unece:BasicBIE",
                    "unece:cefactUNId": "UN01005020",
                    "unece:cefactBieDomainClass": "cefact:Extra_Price.Details",
                    "rdfs:comment": "The indication of whether or not the extra price is a net price."
                },
                {
                    "@id": "cefact:Cancellation_Price.NetPrice.Indicator",
                    "@type": "unece:BasicBIE",
                    "unece:cefactUNId": "UN01005078",
                    "unece:cefactBieDomainClass": "cefact:Cancellation_Price.Details",
                    "rdfs:comment": "The indication of whether or not the cancellation price is a net price."
                },
                {
                    "@id": "cefact:Discount_Price.NetPrice.Indicator",
                    "@type": "unece:BasicBIE",
                    "unece:cefactUNId": "UN01005039",
                    "unece:cefactBieDomainClass": "cefact:Discount_Price.Details",
                    "rdfs:comment": "The indication of whether or not the discount price is a net price."
                },
                {
                    "@id": "cefact:Basic_Price.NetPrice.Indicator",
                    "@type": "unece:BasicBIE",
                    "unece:cefactUNId": "UN01005005",
                    "unece:cefactBieDomainClass": "cefact:Basic_Price.Details",
                    "rdfs:comment": "The indication of whether or not the basic price is a net price."
                }
            ]
        },
        {
            "@id": "tourism:notifiedAllergy",
            "@type": "rdf:Property",
            "schema:rangeIncludes": {
                "@id": "tourism:Allergy"
            },
            "schema:domainIncludes": {
                "@id": "tourism:GuestPerson"
            },
            "rdfs:comment": "An allergy notified for this guest person.",
            "rdfs:label": "notifiedAllergy",
            "unece:cefactElementMetadata": [
                {
                    "@id": "cefact:Guest_Person.Notified.Guest_Allergy",
                    "@type": "unece:AssociationBIE",
                    "unece:cefactUNId": "UN01015227",
                    "unece:cefactBieDomainClass": "cefact:Guest_Person.Details",
                    "rdfs:comment": "An allergy notified for this guest person."
                }
            ]
        },
        {
            "@id": "tourism:notifiedDisability",
            "@type": "rdf:Property",
            "schema:rangeIncludes": {
                "@id": "tourism:Disability"
            },
            "schema:domainIncludes": {
                "@id": "tourism:GuestPerson"
            },
            "rdfs:comment": "A disability notified for this guest person.",
            "rdfs:label": "notifiedDisability",
            "unece:cefactElementMetadata": [
                {
                    "@id": "cefact:Guest_Person.Notified.Guest_Disability",
                    "@type": "unece:AssociationBIE",
                    "unece:cefactUNId": "UN01015226",
                    "unece:cefactBieDomainClass": "cefact:Guest_Person.Details",
                    "rdfs:comment": "A disability notified for this guest person."
                }
            ]
        },
        {
            "@id": "tourism:notifiedFoodChoice",
            "@type": "rdf:Property",
            "schema:rangeIncludes": {
                "@id": "tourism:FoodChoice"
            },
            "schema:domainIncludes": {
                "@id": "tourism:GuestPerson"
            },
            "rdfs:comment": "A food choice notified for this guest person.",
            "rdfs:label": "notifiedFoodChoice",
            "unece:cefactElementMetadata": [
                {
                    "@id": "cefact:Guest_Person.Notified.Guest_FoodChoice",
                    "@type": "unece:AssociationBIE",
                    "unece:cefactUNId": "UN01015231",
                    "unece:cefactBieDomainClass": "cefact:Guest_Person.Details",
                    "rdfs:comment": "A food choice notified for this guest person."
                }
            ]
        },
        {
            "@id": "tourism:notifiedGuestArrival",
            "@type": "rdf:Property",
            "schema:rangeIncludes": {
                "@id": "tourism:GuestArrival"
            },
            "schema:domainIncludes": {
                "@id": "tourism:GuestPerson"
            },
            "rdfs:comment": "An arrival notified for this guest person.",
            "rdfs:label": "notifiedGuestArrival",
            "unece:cefactElementMetadata": [
                {
                    "@id": "cefact:Guest_Person.Notified.Specified_GuestArrival",
                    "@type": "unece:AssociationBIE",
                    "unece:cefactUNId": "UN01015221",
                    "unece:cefactBieDomainClass": "cefact:Guest_Person.Details",
                    "rdfs:comment": "An arrival notified for this guest person."
                }
            ]
        },
        {
            "@id": "tourism:notifiedHealthIndication",
            "@type": "rdf:Property",
            "schema:rangeIncludes": {
                "@id": "tourism:HealthIndication"
            },
            "schema:domainIncludes": {
                "@id": "tourism:GuestPerson"
            },
            "rdfs:comment": "A health indication notified for this guest person.",
            "rdfs:label": "notifiedHealthIndication",
            "unece:cefactElementMetadata": [
                {
                    "@id": "cefact:Guest_Person.Notified.Guest_HealthIndication",
                    "@type": "unece:AssociationBIE",
                    "unece:cefactUNId": "UN01015229",
                    "unece:cefactBieDomainClass": "cefact:Guest_Person.Details",
                    "rdfs:comment": "A health indication notified for this guest person."
                }
            ]
        },
        {
            "@id": "tourism:notifiedPreference",
            "@type": "rdf:Property",
            "schema:rangeIncludes": {
                "@id": "tourism:Preference"
            },
            "schema:domainIncludes": {
                "@id": "tourism:GuestPerson"
            },
            "rdfs:comment": "An experience item preference notified for this guest person.",
            "rdfs:label": "notifiedPreference",
            "unece:cefactElementMetadata": [
                {
                    "@id": "cefact:Guest_Person.Notified.ExperienceItem_Preference",
                    "@type": "unece:AssociationBIE",
                    "unece:cefactUNId": "UN01015230",
                    "unece:cefactBieDomainClass": "cefact:Guest_Person.Details",
                    "rdfs:comment": "An experience item preference notified for this guest person."
                }
            ]
        },
        {
            "@id": "tourism:notifiedProtectionMeans",
            "@type": "rdf:Property",
            "schema:rangeIncludes": {
                "@id": "tourism:ProtectionMeans"
            },
            "schema:domainIncludes": {
                "@id": "tourism:GuestPerson"
            },
            "rdfs:comment": "A disease protection means notified for this guest person.",
            "rdfs:label": "notifiedProtectionMeans",
            "unece:cefactElementMetadata": [
                {
                    "@id": "cefact:Guest_Person.Notified.Disease_ProtectionMeans",
                    "@type": "unece:AssociationBIE",
                    "unece:cefactUNId": "UN01015228",
                    "unece:cefactBieDomainClass": "cefact:Guest_Person.Details",
                    "rdfs:comment": "A disease protection means notified for this guest person."
                }
            ]
        },
        {
            "@id": "tourism:objective",
            "@type": "rdf:Property",
            "schema:rangeIncludes": {
                "@id": "xsd:string"
            },
            "schema:domainIncludes": {
                "@id": "tourism:ExperienceProduct"
            },
            "rdfs:comment": "An objective, expressed as text, for this experience product.",
            "rdfs:label": "objective",
            "unece:cefactElementMetadata": [
                {
                    "@id": "cefact:Experience_Product.Objective.Text",
                    "@type": "unece:BasicBIE",
                    "unece:cefactUNId": "UN01015162",
                    "unece:cefactBieDomainClass": "cefact:Experience_Product.Details",
                    "rdfs:comment": "An objective, expressed as text, for this experience product."
                }
            ]
        },
        {
            "@id": "tourism:occupantCapacityQuantity",
            "@type": "rdf:Property",
            "schema:rangeIncludes": {
                "@id": "xsd:decimal"
            },
            "schema:domainIncludes": {
                "@id": "tourism:LodgingHouseFeature"
            },
            "rdfs:comment": "The maximum number of occupants accommodated in this lodging house feature.",
            "rdfs:label": "occupantCapacityQuantity",
            "unece:cefactElementMetadata": [
                {
                    "@id": "cefact:LodgingHouse_Feature.Occupant_Capacity.Quantity",
                    "@type": "unece:BasicBIE",
                    "unece:cefactUNId": "UN01001189",
                    "unece:cefactBieDomainClass": "cefact:LodgingHouse_Feature.Details",
                    "rdfs:comment": "The maximum number of occupants accommodated in this lodging house feature."
                }
            ]
        },
        {
            "@id": "tourism:offeredService",
            "@type": "rdf:Property",
            "schema:rangeIncludes": {
                "@id": "tourism:Service"
            },
            "schema:domainIncludes": [
                {
                    "@id": "tourism:BathingFacility"
                },
                {
                    "@id": "tourism:BusinessSupportRoomFacility"
                },
                {
                    "@id": "tourism:GuestRoomFacility"
                }
            ],
            "rdfs:comment": [
                "A supplemental service that is offered for this bathing facility.",
                "A supplemental service that is offered for this business support room.",
                "A supplemental service that is offered for this guest room."
            ],
            "rdfs:label": "offeredService",
            "unece:cefactElementMetadata": [
                {
                    "@id": "cefact:GuestRoom_Facility.Offered.Supplemental_Service",
                    "@type": "unece:AssociationBIE",
                    "unece:cefactUNId": "UN01001060",
                    "unece:cefactBieDomainClass": "cefact:GuestRoom_Facility.Details",
                    "rdfs:comment": "A supplemental service that is offered for this guest room."
                },
                {
                    "@id": "cefact:Bathing_Facility.Offered.Supplemental_Service",
                    "@type": "unece:AssociationBIE",
                    "unece:cefactUNId": "UN01001075",
                    "unece:cefactBieDomainClass": "cefact:Bathing_Facility.Details",
                    "rdfs:comment": "A supplemental service that is offered for this bathing facility."
                },
                {
                    "@id": "cefact:BusinessSupportRoom_Facility.Offered.Supplemental_Service",
                    "@type": "unece:AssociationBIE",
                    "unece:cefactUNId": "UN01001117",
                    "unece:cefactBieDomainClass": "cefact:BusinessSupportRoom_Facility.Details",
                    "rdfs:comment": "A supplemental service that is offered for this business support room."
                }
            ]
        },
        {
            "@id": "tourism:operatingPeriod",
            "@type": "rdf:Property",
            "schema:rangeIncludes": {
                "@id": "tourism:Period"
            },
            "schema:domainIncludes": [
                {
                    "@id": "tourism:BathingFacility"
                },
                {
                    "@id": "tourism:BusinessSupportRoomFacility"
                },
                {
                    "@id": "tourism:GuestRoomFacility"
                }
            ],
            "rdfs:comment": [
                "A specified period of operation for this bathing facility.",
                "A specified period of operation for this business support room.",
                "A specified period of operation for this guest room."
            ],
            "rdfs:label": "operatingPeriod",
            "unece:cefactElementMetadata": [
                {
                    "@id": "cefact:Bathing_Facility.Operating.Specified_Period",
                    "@type": "unece:AssociationBIE",
                    "unece:cefactUNId": "UN01001071",
                    "unece:cefactBieDomainClass": "cefact:Bathing_Facility.Details",
                    "rdfs:comment": "A specified period of operation for this bathing facility."
                },
                {
                    "@id": "cefact:BusinessSupportRoom_Facility.Operating.Specified_Period",
                    "@type": "unece:AssociationBIE",
                    "unece:cefactUNId": "UN01001114",
                    "unece:cefactBieDomainClass": "cefact:BusinessSupportRoom_Facility.Details",
                    "rdfs:comment": "A specified period of operation for this business support room."
                },
                {
                    "@id": "cefact:GuestRoom_Facility.Operating.Specified_Period",
                    "@type": "unece:AssociationBIE",
                    "unece:cefactUNId": "UN01001057",
                    "unece:cefactBieDomainClass": "cefact:GuestRoom_Facility.Details",
                    "rdfs:comment": "A specified period of operation for this guest room."
                }
            ]
        },
        {
            "@id": "tourism:operationalPeriod",
            "@type": "rdf:Property",
            "schema:rangeIncludes": {
                "@id": "tourism:Period"
            },
            "schema:domainIncludes": [
                {
                    "@id": "tourism:ExperienceEvent"
                },
                {
                    "@id": "tourism:ExperienceProduct"
                }
            ],
            "rdfs:comment": [
                "A operational period for this experience product.",
                "An operational period specified for this experience event."
            ],
            "rdfs:label": "operationalPeriod",
            "unece:cefactElementMetadata": [
                {
                    "@id": "cefact:Experience_Event.Operational.Specified_Period",
                    "@type": "unece:AssociationBIE",
                    "unece:cefactUNId": "UN01015135",
                    "unece:cefactBieDomainClass": "cefact:Experience_Event.Details",
                    "rdfs:comment": "An operational period specified for this experience event."
                },
                {
                    "@id": "cefact:Experience_Product.Operational.Specified_Period",
                    "@type": "unece:AssociationBIE",
                    "unece:cefactUNId": "UN01015178",
                    "unece:cefactBieDomainClass": "cefact:Experience_Product.Details",
                    "rdfs:comment": "A operational period for this experience product."
                }
            ]
        },
        {
            "@id": "tourism:optionalProduct",
            "@type": "rdf:Property",
            "schema:rangeIncludes": {
                "@id": "tourism:Product"
            },
            "schema:domainIncludes": {
                "@id": "tourism:ExperienceProduct"
            },
            "rdfs:comment": "An optional product for this experience product.",
            "rdfs:label": "optionalProduct",
            "unece:cefactElementMetadata": [
                {
                    "@id": "cefact:Experience_Product.Optional.Experience_Product",
                    "@type": "unece:AssociationBIE",
                    "unece:cefactUNId": "UN01015174",
                    "unece:cefactBieDomainClass": "cefact:Experience_Product.Details",
                    "rdfs:comment": "An optional product for this experience product."
                }
            ]
        },
        {
            "@id": "tourism:originalConstructionDate",
            "@type": "rdf:Property",
            "schema:rangeIncludes": {
                "@id": "xsd:base64Binary"
            },
            "schema:domainIncludes": {
                "@id": "tourism:LodgingHouseBuilding"
            },
            "rdfs:comment": "The date of the original construction of this lodging house building.",
            "rdfs:label": "originalConstructionDate",
            "unece:cefactElementMetadata": [
                {
                    "@id": "cefact:LodgingHouse_Building.Original_Construction.Date",
                    "@type": "unece:BasicBIE",
                    "unece:cefactUNId": "UN01001042",
                    "unece:cefactBieDomainClass": "cefact:LodgingHouse_Building.Details",
                    "rdfs:comment": "The date of the original construction of this lodging house building."
                }
            ]
        },
        {
            "@id": "tourism:ownerName",
            "@type": "rdf:Property",
            "schema:rangeIncludes": {
                "@id": "xsd:string"
            },
            "schema:domainIncludes": {
                "@id": "tourism:LodgingHouseOrganization"
            },
            "rdfs:comment": "The name of the company or individual, expressed as text, who is the owner of this lodging house organization.",
            "rdfs:label": "ownerName",
            "unece:cefactElementMetadata": [
                {
                    "@id": "cefact:LodgingHouse_Organization.Owner_Name.Text",
                    "@type": "unece:BasicBIE",
                    "unece:cefactUNId": "UN01001035",
                    "unece:cefactBieDomainClass": "cefact:LodgingHouse_Organization.Details",
                    "rdfs:comment": "The name of the company or individual, expressed as text, who is the owner of this lodging house organization."
                }
            ]
        },
        {
            "@id": "tourism:passportId",
            "@type": "rdf:Property",
            "schema:rangeIncludes": {
                "@id": "xsd:token"
            },
            "schema:domainIncludes": {
                "@id": "tourism:GuestPerson"
            },
            "rdfs:comment": "The identifier of the passport of this guest.",
            "rdfs:label": "passportId",
            "unece:cefactElementMetadata": [
                {
                    "@id": "cefact:Guest_Person.Passport.Identifier",
                    "@type": "unece:BasicBIE",
                    "unece:TDED": "1194",
                    "unece:cefactUNId": "UN01009716",
                    "unece:cefactBieDomainClass": "cefact:Guest_Person.Details",
                    "rdfs:comment": "The identifier of the passport of this guest."
                }
            ]
        },
        {
            "@id": "tourism:personName",
            "@type": "rdf:Property",
            "schema:rangeIncludes": {
                "@id": "xsd:string"
            },
            "schema:domainIncludes": {
                "@id": "tourism:LodgingHouseContact"
            },
            "rdfs:comment": "The name, expressed as text, of this contact person for this lodging house.",
            "rdfs:label": "personName",
            "unece:cefactElementMetadata": [
                {
                    "@id": "cefact:LodgingHouse_Contact.PersonName.Text",
                    "@type": "unece:BasicBIE",
                    "unece:TDED": "3412",
                    "unece:cefactUNId": "UN01001227",
                    "unece:cefactBieDomainClass": "cefact:LodgingHouse_Contact.Details",
                    "rdfs:comment": "The name, expressed as text, of this contact person for this lodging house."
                }
            ]
        },
        {
            "@id": "tourism:physicalCharacteristic",
            "@type": "rdf:Property",
            "schema:rangeIncludes": {
                "@id": "xsd:string"
            },
            "schema:domainIncludes": {
                "@id": "tourism:LodgingHouseUsageCondition"
            },
            "rdfs:comment": "The physical characteristic limitation, expressed as text, applicable to this lodging house usage condition.",
            "rdfs:label": "physicalCharacteristic",
            "unece:cefactElementMetadata": [
                {
                    "@id": "cefact:LodgingHouse_UsageCondition.PhysicalCharacteristic.Text",
                    "@type": "unece:BasicBIE",
                    "unece:cefactUNId": "UN01001207",
                    "unece:cefactBieDomainClass": "cefact:LodgingHouse_UsageCondition.Details",
                    "rdfs:comment": "The physical characteristic limitation, expressed as text, applicable to this lodging house usage condition."
                }
            ]
        },
        {
            "@id": "tourism:physicalLocation",
            "@type": "rdf:Property",
            "schema:rangeIncludes": {
                "@id": "tourism:Location"
            },
            "schema:domainIncludes": [
                {
                    "@id": "tourism:BathingFacility"
                },
                {
                    "@id": "tourism:BusinessSupportRoomFacility"
                },
                {
                    "@id": "tourism:ExperienceFacility"
                },
                {
                    "@id": "tourism:GuestRoomFacility"
                },
                {
                    "@id": "tourism:LodgingHouseTravelProductSubComponent"
                }
            ],
            "rdfs:comment": [
                "A physical location specified for this experience facility.",
                "The lodging house physical location for this lodging house travel product sub-component.",
                "The physical location of this bathing facility at this lodging house.",
                "The physical location of this business support room at this lodging house.",
                "The physical location of this guest room at this lodging house."
            ],
            "rdfs:label": "physicalLocation",
            "unece:cefactElementMetadata": [
                {
                    "@id": "cefact:Bathing_Facility.Physical.LodgingHouse_Location",
                    "@type": "unece:AssociationBIE",
                    "unece:cefactUNId": "UN01001069",
                    "unece:cefactBieDomainClass": "cefact:Bathing_Facility.Details",
                    "rdfs:comment": "The physical location of this bathing facility at this lodging house."
                },
                {
                    "@id": "cefact:Experience_Facility.Physical.Specified_Location",
                    "@type": "unece:AssociationBIE",
                    "unece:cefactUNId": "UN01015148",
                    "unece:cefactBieDomainClass": "cefact:Experience_Facility.Details",
                    "rdfs:comment": "A physical location specified for this experience facility."
                },
                {
                    "@id": "cefact:GuestRoom_Facility.Physical.LodgingHouse_Location",
                    "@type": "unece:AssociationBIE",
                    "unece:cefactUNId": "UN01001055",
                    "unece:cefactBieDomainClass": "cefact:GuestRoom_Facility.Details",
                    "rdfs:comment": "The physical location of this guest room at this lodging house."
                },
                {
                    "@id": "cefact:LodgingHouse_TravelProductSub-Component.Physical.LodgingHouse_Location",
                    "@type": "unece:AssociationBIE",
                    "unece:cefactUNId": "UN01004998",
                    "unece:cefactBieDomainClass": "cefact:LodgingHouse_TravelProductSubComponent.Details",
                    "rdfs:comment": "The lodging house physical location for this lodging house travel product sub-component."
                },
                {
                    "@id": "cefact:BusinessSupportRoom_Facility.Physical.LodgingHouse_Location",
                    "@type": "unece:AssociationBIE",
                    "unece:cefactUNId": "UN01001112",
                    "unece:cefactBieDomainClass": "cefact:BusinessSupportRoom_Facility.Details",
                    "rdfs:comment": "The physical location of this business support room at this lodging house."
                }
            ]
        },
        {
            "@id": "tourism:postalAddress",
            "@type": "rdf:Property",
            "schema:rangeIncludes": {
                "@id": "tourism:Address"
            },
            "schema:domainIncludes": {
                "@id": "tourism:LodgingHouseContact"
            },
            "rdfs:comment": "A structured postal address for this lodging house contact.",
            "rdfs:label": "postalAddress",
            "unece:cefactElementMetadata": [
                {
                    "@id": "cefact:LodgingHouse_Contact.Postal.Structured_Address",
                    "@type": "unece:AssociationBIE",
                    "unece:cefactUNId": "UN01001231",
                    "unece:cefactBieDomainClass": "cefact:LodgingHouse_Contact.Details",
                    "rdfs:comment": "A structured postal address for this lodging house contact."
                }
            ]
        },
        {
            "@id": "tourism:preferredItem",
            "@type": "rdf:Property",
            "schema:rangeIncludes": {
                "@id": "xsd:string"
            },
            "schema:domainIncludes": {
                "@id": "tourism:ExperienceItemPreference"
            },
            "rdfs:comment": "A preferred item, expressed as text, for this experience item preference.",
            "rdfs:label": "preferredItem",
            "unece:cefactElementMetadata": [
                {
                    "@id": "cefact:ExperienceItem_Preference.Preferred_Item.Text",
                    "@type": "unece:BasicBIE",
                    "unece:cefactUNId": "UN01015151",
                    "unece:cefactBieDomainClass": "cefact:ExperienceItem_Preference.Details",
                    "rdfs:comment": "A preferred item, expressed as text, for this experience item preference."
                }
            ]
        },
        {
            "@id": "tourism:primaryIndicator",
            "@type": "rdf:Property",
            "schema:rangeIncludes": {
                "@id": "xsd:boolean"
            },
            "schema:domainIncludes": {
                "@id": "tourism:LodgingHouseContact"
            },
            "rdfs:comment": "The indication of whether or not this is the primary contact for this lodging house.",
            "rdfs:label": "primaryIndicator",
            "unece:cefactElementMetadata": [
                {
                    "@id": "cefact:LodgingHouse_Contact.Primary.Indicator",
                    "@type": "unece:BasicBIE",
                    "unece:cefactUNId": "UN01001228",
                    "unece:cefactBieDomainClass": "cefact:LodgingHouse_Contact.Details",
                    "rdfs:comment": "The indication of whether or not this is the primary contact for this lodging house."
                }
            ]
        },
        {
            "@id": "tourism:priorityRankingNumeric",
            "@type": "rdf:Property",
            "schema:rangeIncludes": {
                "@id": "xsd:decimal"
            },
            "schema:domainIncludes": {
                "@id": "tourism:ExperienceItemPreference"
            },
            "rdfs:comment": "The priority ranking number for this experience item preference.",
            "rdfs:label": "priorityRankingNumeric",
            "unece:cefactElementMetadata": [
                {
                    "@id": "cefact:ExperienceItem_Preference.Priority_Ranking.Numeric",
                    "@type": "unece:BasicBIE",
                    "unece:cefactUNId": "UN01015153",
                    "unece:cefactBieDomainClass": "cefact:ExperienceItem_Preference.Details",
                    "rdfs:comment": "The priority ranking number for this experience item preference."
                }
            ]
        },
        {
            "@id": "tourism:productEndTime",
            "@type": "rdf:Property",
            "schema:rangeIncludes": {
                "@id": "xsd:time"
            },
            "schema:domainIncludes": {
                "@id": "tourism:ProductComponentItinerary"
            },
            "rdfs:comment": "The end time of the product for this product component itinerary.",
            "rdfs:label": "productEndTime",
            "unece:cefactElementMetadata": [
                {
                    "@id": "cefact:ProductComponent_Itinerary.ProductEnd.Time",
                    "@type": "unece:BasicBIE",
                    "unece:cefactUNId": "UN01004982",
                    "unece:cefactBieDomainClass": "cefact:ProductComponent_Itinerary.Details",
                    "rdfs:comment": "The end time of the product for this product component itinerary."
                }
            ]
        },
        {
            "@id": "tourism:productStartTime",
            "@type": "rdf:Property",
            "schema:rangeIncludes": {
                "@id": "xsd:time"
            },
            "schema:domainIncludes": {
                "@id": "tourism:ProductComponentItinerary"
            },
            "rdfs:comment": "The start time of the product for this product component itinerary.",
            "rdfs:label": "productStartTime",
            "unece:cefactElementMetadata": [
                {
                    "@id": "cefact:ProductComponent_Itinerary.ProductStart.Time",
                    "@type": "unece:BasicBIE",
                    "unece:cefactUNId": "UN01004981",
                    "unece:cefactBieDomainClass": "cefact:ProductComponent_Itinerary.Details",
                    "rdfs:comment": "The start time of the product for this product component itinerary."
                }
            ]
        },
        {
            "@id": "tourism:propertyConfirmationId",
            "@type": "rdf:Property",
            "schema:rangeIncludes": {
                "@id": "xsd:token"
            },
            "schema:domainIncludes": {
                "@id": "tourism:LodgingHouseReservation"
            },
            "rdfs:comment": "The identifier of the property confirmation for this lodging house reservation.",
            "rdfs:label": "propertyConfirmationId",
            "unece:cefactElementMetadata": [
                {
                    "@id": "cefact:LodgingHouse_Reservation.PropertyConfirmation.Identifier",
                    "@type": "unece:BasicBIE",
                    "unece:cefactUNId": "UN01009796",
                    "unece:cefactBieDomainClass": "cefact:LodgingHouse_Reservation.Details",
                    "rdfs:comment": "The identifier of the property confirmation for this lodging house reservation."
                }
            ]
        },
        {
            "@id": "tourism:propertyConfirmationIssuedDateTime",
            "@type": "rdf:Property",
            "schema:rangeIncludes": {
                "@id": "xsd:dateTime"
            },
            "schema:domainIncludes": {
                "@id": "tourism:LodgingHouseReservation"
            },
            "rdfs:comment": "The date, time, date time, or other date time value when the property confirmation is issued for this lodging house reservation.",
            "rdfs:label": "propertyConfirmationIssuedDateTime",
            "unece:cefactElementMetadata": [
                {
                    "@id": "cefact:LodgingHouse_Reservation.PropertyConfirmationIssued.DateTime",
                    "@type": "unece:BasicBIE",
                    "unece:cefactUNId": "UN01009797",
                    "unece:cefactBieDomainClass": "cefact:LodgingHouse_Reservation.Details",
                    "rdfs:comment": "The date, time, date time, or other date time value when the property confirmation is issued for this lodging house reservation."
                }
            ]
        },
        {
            "@id": "tourism:providedCertificate",
            "@type": "rdf:Property",
            "schema:rangeIncludes": {
                "@id": "tourism:Certificate"
            },
            "schema:domainIncludes": [
                {
                    "@id": "tourism:ExperienceEvent"
                },
                {
                    "@id": "tourism:ExperienceProduct"
                }
            ],
            "rdfs:comment": [
                "A certificate provided for this experience product.",
                "A specified certificate provided for this experience event."
            ],
            "rdfs:label": "providedCertificate",
            "unece:cefactElementMetadata": [
                {
                    "@id": "cefact:Experience_Event.Provided.Specified_Certificate",
                    "@type": "unece:AssociationBIE",
                    "unece:cefactUNId": "UN01015133",
                    "unece:cefactBieDomainClass": "cefact:Experience_Event.Details",
                    "rdfs:comment": "A specified certificate provided for this experience event."
                },
                {
                    "@id": "cefact:Experience_Product.Provided.Specified_Certificate",
                    "@type": "unece:AssociationBIE",
                    "unece:cefactUNId": "UN01015175",
                    "unece:cefactBieDomainClass": "cefact:Experience_Product.Details",
                    "rdfs:comment": "A certificate provided for this experience product."
                }
            ]
        },
        {
            "@id": "tourism:providedGuestArrival",
            "@type": "rdf:Property",
            "schema:rangeIncludes": {
                "@id": "tourism:GuestArrival"
            },
            "schema:domainIncludes": {
                "@id": "tourism:LodgingHouseTraveller"
            },
            "rdfs:comment": "The arrival information provided for this lodging house traveller.",
            "rdfs:label": "providedGuestArrival",
            "unece:cefactElementMetadata": [
                {
                    "@id": "cefact:LodgingHouse_Traveller.Provided.Travel_GuestArrival",
                    "@type": "unece:AssociationBIE",
                    "unece:cefactUNId": "UN01009818",
                    "unece:cefactBieDomainClass": "cefact:LodgingHouse_Traveller.Details",
                    "rdfs:comment": "The arrival information provided for this lodging house traveller."
                }
            ]
        },
        {
            "@id": "tourism:providedRequirement",
            "@type": "rdf:Property",
            "schema:rangeIncludes": {
                "@id": "tourism:Requirement"
            },
            "schema:domainIncludes": [
                {
                    "@id": "tourism:ExperienceEvent"
                },
                {
                    "@id": "tourism:ExperienceProduct"
                }
            ],
            "rdfs:comment": [
                "A requirement provided for this experience product.",
                "A specified requirement provided for this experience event."
            ],
            "rdfs:label": "providedRequirement",
            "unece:cefactElementMetadata": [
                {
                    "@id": "cefact:Experience_Product.Provided.Specified_Requirement",
                    "@type": "unece:AssociationBIE",
                    "unece:cefactUNId": "UN01015176",
                    "unece:cefactBieDomainClass": "cefact:Experience_Product.Details",
                    "rdfs:comment": "A requirement provided for this experience product."
                },
                {
                    "@id": "cefact:Experience_Event.Provided.Specified_Requirement",
                    "@type": "unece:AssociationBIE",
                    "unece:cefactUNId": "UN01015129",
                    "unece:cefactBieDomainClass": "cefact:Experience_Event.Details",
                    "rdfs:comment": "A specified requirement provided for this experience event."
                }
            ]
        },
        {
            "@id": "tourism:raisedQuery",
            "@type": "rdf:Property",
            "schema:rangeIncludes": {
                "@id": "tourism:Query"
            },
            "schema:domainIncludes": {
                "@id": "tourism:GuestPerson"
            },
            "rdfs:comment": "A special query raised for this guest person.",
            "rdfs:label": "raisedQuery",
            "unece:cefactElementMetadata": [
                {
                    "@id": "cefact:Guest_Person.Raised.Special_Query",
                    "@type": "unece:AssociationBIE",
                    "unece:cefactUNId": "UN01015222",
                    "unece:cefactBieDomainClass": "cefact:Guest_Person.Details",
                    "rdfs:comment": "A special query raised for this guest person."
                }
            ]
        },
        {
            "@id": "tourism:reasonApplicableQuantity",
            "@type": "rdf:Property",
            "schema:rangeIncludes": {
                "@id": "xsd:decimal"
            },
            "schema:domainIncludes": [
                {
                    "@id": "tourism:DiscountPrice"
                },
                {
                    "@id": "tourism:ExtraPrice"
                }
            ],
            "rdfs:comment": [
                "The number applicable to the reason for this discount price.",
                "The number applicable to the reason for this extra price."
            ],
            "rdfs:label": "reasonApplicableQuantity",
            "unece:cefactElementMetadata": [
                {
                    "@id": "cefact:Extra_Price.ReasonApplicable.Quantity",
                    "@type": "unece:BasicBIE",
                    "unece:cefactUNId": "UN01005028",
                    "unece:cefactBieDomainClass": "cefact:Extra_Price.Details",
                    "rdfs:comment": "The number applicable to the reason for this extra price."
                },
                {
                    "@id": "cefact:Discount_Price.ReasonApplicable.Quantity",
                    "@type": "unece:BasicBIE",
                    "unece:cefactUNId": "UN01005047",
                    "unece:cefactBieDomainClass": "cefact:Discount_Price.Details",
                    "rdfs:comment": "The number applicable to the reason for this discount price."
                }
            ]
        },
        {
            "@id": "tourism:reasonCode",
            "@type": "rdf:Property",
            "schema:rangeIncludes": {
                "@id": "xsd:token"
            },
            "schema:domainIncludes": [
                {
                    "@id": "tourism:DiscountPrice"
                },
                {
                    "@id": "tourism:ExtraPrice"
                }
            ],
            "rdfs:comment": [
                "The code specifying the reason for this discount price.",
                "The code specifying the reason for this extra price."
            ],
            "rdfs:label": "reasonCode",
            "unece:cefactElementMetadata": [
                {
                    "@id": "cefact:Extra_Price.Reason.Code",
                    "@type": "unece:BasicBIE",
                    "unece:cefactUNId": "UN01005027",
                    "unece:cefactBieDomainClass": "cefact:Extra_Price.Details",
                    "rdfs:comment": "The code specifying the reason for this extra price."
                },
                {
                    "@id": "cefact:Discount_Price.Reason.Code",
                    "@type": "unece:BasicBIE",
                    "unece:cefactUNId": "UN01005046",
                    "unece:cefactBieDomainClass": "cefact:Discount_Price.Details",
                    "rdfs:comment": "The code specifying the reason for this discount price."
                }
            ]
        },
        {
            "@id": "tourism:registeredDateTime",
            "@type": "rdf:Property",
            "schema:rangeIncludes": {
                "@id": "xsd:dateTime"
            },
            "schema:domainIncludes": {
                "@id": "tourism:GuestDisability"
            },
            "rdfs:comment": "The date, time, date time, or other date time value when this guest disability has been registered.",
            "rdfs:label": "registeredDateTime",
            "unece:cefactElementMetadata": [
                {
                    "@id": "cefact:Guest_Disability.Registered.DateTime",
                    "@type": "unece:BasicBIE",
                    "unece:cefactUNId": "UN01015205",
                    "unece:cefactBieDomainClass": "cefact:Guest_Disability.Details",
                    "rdfs:comment": "The date, time, date time, or other date time value when this guest disability has been registered."
                }
            ]
        },
        {
            "@id": "tourism:requestedTravelProduct",
            "@type": "rdf:Property",
            "schema:rangeIncludes": {
                "@id": "tourism:TravelProduct"
            },
            "schema:domainIncludes": {
                "@id": "tourism:LodgingHouseTraveller"
            },
            "rdfs:comment": "The travel product requested by this lodging house traveller.",
            "rdfs:label": "requestedTravelProduct",
            "unece:cefactElementMetadata": [
                {
                    "@id": "cefact:LodgingHouse_Traveller.Requested.LodgingHouse_TravelProduct",
                    "@type": "unece:AssociationBIE",
                    "unece:cefactUNId": "UN01009817",
                    "unece:cefactBieDomainClass": "cefact:LodgingHouse_Traveller.Details",
                    "rdfs:comment": "The travel product requested by this lodging house traveller."
                }
            ]
        },
        {
            "@id": "tourism:requiredReservationGuaranteeIndicator",
            "@type": "rdf:Property",
            "schema:rangeIncludes": {
                "@id": "xsd:boolean"
            },
            "schema:domainIncludes": {
                "@id": "tourism:ExperienceProduct"
            },
            "rdfs:comment": "The indication of whether or not this experience product requires a reservation guarantee.",
            "rdfs:label": "requiredReservationGuaranteeIndicator",
            "unece:cefactElementMetadata": [
                {
                    "@id": "cefact:Experience_Product.RequiredReservation_Guarantee.Indicator",
                    "@type": "unece:BasicBIE",
                    "unece:cefactUNId": "UN01015172",
                    "unece:cefactBieDomainClass": "cefact:Experience_Product.Details",
                    "rdfs:comment": "The indication of whether or not this experience product requires a reservation guarantee."
                }
            ]
        },
        {
            "@id": "tourism:requiredSupportingDevice",
            "@type": "rdf:Property",
            "schema:rangeIncludes": {
                "@id": "xsd:string"
            },
            "schema:domainIncludes": {
                "@id": "tourism:GuestDisability"
            },
            "rdfs:comment": "A supporting device, expressed as text, required for this guest disability.",
            "rdfs:label": "requiredSupportingDevice",
            "unece:cefactElementMetadata": [
                {
                    "@id": "cefact:Guest_Disability.Required_SupportingDevice.Text",
                    "@type": "unece:BasicBIE",
                    "unece:cefactUNId": "UN01015203",
                    "unece:cefactBieDomainClass": "cefact:Guest_Disability.Details",
                    "rdfs:comment": "A supporting device, expressed as text, required for this guest disability."
                }
            ]
        },
        {
            "@id": "tourism:requiredUsageCondition",
            "@type": "rdf:Property",
            "schema:rangeIncludes": {
                "@id": "tourism:UsageCondition"
            },
            "schema:domainIncludes": [
                {
                    "@id": "tourism:ExperienceEvent"
                },
                {
                    "@id": "tourism:ExperienceProduct"
                }
            ],
            "rdfs:comment": [
                "A required usage condition for this experience product.",
                "The specified usage condition required for this experience event."
            ],
            "rdfs:label": "requiredUsageCondition",
            "unece:cefactElementMetadata": [
                {
                    "@id": "cefact:Experience_Product.Required.Specified_UsageCondition",
                    "@type": "unece:AssociationBIE",
                    "unece:cefactUNId": "UN01015179",
                    "unece:cefactBieDomainClass": "cefact:Experience_Product.Details",
                    "rdfs:comment": "A required usage condition for this experience product."
                },
                {
                    "@id": "cefact:Experience_Event.Required.Specified_UsageCondition",
                    "@type": "unece:AssociationBIE",
                    "unece:cefactUNId": "UN01015130",
                    "unece:cefactBieDomainClass": "cefact:Experience_Event.Details",
                    "rdfs:comment": "The specified usage condition required for this experience event."
                }
            ]
        },
        {
            "@id": "tourism:reservationGuarantee",
            "@type": "rdf:Property",
            "schema:rangeIncludes": {
                "@id": "xsd:string"
            },
            "schema:domainIncludes": [
                {
                    "@id": "tourism:ExperienceEvent"
                },
                {
                    "@id": "tourism:ExperienceProduct"
                },
                {
                    "@id": "tourism:LodgingHouseTravelProduct"
                }
            ],
            "rdfs:comment": [
                "A reservation guarantee, expressed as text, for this experience event.",
                "A reservation guarantee, expressed as text, for this experience product.",
                "The reservation guarantee, expressed as text, for this lodging house travel product."
            ],
            "rdfs:label": "reservationGuarantee",
            "unece:cefactElementMetadata": [
                {
                    "@id": "cefact:Experience_Event.Reservation_Guarantee.Text",
                    "@type": "unece:BasicBIE",
                    "unece:cefactUNId": "UN01015126",
                    "unece:cefactBieDomainClass": "cefact:Experience_Event.Details",
                    "rdfs:comment": "A reservation guarantee, expressed as text, for this experience event."
                },
                {
                    "@id": "cefact:Experience_Product.Reservation_Guarantee.Text",
                    "@type": "unece:BasicBIE",
                    "unece:cefactUNId": "UN01015165",
                    "unece:cefactBieDomainClass": "cefact:Experience_Product.Details",
                    "rdfs:comment": "A reservation guarantee, expressed as text, for this experience product."
                },
                {
                    "@id": "cefact:LodgingHouse_TravelProduct.ReservationGuarantee.Text",
                    "@type": "unece:BasicBIE",
                    "unece:cefactUNId": "UN01004927",
                    "unece:cefactBieDomainClass": "cefact:LodgingHouse_TravelProduct.Details",
                    "rdfs:comment": "The reservation guarantee, expressed as text, for this lodging house travel product."
                }
            ]
        },
        {
            "@id": "tourism:reservationGuaranteeRequiredIndicator",
            "@type": "rdf:Property",
            "schema:rangeIncludes": {
                "@id": "xsd:boolean"
            },
            "schema:domainIncludes": {
                "@id": "tourism:LodgingHouseTravelProduct"
            },
            "rdfs:comment": "The indication of whether or not this lodging house travel product requires a reservation guarantee.",
            "rdfs:label": "reservationGuaranteeRequiredIndicator",
            "unece:cefactElementMetadata": [
                {
                    "@id": "cefact:LodgingHouse_TravelProduct.ReservationGuaranteeRequired.Indicator",
                    "@type": "unece:BasicBIE",
                    "unece:cefactUNId": "UN01004926",
                    "unece:cefactBieDomainClass": "cefact:LodgingHouse_TravelProduct.Details",
                    "rdfs:comment": "The indication of whether or not this lodging house travel product requires a reservation guarantee."
                }
            ]
        },
        {
            "@id": "tourism:reservationRequiredIndicator",
            "@type": "rdf:Property",
            "schema:rangeIncludes": {
                "@id": "xsd:boolean"
            },
            "schema:domainIncludes": [
                {
                    "@id": "tourism:ExperienceEvent"
                },
                {
                    "@id": "tourism:LodgingHouseUsageCondition"
                }
            ],
            "rdfs:comment": [
                "The indication of whether or not a reservation is required for this experience event.",
                "The indication of whether or not this lodging house usage condition requires a reservation."
            ],
            "rdfs:label": "reservationRequiredIndicator",
            "unece:cefactElementMetadata": [
                {
                    "@id": "cefact:Experience_Event.Reservation_Required.Indicator",
                    "@type": "unece:BasicBIE",
                    "unece:cefactUNId": "UN01015121",
                    "unece:cefactBieDomainClass": "cefact:Experience_Event.Details",
                    "rdfs:comment": "The indication of whether or not a reservation is required for this experience event."
                },
                {
                    "@id": "cefact:LodgingHouse_UsageCondition.Reservation_Required.Indicator",
                    "@type": "unece:BasicBIE",
                    "unece:cefactUNId": "UN01001202",
                    "unece:cefactBieDomainClass": "cefact:LodgingHouse_UsageCondition.Details",
                    "rdfs:comment": "The indication of whether or not this lodging house usage condition requires a reservation."
                }
            ]
        },
        {
            "@id": "tourism:reservationStatusCode",
            "@type": "rdf:Property",
            "schema:rangeIncludes": {
                "@id": "xsd:token"
            },
            "schema:domainIncludes": {
                "@id": "tourism:LodgingHouseTraveller"
            },
            "rdfs:comment": "The code specifying the reservation status of this lodging house traveller.",
            "rdfs:label": "reservationStatusCode",
            "unece:cefactElementMetadata": [
                {
                    "@id": "cefact:LodgingHouse_Traveller.ReservationStatus.Code",
                    "@type": "unece:BasicBIE",
                    "unece:cefactUNId": "UN01009813",
                    "unece:cefactBieDomainClass": "cefact:LodgingHouse_Traveller.Details",
                    "rdfs:comment": "The code specifying the reservation status of this lodging house traveller."
                }
            ]
        },
        {
            "@id": "tourism:residenceCountryId",
            "@type": "rdf:Property",
            "schema:rangeIncludes": {
                "@id": "xsd:token"
            },
            "schema:domainIncludes": {
                "@id": "tourism:GuestPerson"
            },
            "rdfs:comment": "The identifier of the residence country of this guest person.",
            "rdfs:label": "residenceCountryId",
            "unece:cefactElementMetadata": [
                {
                    "@id": "cefact:Guest_Person.ResidenceCountry.Identifier",
                    "@type": "unece:BasicBIE",
                    "unece:cefactUNId": "UN01015220",
                    "unece:cefactBieDomainClass": "cefact:Guest_Person.Details",
                    "rdfs:comment": "The identifier of the residence country of this guest person."
                }
            ]
        },
        {
            "@id": "tourism:responsibility",
            "@type": "rdf:Property",
            "schema:rangeIncludes": {
                "@id": "xsd:string"
            },
            "schema:domainIncludes": {
                "@id": "tourism:LodgingHouseContact"
            },
            "rdfs:comment": "The responsibility, expressed as text, of this lodging house contact.",
            "rdfs:label": "responsibility",
            "unece:cefactElementMetadata": [
                {
                    "@id": "cefact:LodgingHouse_Contact.Responsibility.Text",
                    "@type": "unece:BasicBIE",
                    "unece:cefactUNId": "UN01001224",
                    "unece:cefactBieDomainClass": "cefact:LodgingHouse_Contact.Details",
                    "rdfs:comment": "The responsibility, expressed as text, of this lodging house contact."
                }
            ]
        },
        {
            "@id": "tourism:restriction",
            "@type": "rdf:Property",
            "schema:rangeIncludes": {
                "@id": "xsd:string"
            },
            "schema:domainIncludes": [
                {
                    "@id": "tourism:GuestAllergy"
                },
                {
                    "@id": "tourism:GuestCarriedEquipment"
                },
                {
                    "@id": "tourism:GuestDisability"
                },
                {
                    "@id": "tourism:GuestFoodChoice"
                },
                {
                    "@id": "tourism:GuestHealthIndication"
                }
            ],
            "rdfs:comment": [
                "A restriction, expressed as text, for this guest carried equipment.",
                "A restriction, expressed as text, for this guest disability.",
                "A restriction, expressed as text, for this guest food choice.",
                "A restriction, expressed as text, for this guest health indication.",
                "A restriction, expressed as text, related to this guest allergy."
            ],
            "rdfs:label": "restriction",
            "unece:cefactElementMetadata": [
                {
                    "@id": "cefact:Guest_CarriedEquipment.Restriction.Text",
                    "@type": "unece:BasicBIE",
                    "unece:cefactUNId": "UN01015197",
                    "unece:cefactBieDomainClass": "cefact:Guest_CarriedEquipment.Details",
                    "rdfs:comment": "A restriction, expressed as text, for this guest carried equipment."
                },
                {
                    "@id": "cefact:Guest_Disability.Restriction.Text",
                    "@type": "unece:BasicBIE",
                    "unece:cefactUNId": "UN01015204",
                    "unece:cefactBieDomainClass": "cefact:Guest_Disability.Details",
                    "rdfs:comment": "A restriction, expressed as text, for this guest disability."
                },
                {
                    "@id": "cefact:Guest_HealthIndication.Restriction.Text",
                    "@type": "unece:BasicBIE",
                    "unece:cefactUNId": "UN01015215",
                    "unece:cefactBieDomainClass": "cefact:Guest_HealthIndication.Details",
                    "rdfs:comment": "A restriction, expressed as text, for this guest health indication."
                },
                {
                    "@id": "cefact:Guest_FoodChoice.Restriction.Text",
                    "@type": "unece:BasicBIE",
                    "unece:cefactUNId": "UN01015210",
                    "unece:cefactBieDomainClass": "cefact:Guest_FoodChoice.Details",
                    "rdfs:comment": "A restriction, expressed as text, for this guest food choice."
                },
                {
                    "@id": "cefact:Guest_Allergy.Restriction.Text",
                    "@type": "unece:BasicBIE",
                    "unece:cefactUNId": "UN01015192",
                    "unece:cefactBieDomainClass": "cefact:Guest_Allergy.Details",
                    "rdfs:comment": "A restriction, expressed as text, related to this guest allergy."
                }
            ]
        },
        {
            "@id": "tourism:roleCode",
            "@type": "rdf:Property",
            "schema:rangeIncludes": {
                "@id": "xsd:token"
            },
            "schema:domainIncludes": {
                "@id": "tourism:GuestPerson"
            },
            "rdfs:comment": "The code specifying the role of this guest person.",
            "rdfs:label": "roleCode",
            "unece:cefactElementMetadata": [
                {
                    "@id": "cefact:Guest_Person.Role.Code",
                    "@type": "unece:BasicBIE",
                    "unece:cefactUNId": "UN01015218",
                    "unece:cefactBieDomainClass": "cefact:Guest_Person.Details",
                    "rdfs:comment": "The code specifying the role of this guest person."
                }
            ]
        },
        {
            "@id": "tourism:rooming",
            "@type": "rdf:Property",
            "schema:rangeIncludes": {
                "@id": "xsd:string"
            },
            "schema:domainIncludes": {
                "@id": "tourism:LodgingHouseTraveller"
            },
            "rdfs:comment": "The rooming, expressed as text, for this lodging house traveller.",
            "rdfs:label": "rooming",
            "unece:cefactElementMetadata": [
                {
                    "@id": "cefact:LodgingHouse_Traveller.Rooming.Text",
                    "@type": "unece:BasicBIE",
                    "unece:cefactUNId": "UN01009815",
                    "unece:cefactBieDomainClass": "cefact:LodgingHouse_Traveller.Details",
                    "rdfs:comment": "The rooming, expressed as text, for this lodging house traveller."
                }
            ]
        },
        {
            "@id": "tourism:salesManagerName",
            "@type": "rdf:Property",
            "schema:rangeIncludes": {
                "@id": "xsd:string"
            },
            "schema:domainIncludes": {
                "@id": "tourism:LodgingHouseTravelProduct"
            },
            "rdfs:comment": "The name, expressed as text, of the sales manager for this lodging house travel product.",
            "rdfs:label": "salesManagerName",
            "unece:cefactElementMetadata": [
                {
                    "@id": "cefact:LodgingHouse_TravelProduct.SalesManagerName.Text",
                    "@type": "unece:BasicBIE",
                    "unece:cefactUNId": "UN01004924",
                    "unece:cefactBieDomainClass": "cefact:LodgingHouse_TravelProduct.Details",
                    "rdfs:comment": "The name, expressed as text, of the sales manager for this lodging house travel product."
                }
            ]
        },
        {
            "@id": "tourism:salesOfficeInformation",
            "@type": "rdf:Property",
            "schema:rangeIncludes": {
                "@id": "xsd:string"
            },
            "schema:domainIncludes": {
                "@id": "tourism:LodgingHouseTravelProduct"
            },
            "rdfs:comment": "Sales office information, expressed as text, for this lodging house travel product.",
            "rdfs:label": "salesOfficeInformation",
            "unece:cefactElementMetadata": [
                {
                    "@id": "cefact:LodgingHouse_TravelProduct.SalesOfficeInformation.Text",
                    "@type": "unece:BasicBIE",
                    "unece:cefactUNId": "UN01004930",
                    "unece:cefactBieDomainClass": "cefact:LodgingHouse_TravelProduct.Details",
                    "rdfs:comment": "Sales office information, expressed as text, for this lodging house travel product."
                }
            ]
        },
        {
            "@id": "tourism:salesPolicyAcceptedIndicator",
            "@type": "rdf:Property",
            "schema:rangeIncludes": {
                "@id": "xsd:boolean"
            },
            "schema:domainIncludes": {
                "@id": "tourism:LodgingHouseReservation"
            },
            "rdfs:comment": "The indication of whether or not this lodging house reservation has met the sales policy.",
            "rdfs:label": "salesPolicyAcceptedIndicator",
            "unece:cefactElementMetadata": [
                {
                    "@id": "cefact:LodgingHouse_Reservation.SalesPolicyAccepted.Indicator",
                    "@type": "unece:BasicBIE",
                    "unece:cefactUNId": "UN01009795",
                    "unece:cefactBieDomainClass": "cefact:LodgingHouse_Reservation.Details",
                    "rdfs:comment": "The indication of whether or not this lodging house reservation has met the sales policy."
                }
            ]
        },
        {
            "@id": "tourism:seasonalRankCode",
            "@type": "rdf:Property",
            "schema:rangeIncludes": {
                "@id": "xsd:token"
            },
            "schema:domainIncludes": [
                {
                    "@id": "tourism:BasicPrice"
                },
                {
                    "@id": "tourism:CancellationPrice"
                },
                {
                    "@id": "tourism:DiscountPrice"
                },
                {
                    "@id": "tourism:ExtraPrice"
                }
            ],
            "rdfs:comment": [
                "The code specifying the seasonal rank of this basic price, such as peak or bottom.",
                "The code specifying the seasonal rank of this cancellation price.",
                "The code specifying the seasonal rank of this discount price.",
                "The code specifying the seasonal rank of this extra price."
            ],
            "rdfs:label": "seasonalRankCode",
            "unece:cefactElementMetadata": [
                {
                    "@id": "cefact:Cancellation_Price.Seasonal_Rank.Code",
                    "@type": "unece:BasicBIE",
                    "unece:cefactUNId": "UN01005075",
                    "unece:cefactBieDomainClass": "cefact:Cancellation_Price.Details",
                    "rdfs:comment": "The code specifying the seasonal rank of this cancellation price."
                },
                {
                    "@id": "cefact:Discount_Price.Seasonal_Rank.Code",
                    "@type": "unece:BasicBIE",
                    "unece:cefactUNId": "UN01005037",
                    "unece:cefactBieDomainClass": "cefact:Discount_Price.Details",
                    "rdfs:comment": "The code specifying the seasonal rank of this discount price."
                },
                {
                    "@id": "cefact:Extra_Price.Seasonal_Rank.Code",
                    "@type": "unece:BasicBIE",
                    "unece:cefactUNId": "UN01005018",
                    "unece:cefactBieDomainClass": "cefact:Extra_Price.Details",
                    "rdfs:comment": "The code specifying the seasonal rank of this extra price."
                },
                {
                    "@id": "cefact:Basic_Price.Seasonal_Rank.Code",
                    "@type": "unece:BasicBIE",
                    "unece:cefactUNId": "UN01005002",
                    "unece:cefactBieDomainClass": "cefact:Basic_Price.Details",
                    "rdfs:comment": "The code specifying the seasonal rank of this basic price, such as peak or bottom."
                }
            ]
        },
        {
            "@id": "tourism:sequenceId",
            "@type": "rdf:Property",
            "schema:rangeIncludes": {
                "@id": "xsd:token"
            },
            "schema:domainIncludes": {
                "@id": "tourism:LodgingHouseTraveller"
            },
            "rdfs:comment": "The sequence identifier for this lodging house traveller.",
            "rdfs:label": "sequenceId",
            "unece:cefactElementMetadata": [
                {
                    "@id": "cefact:LodgingHouse_Traveller.Sequence.Identifier",
                    "@type": "unece:BasicBIE",
                    "unece:cefactUNId": "UN01009811",
                    "unece:cefactBieDomainClass": "cefact:LodgingHouse_Traveller.Details",
                    "rdfs:comment": "The sequence identifier for this lodging house traveller."
                }
            ]
        },
        {
            "@id": "tourism:serviceChargeAmount",
            "@type": "rdf:Property",
            "schema:rangeIncludes": {
                "@id": "xsd:decimal"
            },
            "schema:domainIncludes": {
                "@id": "tourism:DailyPrice"
            },
            "rdfs:comment": "The monetary value of the service charge on which this daily price is calculated.",
            "rdfs:label": "serviceChargeAmount",
            "unece:cefactElementMetadata": [
                {
                    "@id": "cefact:Daily_Price.Service_Charge.Amount",
                    "@type": "unece:BasicBIE",
                    "unece:cefactUNId": "UN01009693",
                    "unece:cefactBieDomainClass": "cefact:Daily_Price.Details",
                    "rdfs:comment": "The monetary value of the service charge on which this daily price is calculated."
                }
            ]
        },
        {
            "@id": "tourism:serviceChargeApplicableIndicator",
            "@type": "rdf:Property",
            "schema:rangeIncludes": {
                "@id": "xsd:boolean"
            },
            "schema:domainIncludes": [
                {
                    "@id": "tourism:BasicPrice"
                },
                {
                    "@id": "tourism:DiscountPrice"
                },
                {
                    "@id": "tourism:ExtraPrice"
                }
            ],
            "rdfs:comment": [
                "The indication of whether or not a service charge is applicable to the basic price.",
                "The indication of whether or not a service charge is applicable to the discount price.",
                "The indication of whether or not a service charge is applicable to the extra price."
            ],
            "rdfs:label": "serviceChargeApplicableIndicator",
            "unece:cefactElementMetadata": [
                {
                    "@id": "cefact:Basic_Price.Service_ChargeApplicable.Indicator",
                    "@type": "unece:BasicBIE",
                    "unece:cefactUNId": "UN01005007",
                    "unece:cefactBieDomainClass": "cefact:Basic_Price.Details",
                    "rdfs:comment": "The indication of whether or not a service charge is applicable to the basic price."
                },
                {
                    "@id": "cefact:Extra_Price.Service_ChargeApplicable.Indicator",
                    "@type": "unece:BasicBIE",
                    "unece:cefactUNId": "UN01005023",
                    "unece:cefactBieDomainClass": "cefact:Extra_Price.Details",
                    "rdfs:comment": "The indication of whether or not a service charge is applicable to the extra price."
                },
                {
                    "@id": "cefact:Discount_Price.Service_ChargeApplicable.Indicator",
                    "@type": "unece:BasicBIE",
                    "unece:cefactUNId": "UN01005042",
                    "unece:cefactBieDomainClass": "cefact:Discount_Price.Details",
                    "rdfs:comment": "The indication of whether or not a service charge is applicable to the discount price."
                }
            ]
        },
        {
            "@id": "tourism:situatedAtSource",
            "@type": "rdf:Property",
            "schema:rangeIncludes": {
                "@id": "tourism:Source"
            },
            "schema:domainIncludes": {
                "@id": "tourism:BathingFacility"
            },
            "rdfs:comment": "A hot springs natural source that is situated in this bathing facility.",
            "rdfs:label": "situatedAtSource",
            "unece:cefactElementMetadata": [
                {
                    "@id": "cefact:Bathing_Facility.SituatedAt.HotSprings_Source",
                    "@type": "unece:AssociationBIE",
                    "unece:cefactUNId": "UN01001072",
                    "unece:cefactBieDomainClass": "cefact:Bathing_Facility.Details",
                    "rdfs:comment": "A hot springs natural source that is situated in this bathing facility."
                }
            ]
        },
        {
            "@id": "tourism:specialBeddingServiceOfferedIndicator",
            "@type": "rdf:Property",
            "schema:rangeIncludes": {
                "@id": "xsd:boolean"
            },
            "schema:domainIncludes": [
                {
                    "@id": "tourism:CustomerClass"
                },
                {
                    "@id": "tourism:LodgingHouseCustomerClass"
                }
            ],
            "rdfs:comment": [
                "The indication of whether or not special bedding service is offered for a customer class.",
                "The indication of whether or not special bedding service is offered for this lodging house customer class."
            ],
            "rdfs:label": "specialBeddingServiceOfferedIndicator",
            "unece:cefactElementMetadata": [
                {
                    "@id": "cefact:CustomerClass.SpecialBeddingServiceOffered.Indicator",
                    "@type": "unece:BasicBIE",
                    "unece:cefactUNId": "UN01004952",
                    "unece:cefactBieDomainClass": "cefact:CustomerClass.Details",
                    "rdfs:comment": "The indication of whether or not special bedding service is offered for a customer class."
                },
                {
                    "@id": "cefact:LodgingHouse_CustomerClass.SpecialBeddingServiceOffered.Indicator",
                    "@type": "unece:BasicBIE",
                    "unece:cefactUNId": "UN01010036",
                    "unece:cefactBieDomainClass": "cefact:LodgingHouse_CustomerClass.Details",
                    "rdfs:comment": "The indication of whether or not special bedding service is offered for this lodging house customer class."
                }
            ]
        },
        {
            "@id": "tourism:specificationNote",
            "@type": "rdf:Property",
            "schema:rangeIncludes": {
                "@id": "tourism:Note"
            },
            "schema:domainIncludes": {
                "@id": "tourism:GuestCarriedEquipment"
            },
            "rdfs:comment": "A specification note for this guest carried equipment.",
            "rdfs:label": "specificationNote",
            "unece:cefactElementMetadata": [
                {
                    "@id": "cefact:Guest_CarriedEquipment.Specification.Specified_Note",
                    "@type": "unece:AssociationBIE",
                    "unece:cefactUNId": "UN01015199",
                    "unece:cefactBieDomainClass": "cefact:Guest_CarriedEquipment.Details",
                    "rdfs:comment": "A specification note for this guest carried equipment."
                }
            ]
        },
        {
            "@id": "tourism:specifiedArea",
            "@type": "rdf:Property",
            "schema:rangeIncludes": {
                "@id": "xsd:string"
            },
            "schema:domainIncludes": {
                "@id": "tourism:ProductComponentItinerary"
            },
            "rdfs:comment": "The specified area, expressed as text, for this product component itinerary.",
            "rdfs:label": "specifiedArea",
            "unece:cefactElementMetadata": [
                {
                    "@id": "cefact:ProductComponent_Itinerary.SpecifiedArea.Text",
                    "@type": "unece:BasicBIE",
                    "unece:cefactUNId": "UN01004983",
                    "unece:cefactBieDomainClass": "cefact:ProductComponent_Itinerary.Details",
                    "rdfs:comment": "The specified area, expressed as text, for this product component itinerary."
                }
            ]
        },
        {
            "@id": "tourism:specifiedAvailability",
            "@type": "rdf:Property",
            "schema:rangeIncludes": {
                "@id": "tourism:Availability"
            },
            "schema:domainIncludes": {
                "@id": "tourism:LodgingHouseTravelProductSubComponent"
            },
            "rdfs:comment": "An availability specified for this lodging house travel product sub-component.",
            "rdfs:label": "specifiedAvailability",
            "unece:cefactElementMetadata": [
                {
                    "@id": "cefact:LodgingHouse_TravelProductSub-Component.Specified.Product_Availability",
                    "@type": "unece:AssociationBIE",
                    "unece:cefactUNId": "UN01009805",
                    "unece:cefactBieDomainClass": "cefact:LodgingHouse_TravelProductSubComponent.Details",
                    "rdfs:comment": "An availability specified for this lodging house travel product sub-component."
                }
            ]
        },
        {
            "@id": "tourism:specifiedCarriedEquipment",
            "@type": "rdf:Property",
            "schema:rangeIncludes": {
                "@id": "tourism:CarriedEquipment"
            },
            "schema:domainIncludes": {
                "@id": "tourism:GuestPerson"
            },
            "rdfs:comment": "Carried equipment specified for this guest person.",
            "rdfs:label": "specifiedCarriedEquipment",
            "unece:cefactElementMetadata": [
                {
                    "@id": "cefact:Guest_Person.Specified.Guest_CarriedEquipment",
                    "@type": "unece:AssociationBIE",
                    "unece:cefactUNId": "UN01015225",
                    "unece:cefactBieDomainClass": "cefact:Guest_Person.Details",
                    "rdfs:comment": "Carried equipment specified for this guest person."
                }
            ]
        },
        {
            "@id": "tourism:specifiedCommunication",
            "@type": "rdf:Property",
            "schema:rangeIncludes": {
                "@id": "tourism:Communication"
            },
            "schema:domainIncludes": {
                "@id": "tourism:ExperienceFacility"
            },
            "rdfs:comment": "A specified universal communication for this experience facility.",
            "rdfs:label": "specifiedCommunication",
            "unece:cefactElementMetadata": [
                {
                    "@id": "cefact:Experience_Facility.Specified.Universal_Communication",
                    "@type": "unece:AssociationBIE",
                    "unece:cefactUNId": "UN01015149",
                    "unece:cefactBieDomainClass": "cefact:Experience_Facility.Details",
                    "rdfs:comment": "A specified universal communication for this experience facility."
                }
            ]
        },
        {
            "@id": "tourism:specifiedIntermediarySale",
            "@type": "rdf:Property",
            "schema:rangeIncludes": {
                "@id": "tourism:IntermediarySale"
            },
            "schema:domainIncludes": {
                "@id": "tourism:LodgingHouseTravelProduct"
            },
            "rdfs:comment": "Intermediary sale information specified for this lodging house travel product.",
            "rdfs:label": "specifiedIntermediarySale",
            "unece:cefactElementMetadata": [
                {
                    "@id": "cefact:LodgingHouse_TravelProduct.Specified.IntermediarySale",
                    "@type": "unece:AssociationBIE",
                    "unece:cefactUNId": "UN01004934",
                    "unece:cefactBieDomainClass": "cefact:LodgingHouse_TravelProduct.Details",
                    "rdfs:comment": "Intermediary sale information specified for this lodging house travel product."
                },
                {
                    "@id": "cefact:LodgingHouse_TravelProduct.Specified.TravelProduct_IntermediarySale",
                    "@type": "unece:AssociationBIE",
                    "unece:cefactUNId": "UN01010198",
                    "unece:cefactBieDomainClass": "cefact:LodgingHouse_TravelProduct.Details",
                    "rdfs:comment": "Intermediary sale information specified for this lodging house travel product."
                }
            ]
        },
        {
            "@id": "tourism:specifiedItinerary",
            "@type": "rdf:Property",
            "schema:rangeIncludes": {
                "@id": "tourism:Itinerary"
            },
            "schema:domainIncludes": {
                "@id": "tourism:LodgingHouseTravelProductComponent"
            },
            "rdfs:comment": "A product component itinerary specified for this lodging house travel product component.",
            "rdfs:label": "specifiedItinerary",
            "unece:cefactElementMetadata": [
                {
                    "@id": "cefact:LodgingHouse_TravelProductComponent.Specified.ProductComponent_Itinerary",
                    "@type": "unece:AssociationBIE",
                    "unece:cefactUNId": "UN01004978",
                    "unece:cefactBieDomainClass": "cefact:LodgingHouse_TravelProductComponent.Details",
                    "rdfs:comment": "A product component itinerary specified for this lodging house travel product component."
                }
            ]
        },
        {
            "@id": "tourism:specifiedParty",
            "@type": "rdf:Property",
            "schema:rangeIncludes": {
                "@id": "tourism:Party"
            },
            "schema:domainIncludes": [
                {
                    "@id": "tourism:ExperienceEvent"
                },
                {
                    "@id": "tourism:ExperienceProduct"
                },
                {
                    "@id": "tourism:ExperienceProgramAction"
                }
            ],
            "rdfs:comment": [
                "A party specified for this experience event.",
                "A party specified for this experience product.",
                "A party specified for this experience program action."
            ],
            "rdfs:label": "specifiedParty",
            "unece:cefactElementMetadata": [
                {
                    "@id": "cefact:Experience_Event.Specified.Trade_Party",
                    "@type": "unece:AssociationBIE",
                    "unece:cefactUNId": "UN01015131",
                    "unece:cefactBieDomainClass": "cefact:Experience_Event.Details",
                    "rdfs:comment": "A party specified for this experience event."
                },
                {
                    "@id": "cefact:ExperienceProgram_Action.Specified.Trade_Party",
                    "@type": "unece:AssociationBIE",
                    "unece:cefactUNId": "UN01015188",
                    "unece:cefactBieDomainClass": "cefact:ExperienceProgram_Action.Details",
                    "rdfs:comment": "A party specified for this experience program action."
                },
                {
                    "@id": "cefact:Experience_Product.Specified.Trade_Party",
                    "@type": "unece:AssociationBIE",
                    "unece:cefactUNId": "UN01015182",
                    "unece:cefactBieDomainClass": "cefact:Experience_Product.Details",
                    "rdfs:comment": "A party specified for this experience product."
                }
            ]
        },
        {
            "@id": "tourism:specifiedPaymentMeans",
            "@type": "rdf:Property",
            "schema:rangeIncludes": {
                "@id": "tourism:PaymentMeans"
            },
            "schema:domainIncludes": {
                "@id": "tourism:GuestPerson"
            },
            "rdfs:comment": "A trade settlement payment means specified for this guest person.",
            "rdfs:label": "specifiedPaymentMeans",
            "unece:cefactElementMetadata": [
                {
                    "@id": "cefact:Guest_Person.Specified.TradeSettlement_PaymentMeans",
                    "@type": "unece:AssociationBIE",
                    "unece:cefactUNId": "UN01015235",
                    "unece:cefactBieDomainClass": "cefact:Guest_Person.Details",
                    "rdfs:comment": "A trade settlement payment means specified for this guest person."
                }
            ]
        },
        {
            "@id": "tourism:specifiedPeriod",
            "@type": "rdf:Property",
            "schema:rangeIncludes": {
                "@id": "tourism:Period"
            },
            "schema:domainIncludes": {
                "@id": "tourism:LodgingHouseTravelProduct"
            },
            "rdfs:comment": "The period specified for this lodging house travel product.",
            "rdfs:label": "specifiedPeriod",
            "unece:cefactElementMetadata": [
                {
                    "@id": "cefact:LodgingHouse_TravelProduct.Specified.TravelProduct_Period",
                    "@type": "unece:AssociationBIE",
                    "unece:cefactUNId": "UN01009807",
                    "unece:cefactBieDomainClass": "cefact:LodgingHouse_TravelProduct.Details",
                    "rdfs:comment": "The period specified for this lodging house travel product."
                }
            ]
        },
        {
            "@id": "tourism:specifiedReservationRestriction",
            "@type": "rdf:Property",
            "schema:rangeIncludes": {
                "@id": "tourism:ReservationRestriction"
            },
            "schema:domainIncludes": {
                "@id": "tourism:LodgingHouseTravelProduct"
            },
            "rdfs:comment": "A reservation restriction specified for this lodging house travel product.",
            "rdfs:label": "specifiedReservationRestriction",
            "unece:cefactElementMetadata": [
                {
                    "@id": "cefact:LodgingHouse_TravelProduct.Specified.LodgingHouse_ReservationRestriction",
                    "@type": "unece:AssociationBIE",
                    "unece:cefactUNId": "UN01010197",
                    "unece:cefactBieDomainClass": "cefact:LodgingHouse_TravelProduct.Details",
                    "rdfs:comment": "A reservation restriction specified for this lodging house travel product."
                },
                {
                    "@id": "cefact:LodgingHouse_TravelProduct.Specified.ReservationRestriction",
                    "@type": "unece:AssociationBIE",
                    "unece:cefactUNId": "UN01004933",
                    "unece:cefactBieDomainClass": "cefact:LodgingHouse_TravelProduct.Details",
                    "rdfs:comment": "A reservation restriction specified for this lodging house travel product."
                }
            ]
        },
        {
            "@id": "tourism:specifiedServiceOption",
            "@type": "rdf:Property",
            "schema:rangeIncludes": {
                "@id": "tourism:ServiceOption"
            },
            "schema:domainIncludes": {
                "@id": "tourism:LodgingHouseTravelProductSubComponent"
            },
            "rdfs:comment": "A service option specified for this lodging house travel product sub-component.",
            "rdfs:label": "specifiedServiceOption",
            "unece:cefactElementMetadata": [
                {
                    "@id": "cefact:LodgingHouse_TravelProductSub-Component.Specified.Specified_ServiceOption",
                    "@type": "unece:AssociationBIE",
                    "unece:cefactUNId": "UN01004995",
                    "unece:cefactBieDomainClass": "cefact:LodgingHouse_TravelProductSubComponent.Details",
                    "rdfs:comment": "A service option specified for this lodging house travel product sub-component."
                }
            ]
        },
        {
            "@id": "tourism:specifiedTravelProductComponent",
            "@type": "rdf:Property",
            "schema:rangeIncludes": {
                "@id": "tourism:TravelProductComponent"
            },
            "schema:domainIncludes": {
                "@id": "tourism:LodgingHouseTravelProduct"
            },
            "rdfs:comment": "A travel component specified for this lodging house travel product.",
            "rdfs:label": "specifiedTravelProductComponent",
            "unece:cefactElementMetadata": [
                {
                    "@id": "cefact:LodgingHouse_TravelProduct.Specified.LodgingHouse_TravelProductComponent",
                    "@type": "unece:AssociationBIE",
                    "unece:cefactUNId": "UN01009808",
                    "unece:cefactBieDomainClass": "cefact:LodgingHouse_TravelProduct.Details",
                    "rdfs:comment": "A travel component specified for this lodging house travel product."
                }
            ]
        },
        {
            "@id": "tourism:specifiedTraveller",
            "@type": "rdf:Property",
            "schema:rangeIncludes": {
                "@id": "tourism:Traveller"
            },
            "schema:domainIncludes": {
                "@id": "tourism:LodgingHouseReservation"
            },
            "rdfs:comment": "A traveller specified for this lodging house reservation.",
            "rdfs:label": "specifiedTraveller",
            "unece:cefactElementMetadata": [
                {
                    "@id": "cefact:LodgingHouse_Reservation.Specified.LodgingHouse_Traveller",
                    "@type": "unece:AssociationBIE",
                    "unece:cefactUNId": "UN01009801",
                    "unece:cefactBieDomainClass": "cefact:LodgingHouse_Reservation.Details",
                    "rdfs:comment": "A traveller specified for this lodging house reservation."
                }
            ]
        },
        {
            "@id": "tourism:specifiedUsageCondition",
            "@type": "rdf:Property",
            "schema:rangeIncludes": {
                "@id": "tourism:UsageCondition"
            },
            "schema:domainIncludes": [
                {
                    "@id": "tourism:BathingFacility"
                },
                {
                    "@id": "tourism:BusinessSupportRoomFacility"
                },
                {
                    "@id": "tourism:GuestRoomFacility"
                }
            ],
            "rdfs:comment": [
                "A specified usage condition for this bathing facility at this lodging house.",
                "A specified usage condition for this guest room at this lodging house.",
                "A specified usage condition this business support room at this lodging house."
            ],
            "rdfs:label": "specifiedUsageCondition",
            "unece:cefactElementMetadata": [
                {
                    "@id": "cefact:GuestRoom_Facility.Specified.LodgingHouse_UsageCondition",
                    "@type": "unece:AssociationBIE",
                    "unece:cefactUNId": "UN01001056",
                    "unece:cefactBieDomainClass": "cefact:GuestRoom_Facility.Details",
                    "rdfs:comment": "A specified usage condition for this guest room at this lodging house."
                },
                {
                    "@id": "cefact:BusinessSupportRoom_Facility.Specified.LodgingHouse_UsageCondition",
                    "@type": "unece:AssociationBIE",
                    "unece:cefactUNId": "UN01001113",
                    "unece:cefactBieDomainClass": "cefact:BusinessSupportRoom_Facility.Details",
                    "rdfs:comment": "A specified usage condition this business support room at this lodging house."
                },
                {
                    "@id": "cefact:Bathing_Facility.Specified.LodgingHouse_UsageCondition",
                    "@type": "unece:AssociationBIE",
                    "unece:cefactUNId": "UN01001070",
                    "unece:cefactBieDomainClass": "cefact:Bathing_Facility.Details",
                    "rdfs:comment": "A specified usage condition for this bathing facility at this lodging house."
                }
            ]
        },
        {
            "@id": "tourism:startDate",
            "@type": "rdf:Property",
            "schema:rangeIncludes": {
                "@id": "xsd:base64Binary"
            },
            "schema:domainIncludes": {
                "@id": "tourism:LodgingHouseContract"
            },
            "rdfs:comment": "The date on which this lodging house contract starts.",
            "rdfs:label": "startDate",
            "unece:cefactElementMetadata": [
                {
                    "@id": "cefact:LodgingHouse_Contract.Start.Date",
                    "@type": "unece:BasicBIE",
                    "unece:cefactUNId": "UN01001213",
                    "unece:cefactBieDomainClass": "cefact:LodgingHouse_Contract.Details",
                    "rdfs:comment": "The date on which this lodging house contract starts."
                }
            ]
        },
        {
            "@id": "tourism:startDateTime",
            "@type": "rdf:Property",
            "schema:rangeIncludes": {
                "@id": "xsd:dateTime"
            },
            "schema:domainIncludes": {
                "@id": ":AvailablePeriod"
            },
            "rdfs:comment": "The date, time, date time or other date time value for the start of this available period of time.",
            "rdfs:label": "startDateTime",
            "unece:cefactElementMetadata": [
                {
                    "@id": "cefact:Available_Period.Start.DateTime",
                    "@type": "unece:BasicBIE",
                    "unece:cefactUNId": "UN01005109",
                    "unece:cefactBieDomainClass": "cefact:Available_Period.Details",
                    "rdfs:comment": "The date, time, date time or other date time value for the start of this available period of time."
                }
            ]
        },
        {
            "@id": "tourism:status",
            "@type": "rdf:Property",
            "schema:rangeIncludes": {
                "@id": "xsd:string"
            },
            "schema:domainIncludes": {
                "@id": "tourism:GuestHealthIndication"
            },
            "rdfs:comment": "A status, expressed as text, for this guest health indication.",
            "rdfs:label": "status",
            "unece:cefactElementMetadata": [
                {
                    "@id": "cefact:Guest_HealthIndication.Status.Text",
                    "@type": "unece:BasicBIE",
                    "unece:cefactUNId": "UN01015213",
                    "unece:cefactBieDomainClass": "cefact:Guest_HealthIndication.Details",
                    "rdfs:comment": "A status, expressed as text, for this guest health indication."
                }
            ]
        },
        {
            "@id": "tourism:statusCode",
            "@type": "rdf:Property",
            "schema:rangeIncludes": {
                "@id": "xsd:token"
            },
            "schema:domainIncludes": [
                {
                    "@id": "tourism:ExperienceProgramAction"
                },
                {
                    "@id": "tourism:LodgingHouseReservation"
                }
            ],
            "rdfs:comment": [
                "The code specifying the status of this experience program action.",
                "The code specifying the status of this lodging house reservation."
            ],
            "rdfs:label": "statusCode",
            "unece:cefactElementMetadata": [
                {
                    "@id": "cefact:LodgingHouse_Reservation.Status.Code",
                    "@type": "unece:BasicBIE",
                    "unece:cefactUNId": "UN01009793",
                    "unece:cefactBieDomainClass": "cefact:LodgingHouse_Reservation.Details",
                    "rdfs:comment": "The code specifying the status of this lodging house reservation."
                },
                {
                    "@id": "cefact:ExperienceProgram_Action.Status.Code",
                    "@type": "unece:BasicBIE",
                    "unece:cefactUNId": "UN01015186",
                    "unece:cefactBieDomainClass": "cefact:ExperienceProgram_Action.Details",
                    "rdfs:comment": "The code specifying the status of this experience program action."
                }
            ]
        },
        {
            "@id": "tourism:subject",
            "@type": "rdf:Property",
            "schema:rangeIncludes": {
                "@id": "xsd:string"
            },
            "schema:domainIncludes": {
                "@id": "tourism:LodgingHousePicture"
            },
            "rdfs:comment": "The subject, expressed as text, for this lodging house picture.",
            "rdfs:label": "subject",
            "unece:cefactElementMetadata": [
                {
                    "@id": "cefact:LodgingHouse_Picture.Subject.Text",
                    "@type": "unece:BasicBIE",
                    "unece:cefactUNId": "UN01001246",
                    "unece:cefactBieDomainClass": "cefact:LodgingHouse_Picture.Details",
                    "rdfs:comment": "The subject, expressed as text, for this lodging house picture."
                }
            ]
        },
        {
            "@id": "tourism:submittedQuery",
            "@type": "rdf:Property",
            "schema:rangeIncludes": {
                "@id": "tourism:Query"
            },
            "schema:domainIncludes": {
                "@id": "tourism:LodgingHouseTraveller"
            },
            "rdfs:comment": "A special query submitted by this lodging house traveller.",
            "rdfs:label": "submittedQuery",
            "unece:cefactElementMetadata": [
                {
                    "@id": "cefact:LodgingHouse_Traveller.Submitted.Special_Query",
                    "@type": "unece:AssociationBIE",
                    "unece:cefactUNId": "UN01009819",
                    "unece:cefactBieDomainClass": "cefact:LodgingHouse_Traveller.Details",
                    "rdfs:comment": "A special query submitted by this lodging house traveller."
                }
            ]
        },
        {
            "@id": "tourism:supplierId",
            "@type": "rdf:Property",
            "schema:rangeIncludes": {
                "@id": "xsd:token"
            },
            "schema:domainIncludes": [
                {
                    "@id": "tourism:LodgingHouseTravelProduct"
                },
                {
                    "@id": "tourism:LodgingHouseTravelProductSubComponent"
                }
            ],
            "rdfs:comment": [
                "The unique identifier for the supplier of this lodging house travel product sub-component.",
                "The unique identifier for the supplier of this lodging house travel product."
            ],
            "rdfs:label": "supplierId",
            "unece:cefactElementMetadata": [
                {
                    "@id": "cefact:LodgingHouse_TravelProductSub-Component.Supplier.Identifier",
                    "@type": "unece:BasicBIE",
                    "unece:cefactUNId": "UN01004990",
                    "unece:cefactBieDomainClass": "cefact:LodgingHouse_TravelProductSubComponent.Details",
                    "rdfs:comment": "The unique identifier for the supplier of this lodging house travel product sub-component."
                },
                {
                    "@id": "cefact:LodgingHouse_TravelProduct.Supplier.Identifier",
                    "@type": "unece:BasicBIE",
                    "unece:cefactUNId": "UN01004923",
                    "unece:cefactBieDomainClass": "cefact:LodgingHouse_TravelProduct.Details",
                    "rdfs:comment": "The unique identifier for the supplier of this lodging house travel product."
                }
            ]
        },
        {
            "@id": "tourism:supplierName",
            "@type": "rdf:Property",
            "schema:rangeIncludes": {
                "@id": "xsd:string"
            },
            "schema:domainIncludes": [
                {
                    "@id": "tourism:LodgingHouseTravelProduct"
                },
                {
                    "@id": "tourism:LodgingHouseTravelProductSubComponent"
                }
            ],
            "rdfs:comment": [
                "The name, expressed as text, of the supplier of this lodging house travel product sub-component.",
                "The name, expressed as text, of the supplier of this lodging house travel product."
            ],
            "rdfs:label": "supplierName",
            "unece:cefactElementMetadata": [
                {
                    "@id": "cefact:LodgingHouse_TravelProductSub-Component.SupplierName.Text",
                    "@type": "unece:BasicBIE",
                    "unece:cefactUNId": "UN01004991",
                    "unece:cefactBieDomainClass": "cefact:LodgingHouse_TravelProductSubComponent.Details",
                    "rdfs:comment": "The name, expressed as text, of the supplier of this lodging house travel product sub-component."
                },
                {
                    "@id": "cefact:LodgingHouse_TravelProduct.SupplierName.Text",
                    "@type": "unece:BasicBIE",
                    "unece:cefactUNId": "UN01004922",
                    "unece:cefactBieDomainClass": "cefact:LodgingHouse_TravelProduct.Details",
                    "rdfs:comment": "The name, expressed as text, of the supplier of this lodging house travel product."
                }
            ]
        },
        {
            "@id": "tourism:takenDateTime",
            "@type": "rdf:Property",
            "schema:rangeIncludes": {
                "@id": "xsd:dateTime"
            },
            "schema:domainIncludes": {
                "@id": "tourism:LodgingHousePicture"
            },
            "rdfs:comment": "The date, time, date time, or other date value when this lodging house picture was created.",
            "rdfs:label": "takenDateTime",
            "unece:cefactElementMetadata": [
                {
                    "@id": "cefact:LodgingHouse_Picture.Taken.DateTime",
                    "@type": "unece:BasicBIE",
                    "unece:cefactUNId": "UN01001249",
                    "unece:cefactBieDomainClass": "cefact:LodgingHouse_Picture.Details",
                    "rdfs:comment": "The date, time, date time, or other date value when this lodging house picture was created."
                }
            ]
        },
        {
            "@id": "tourism:taxChargeApplicableIndicator",
            "@type": "rdf:Property",
            "schema:rangeIncludes": {
                "@id": "xsd:boolean"
            },
            "schema:domainIncludes": [
                {
                    "@id": "tourism:BasicPrice"
                },
                {
                    "@id": "tourism:DiscountPrice"
                },
                {
                    "@id": "tourism:ExtraPrice"
                }
            ],
            "rdfs:comment": [
                "The indication of whether or not a tax charge is applicable to the basic price.",
                "The indication of whether or not a tax charge is applicable to the discount price.",
                "The indication of whether or not a tax charge is applicable to the extra price."
            ],
            "rdfs:label": "taxChargeApplicableIndicator",
            "unece:cefactElementMetadata": [
                {
                    "@id": "cefact:Extra_Price.Tax_ChargeApplicable.Indicator",
                    "@type": "unece:BasicBIE",
                    "unece:cefactUNId": "UN01005024",
                    "unece:cefactBieDomainClass": "cefact:Extra_Price.Details",
                    "rdfs:comment": "The indication of whether or not a tax charge is applicable to the extra price."
                },
                {
                    "@id": "cefact:Basic_Price.Tax_ChargeApplicable.Indicator",
                    "@type": "unece:BasicBIE",
                    "unece:cefactUNId": "UN01005008",
                    "unece:cefactBieDomainClass": "cefact:Basic_Price.Details",
                    "rdfs:comment": "The indication of whether or not a tax charge is applicable to the basic price."
                },
                {
                    "@id": "cefact:Discount_Price.Tax_ChargeApplicable.Indicator",
                    "@type": "unece:BasicBIE",
                    "unece:cefactUNId": "UN01005043",
                    "unece:cefactBieDomainClass": "cefact:Discount_Price.Details",
                    "rdfs:comment": "The indication of whether or not a tax charge is applicable to the discount price."
                }
            ]
        },
        {
            "@id": "tourism:taxCommissionChargeAmount",
            "@type": "rdf:Property",
            "schema:rangeIncludes": {
                "@id": "xsd:decimal"
            },
            "schema:domainIncludes": {
                "@id": "tourism:DailyPrice"
            },
            "rdfs:comment": "The monetary value of the tax, such as sales tax, charged for this commission price on which the daily price is calculated.",
            "rdfs:label": "taxCommissionChargeAmount",
            "unece:cefactElementMetadata": [
                {
                    "@id": "cefact:Daily_Price.Tax_Commission_Charge.Amount",
                    "@type": "unece:BasicBIE",
                    "unece:cefactUNId": "UN01009694",
                    "unece:cefactBieDomainClass": "cefact:Daily_Price.Details",
                    "rdfs:comment": "The monetary value of the tax, such as sales tax, charged for this commission price on which the daily price is calculated."
                }
            ]
        },
        {
            "@id": "tourism:telephoneCommunication",
            "@type": "rdf:Property",
            "schema:rangeIncludes": {
                "@id": "tourism:Communication"
            },
            "schema:domainIncludes": {
                "@id": "tourism:LodgingHouseContact"
            },
            "rdfs:comment": "A universal telephone communication for this lodging house contact.",
            "rdfs:label": "telephoneCommunication",
            "unece:cefactElementMetadata": [
                {
                    "@id": "cefact:LodgingHouse_Contact.Telephone.Universal_Communication",
                    "@type": "unece:AssociationBIE",
                    "unece:cefactUNId": "UN01001230",
                    "unece:cefactBieDomainClass": "cefact:LodgingHouse_Contact.Details",
                    "rdfs:comment": "A universal telephone communication for this lodging house contact."
                }
            ]
        },
        {
            "@id": "tourism:theme",
            "@type": "rdf:Property",
            "schema:rangeIncludes": {
                "@id": "xsd:string"
            },
            "schema:domainIncludes": {
                "@id": "tourism:ExperienceProduct"
            },
            "rdfs:comment": "A theme, expressed as text, for this experience product.",
            "rdfs:label": "theme",
            "unece:cefactElementMetadata": [
                {
                    "@id": "cefact:Experience_Product.Theme.Text",
                    "@type": "unece:BasicBIE",
                    "unece:cefactUNId": "UN01015157",
                    "unece:cefactBieDomainClass": "cefact:Experience_Product.Details",
                    "rdfs:comment": "A theme, expressed as text, for this experience product."
                }
            ]
        },
        {
            "@id": "tourism:themeTypeCode",
            "@type": "rdf:Property",
            "schema:rangeIncludes": {
                "@id": "xsd:token"
            },
            "schema:domainIncludes": {
                "@id": "tourism:ExperienceProduct"
            },
            "rdfs:comment": "The code specifying the type of theme for this experience product.",
            "rdfs:label": "themeTypeCode",
            "unece:cefactElementMetadata": [
                {
                    "@id": "cefact:Experience_Product.ThemeType.Code",
                    "@type": "unece:BasicBIE",
                    "unece:cefactUNId": "UN01015158",
                    "unece:cefactBieDomainClass": "cefact:Experience_Product.Details",
                    "rdfs:comment": "The code specifying the type of theme for this experience product."
                }
            ]
        },
        {
            "@id": "tourism:title",
            "@type": "rdf:Property",
            "schema:rangeIncludes": {
                "@id": "xsd:string"
            },
            "schema:domainIncludes": {
                "@id": "tourism:GuestPerson"
            },
            "rdfs:comment": "The title, expressed as text, associated with this guest, such as Doctor, Mr., Mrs., Ms.",
            "rdfs:label": "title",
            "unece:cefactElementMetadata": [
                {
                    "@id": "cefact:Guest_Person.Title.Text",
                    "@type": "unece:BasicBIE",
                    "unece:TDED": "3504",
                    "unece:cefactUNId": "UN01009711",
                    "unece:cefactBieDomainClass": "cefact:Guest_Person.Details",
                    "rdfs:comment": "The title, expressed as text, associated with this guest, such as Doctor, Mr., Mrs., Ms."
                }
            ]
        },
        {
            "@id": "tourism:titleCode",
            "@type": "rdf:Property",
            "schema:rangeIncludes": {
                "@id": "xsd:token"
            },
            "schema:domainIncludes": {
                "@id": "tourism:GuestPerson"
            },
            "rdfs:comment": "The code specifying the title of this guest person.",
            "rdfs:label": "titleCode",
            "unece:cefactElementMetadata": [
                {
                    "@id": "cefact:Guest_Person.Title.Code",
                    "@type": "unece:BasicBIE",
                    "unece:cefactUNId": "UN01015217",
                    "unece:cefactBieDomainClass": "cefact:Guest_Person.Details",
                    "rdfs:comment": "The code specifying the title of this guest person."
                }
            ]
        },
        {
            "@id": "tourism:titleName",
            "@type": "rdf:Property",
            "schema:rangeIncludes": {
                "@id": "xsd:string"
            },
            "schema:domainIncludes": {
                "@id": "tourism:LodgingHousePicture"
            },
            "rdfs:comment": "The title name, expressed as text, for this lodging house picture.",
            "rdfs:label": "titleName",
            "unece:cefactElementMetadata": [
                {
                    "@id": "cefact:LodgingHouse_Picture.TitleName.Text",
                    "@type": "unece:BasicBIE",
                    "unece:cefactUNId": "UN01001243",
                    "unece:cefactBieDomainClass": "cefact:LodgingHouse_Picture.Details",
                    "rdfs:comment": "The title name, expressed as text, for this lodging house picture."
                }
            ]
        },
        {
            "@id": "tourism:totalCustomerQuantity",
            "@type": "rdf:Property",
            "schema:rangeIncludes": {
                "@id": "xsd:decimal"
            },
            "schema:domainIncludes": {
                "@id": "tourism:LodgingHouseReservation"
            },
            "rdfs:comment": "The total number of customers for this lodging house reservation.",
            "rdfs:label": "totalCustomerQuantity",
            "unece:cefactElementMetadata": [
                {
                    "@id": "cefact:LodgingHouse_Reservation.TotalCustomer.Quantity",
                    "@type": "unece:BasicBIE",
                    "unece:cefactUNId": "UN01009794",
                    "unece:cefactBieDomainClass": "cefact:LodgingHouse_Reservation.Details",
                    "rdfs:comment": "The total number of customers for this lodging house reservation."
                }
            ]
        },
        {
            "@id": "tourism:tradingPartnerId",
            "@type": "rdf:Property",
            "schema:rangeIncludes": {
                "@id": "xsd:token"
            },
            "schema:domainIncludes": {
                "@id": "tourism:LodgingHouseContract"
            },
            "rdfs:comment": "The unique identifier for the trading partner for this lodging house contract.",
            "rdfs:label": "tradingPartnerId",
            "unece:cefactElementMetadata": [
                {
                    "@id": "cefact:LodgingHouse_Contract.TradingPartner_Identification.Identifier",
                    "@type": "unece:BasicBIE",
                    "unece:TDED": "1296",
                    "unece:cefactUNId": "UN01001212",
                    "unece:cefactBieDomainClass": "cefact:LodgingHouse_Contract.Details",
                    "rdfs:comment": "The unique identifier for the trading partner for this lodging house contract."
                }
            ]
        },
        {
            "@id": "tourism:transportMeans",
            "@type": "rdf:Property",
            "schema:rangeIncludes": {
                "@id": "xsd:string"
            },
            "schema:domainIncludes": {
                "@id": "tourism:LodgingHouseRoute"
            },
            "rdfs:comment": "A means of transport, expressed as text, used for this route to this lodging house.",
            "rdfs:label": "transportMeans",
            "unece:cefactElementMetadata": [
                {
                    "@id": "cefact:LodgingHouse_Route.TransportMeans.Text",
                    "@type": "unece:BasicBIE",
                    "unece:cefactUNId": "UN01001240",
                    "unece:cefactBieDomainClass": "cefact:LodgingHouse_Route.Details",
                    "rdfs:comment": "A means of transport, expressed as text, used for this route to this lodging house."
                }
            ]
        },
        {
            "@id": "tourism:travelInsuranceCertificate",
            "@type": "rdf:Property",
            "schema:rangeIncludes": {
                "@id": "tourism:Certificate"
            },
            "schema:domainIncludes": {
                "@id": "tourism:GuestPerson"
            },
            "rdfs:comment": "A travel insurance certificate for this guest person.",
            "rdfs:label": "travelInsuranceCertificate",
            "unece:cefactElementMetadata": [
                {
                    "@id": "cefact:Guest_Person.Travel_Insurance.Specified_Certificate",
                    "@type": "unece:AssociationBIE",
                    "unece:cefactUNId": "UN01015232",
                    "unece:cefactBieDomainClass": "cefact:Guest_Person.Details",
                    "rdfs:comment": "A travel insurance certificate for this guest person."
                }
            ]
        },
        {
            "@id": "tourism:travelLicenceId",
            "@type": "rdf:Property",
            "schema:rangeIncludes": {
                "@id": "xsd:token"
            },
            "schema:domainIncludes": {
                "@id": "tourism:LodgingHouseTravelProduct"
            },
            "rdfs:comment": "The unique travel licence identifier for this lodging house travel product.",
            "rdfs:label": "travelLicenceId",
            "unece:cefactElementMetadata": [
                {
                    "@id": "cefact:LodgingHouse_TravelProduct.TravelLicence.Identifier",
                    "@type": "unece:BasicBIE",
                    "unece:cefactUNId": "UN01004925",
                    "unece:cefactBieDomainClass": "cefact:LodgingHouse_TravelProduct.Details",
                    "rdfs:comment": "The unique travel licence identifier for this lodging house travel product."
                }
            ]
        },
        {
            "@id": "tourism:travelProductTaxChargeAmount",
            "@type": "rdf:Property",
            "schema:rangeIncludes": {
                "@id": "xsd:decimal"
            },
            "schema:domainIncludes": {
                "@id": "tourism:DailyPrice"
            },
            "rdfs:comment": "The monetary value of the travel product tax charged on which this daily price is calculated.",
            "rdfs:label": "travelProductTaxChargeAmount",
            "unece:cefactElementMetadata": [
                {
                    "@id": "cefact:Daily_Price.TravelProduct_Tax_Charge.Amount",
                    "@type": "unece:BasicBIE",
                    "unece:cefactUNId": "UN01009696",
                    "unece:cefactBieDomainClass": "cefact:Daily_Price.Details",
                    "rdfs:comment": "The monetary value of the travel product tax charged on which this daily price is calculated."
                }
            ]
        },
        {
            "@id": "tourism:type",
            "@type": "rdf:Property",
            "schema:rangeIncludes": {
                "@id": "xsd:string"
            },
            "schema:domainIncludes": [
                {
                    "@id": "tourism:BasicPrice"
                },
                {
                    "@id": "tourism:DailyPrice"
                },
                {
                    "@id": "tourism:DiscountPrice"
                },
                {
                    "@id": "tourism:ExperienceFacility"
                },
                {
                    "@id": "tourism:ExperienceProgramAction"
                },
                {
                    "@id": "tourism:ExtraPrice"
                },
                {
                    "@id": "tourism:GuestRoomFacility"
                },
                {
                    "@id": "tourism:LodgingHousePicture"
                }
            ],
            "rdfs:comment": [
                "A type, expressed as text, of experience program action.",
                "A type, expressed as text, of this experience facility.",
                "The type, expressed as text, for this daily price.",
                "The type, expressed as text, for this lodging house picture.",
                "The type, expressed as text, of the basic price.",
                "The type, expressed as text, of this discount price.",
                "The type, expressed as text, of this extra price.",
                "The type, expressed as text, of this guest room."
            ],
            "rdfs:label": "type",
            "unece:cefactElementMetadata": [
                {
                    "@id": "cefact:Basic_Price.Type.Text",
                    "@type": "unece:BasicBIE",
                    "unece:cefactUNId": "UN01005001",
                    "unece:cefactBieDomainClass": "cefact:Basic_Price.Details",
                    "rdfs:comment": "The type, expressed as text, of the basic price."
                },
                {
                    "@id": "cefact:Discount_Price.Type.Text",
                    "@type": "unece:BasicBIE",
                    "unece:cefactUNId": "UN01005036",
                    "unece:cefactBieDomainClass": "cefact:Discount_Price.Details",
                    "rdfs:comment": "The type, expressed as text, of this discount price."
                },
                {
                    "@id": "cefact:LodgingHouse_Picture.Type.Text",
                    "@type": "unece:BasicBIE",
                    "unece:cefactUNId": "UN01001245",
                    "unece:cefactBieDomainClass": "cefact:LodgingHouse_Picture.Details",
                    "rdfs:comment": "The type, expressed as text, for this lodging house picture."
                },
                {
                    "@id": "cefact:ExperienceProgram_Action.Type.Text",
                    "@type": "unece:BasicBIE",
                    "unece:cefactUNId": "UN01015185",
                    "unece:cefactBieDomainClass": "cefact:ExperienceProgram_Action.Details",
                    "rdfs:comment": "A type, expressed as text, of experience program action."
                },
                {
                    "@id": "cefact:Extra_Price.Type.Text",
                    "@type": "unece:BasicBIE",
                    "unece:cefactUNId": "UN01005017",
                    "unece:cefactBieDomainClass": "cefact:Extra_Price.Details",
                    "rdfs:comment": "The type, expressed as text, of this extra price."
                },
                {
                    "@id": "cefact:GuestRoom_Facility.Type.Text",
                    "@type": "unece:BasicBIE",
                    "unece:TDED": "9038",
                    "unece:cefactUNId": "UN01001054",
                    "unece:cefactBieDomainClass": "cefact:GuestRoom_Facility.Details",
                    "rdfs:comment": "The type, expressed as text, of this guest room."
                },
                {
                    "@id": "cefact:Daily_Price.Type.Text",
                    "@type": "unece:BasicBIE",
                    "unece:cefactUNId": "UN01009687",
                    "unece:cefactBieDomainClass": "cefact:Daily_Price.Details",
                    "rdfs:comment": "The type, expressed as text, for this daily price."
                },
                {
                    "@id": "cefact:Experience_Facility.Type.Text",
                    "@type": "unece:BasicBIE",
                    "unece:TDED": "9038",
                    "unece:cefactUNId": "UN01015141",
                    "unece:cefactBieDomainClass": "cefact:Experience_Facility.Details",
                    "rdfs:comment": "A type, expressed as text, of this experience facility."
                }
            ]
        },
        {
            "@id": "tourism:typeCode",
            "@type": "rdf:Property",
            "schema:rangeIncludes": {
                "@id": "xsd:token"
            },
            "schema:domainIncludes": [
                {
                    "@id": "tourism:ExperienceItemVoucher"
                },
                {
                    "@id": "tourism:ExperienceProgramAction"
                },
                {
                    "@id": "tourism:GuestAllergy"
                },
                {
                    "@id": "tourism:GuestCarriedEquipment"
                },
                {
                    "@id": "tourism:GuestDisability"
                },
                {
                    "@id": "tourism:GuestFoodChoice"
                },
                {
                    "@id": "tourism:GuestHealthIndication"
                },
                {
                    "@id": "tourism:LodgingHouseContact"
                },
                {
                    "@id": "tourism:LodgingHouseParty"
                },
                {
                    "@id": "tourism:LodgingHouseReservationRestriction"
                },
                {
                    "@id": "tourism:LodgingHouseTravelProduct"
                },
                {
                    "@id": "tourism:ReservationRestriction"
                }
            ],
            "rdfs:comment": [
                "A code specifying the type of this lodging house party.",
                "The code specifying the type of contact for this lodging house.",
                "The code specifying the type of experience item voucher.",
                "The code specifying the type of experience program action.",
                "The code specifying the type of guest allergy.",
                "The code specifying the type of guest carried equipment.",
                "The code specifying the type of guest disability.",
                "The code specifying the type of guest food choice.",
                "The code specifying the type of guest heath indication.",
                "The code specifying the type of lodging house reservation restriction.",
                "The code specifying the type of lodging house travel product.",
                "The code specifying the type of reservation restriction."
            ],
            "rdfs:label": "typeCode",
            "unece:cefactElementMetadata": [
                {
                    "@id": "cefact:ExperienceItem_Voucher.Type.Code",
                    "@type": "unece:BasicBIE",
                    "unece:cefactUNId": "UN01015243",
                    "unece:cefactBieDomainClass": "cefact:ExperienceItem_Voucher.Details",
                    "rdfs:comment": "The code specifying the type of experience item voucher."
                },
                {
                    "@id": "cefact:ExperienceProgram_Action.Type.Code",
                    "@type": "unece:BasicBIE",
                    "unece:cefactUNId": "UN01015184",
                    "unece:cefactBieDomainClass": "cefact:ExperienceProgram_Action.Details",
                    "rdfs:comment": "The code specifying the type of experience program action."
                },
                {
                    "@id": "cefact:Guest_Allergy.Type.Code",
                    "@type": "unece:BasicBIE",
                    "unece:cefactUNId": "UN01015191",
                    "unece:cefactBieDomainClass": "cefact:Guest_Allergy.Details",
                    "rdfs:comment": "The code specifying the type of guest allergy."
                },
                {
                    "@id": "cefact:Guest_Disability.Type.Code",
                    "@type": "unece:BasicBIE",
                    "unece:cefactUNId": "UN01015202",
                    "unece:cefactBieDomainClass": "cefact:Guest_Disability.Details",
                    "rdfs:comment": "The code specifying the type of guest disability."
                },
                {
                    "@id": "cefact:ReservationRestriction.Type.Code",
                    "@type": "unece:BasicBIE",
                    "unece:cefactUNId": "UN01004955",
                    "unece:cefactBieDomainClass": "cefact:ReservationRestriction.Details",
                    "rdfs:comment": "The code specifying the type of reservation restriction."
                },
                {
                    "@id": "cefact:LodgingHouse_ReservationRestriction.Type.Code",
                    "@type": "unece:BasicBIE",
                    "unece:cefactUNId": "UN01010047",
                    "unece:cefactBieDomainClass": "cefact:LodgingHouse_ReservationRestriction.Details",
                    "rdfs:comment": "The code specifying the type of lodging house reservation restriction."
                },
                {
                    "@id": "cefact:LodgingHouse_TravelProduct.Type.Code",
                    "@type": "unece:BasicBIE",
                    "unece:cefactUNId": "UN01004917",
                    "unece:cefactBieDomainClass": "cefact:LodgingHouse_TravelProduct.Details",
                    "rdfs:comment": "The code specifying the type of lodging house travel product."
                },
                {
                    "@id": "cefact:LodgingHouse_Party.Type.Code",
                    "@type": "unece:BasicBIE",
                    "unece:cefactUNId": "UN01001282",
                    "unece:cefactBieDomainClass": "cefact:LodgingHouse_Party.Details",
                    "rdfs:comment": "A code specifying the type of this lodging house party."
                },
                {
                    "@id": "cefact:LodgingHouse_Contact.Type.Code",
                    "@type": "unece:BasicBIE",
                    "unece:cefactUNId": "UN01001226",
                    "unece:cefactBieDomainClass": "cefact:LodgingHouse_Contact.Details",
                    "rdfs:comment": "The code specifying the type of contact for this lodging house."
                },
                {
                    "@id": "cefact:Guest_CarriedEquipment.Type.Code",
                    "@type": "unece:BasicBIE",
                    "unece:cefactUNId": "UN01015196",
                    "unece:cefactBieDomainClass": "cefact:Guest_CarriedEquipment.Details",
                    "rdfs:comment": "The code specifying the type of guest carried equipment."
                },
                {
                    "@id": "cefact:Guest_FoodChoice.Type.Code",
                    "@type": "unece:BasicBIE",
                    "unece:cefactUNId": "UN01015209",
                    "unece:cefactBieDomainClass": "cefact:Guest_FoodChoice.Details",
                    "rdfs:comment": "The code specifying the type of guest food choice."
                },
                {
                    "@id": "cefact:Guest_HealthIndication.Type.Code",
                    "@type": "unece:BasicBIE",
                    "unece:cefactUNId": "UN01015214",
                    "unece:cefactBieDomainClass": "cefact:Guest_HealthIndication.Details",
                    "rdfs:comment": "The code specifying the type of guest heath indication."
                }
            ]
        },
        {
            "@id": "tourism:unitId",
            "@type": "rdf:Property",
            "schema:rangeIncludes": {
                "@id": "xsd:token"
            },
            "schema:domainIncludes": {
                "@id": "tourism:TravelProductReservationItem"
            },
            "rdfs:comment": "The identifier of the unit for this travel product reservation item.",
            "rdfs:label": "unitId",
            "unece:cefactElementMetadata": [
                {
                    "@id": "cefact:TravelProduct_ReservationItem.Unit.Identifier",
                    "@type": "unece:BasicBIE",
                    "unece:cefactUNId": "UN01009974",
                    "unece:cefactBieDomainClass": "cefact:TravelProduct_ReservationItem.Details",
                    "rdfs:comment": "The identifier of the unit for this travel product reservation item."
                }
            ]
        },
        {
            "@id": "tourism:unitQuantity",
            "@type": "rdf:Property",
            "schema:rangeIncludes": {
                "@id": "xsd:decimal"
            },
            "schema:domainIncludes": {
                "@id": "tourism:TravelProductReservationItem"
            },
            "rdfs:comment": "The number of units of this travel product reservation item.",
            "rdfs:label": "unitQuantity",
            "unece:cefactElementMetadata": [
                {
                    "@id": "cefact:TravelProduct_ReservationItem.Unit.Quantity",
                    "@type": "unece:BasicBIE",
                    "unece:cefactUNId": "UN01009973",
                    "unece:cefactBieDomainClass": "cefact:TravelProduct_ReservationItem.Details",
                    "rdfs:comment": "The number of units of this travel product reservation item."
                }
            ]
        },
        {
            "@id": "tourism:upperAgeLimitNumeric",
            "@type": "rdf:Property",
            "schema:rangeIncludes": {
                "@id": "xsd:decimal"
            },
            "schema:domainIncludes": [
                {
                    "@id": "tourism:CustomerClass"
                },
                {
                    "@id": "tourism:LodgingHouseCustomerClass"
                }
            ],
            "rdfs:comment": [
                "The upper age limit in number of years for the category of a customer class.",
                "The upper age limit in number of years for the category of this lodging house customer class."
            ],
            "rdfs:label": "upperAgeLimitNumeric",
            "unece:cefactElementMetadata": [
                {
                    "@id": "cefact:CustomerClass.UpperAgeLimit.Numeric",
                    "@type": "unece:BasicBIE",
                    "unece:cefactUNId": "UN01004948",
                    "unece:cefactBieDomainClass": "cefact:CustomerClass.Details",
                    "rdfs:comment": "The upper age limit in number of years for the category of a customer class."
                },
                {
                    "@id": "cefact:LodgingHouse_CustomerClass.UpperAgeLimit.Numeric",
                    "@type": "unece:BasicBIE",
                    "unece:cefactUNId": "UN01010032",
                    "unece:cefactBieDomainClass": "cefact:LodgingHouse_CustomerClass.Details",
                    "rdfs:comment": "The upper age limit in number of years for the category of this lodging house customer class."
                }
            ]
        },
        {
            "@id": "tourism:usedCommunication",
            "@type": "rdf:Property",
            "schema:rangeIncludes": {
                "@id": "tourism:Communication"
            },
            "schema:domainIncludes": {
                "@id": "tourism:GuestPerson"
            },
            "rdfs:comment": "A universal communication used by this guest.",
            "rdfs:label": "usedCommunication",
            "unece:cefactElementMetadata": [
                {
                    "@id": "cefact:Guest_Person.Used.Universal_Communication",
                    "@type": "unece:AssociationBIE",
                    "unece:cefactUNId": "UN01009717",
                    "unece:cefactBieDomainClass": "cefact:Guest_Person.Details",
                    "rdfs:comment": "A universal communication used by this guest."
                }
            ]
        },
        {
            "@id": "tourism:usedSalesChannel",
            "@type": "rdf:Property",
            "schema:rangeIncludes": {
                "@id": "tourism:SalesChannel"
            },
            "schema:domainIncludes": {
                "@id": "tourism:LodgingHouseReservation"
            },
            "rdfs:comment": "A travel sales channel used for this lodging house reservation.",
            "rdfs:label": "usedSalesChannel",
            "unece:cefactElementMetadata": [
                {
                    "@id": "cefact:LodgingHouse_Reservation.Used.Travel_SalesChannel",
                    "@type": "unece:AssociationBIE",
                    "unece:cefactUNId": "UN01009802",
                    "unece:cefactBieDomainClass": "cefact:LodgingHouse_Reservation.Details",
                    "rdfs:comment": "A travel sales channel used for this lodging house reservation."
                }
            ]
        },
        {
            "@id": "tourism:usedSource",
            "@type": "rdf:Property",
            "schema:rangeIncludes": {
                "@id": "tourism:Source"
            },
            "schema:domainIncludes": {
                "@id": "tourism:ExperienceFacility"
            },
            "rdfs:comment": "A water source used by this experience facility.",
            "rdfs:label": "usedSource",
            "unece:cefactElementMetadata": [
                {
                    "@id": "cefact:Experience_Facility.Used.Water_Source",
                    "@type": "unece:AssociationBIE",
                    "unece:cefactUNId": "UN01015146",
                    "unece:cefactBieDomainClass": "cefact:Experience_Facility.Details",
                    "rdfs:comment": "A water source used by this experience facility."
                }
            ]
        },
        {
            "@id": "tourism:validityPeriod",
            "@type": "rdf:Property",
            "schema:rangeIncludes": {
                "@id": "tourism:Period"
            },
            "schema:domainIncludes": [
                {
                    "@id": "tourism:BasicPrice"
                },
                {
                    "@id": "tourism:CancellationPrice"
                },
                {
                    "@id": "tourism:DiscountPrice"
                },
                {
                    "@id": "tourism:ExtraPrice"
                }
            ],
            "rdfs:comment": [
                "A seasonal period for which this basic price is valid.",
                "A seasonal period for which this cancellation price is valid.",
                "A seasonal period for which this discount price is valid.",
                "A seasonal period for which this extra price is valid.",
                "A travel product period for which this basic price is valid.",
                "A travel product period for which this cancellation price is valid.",
                "A travel product period for which this discount price is valid.",
                "A travel product period for which this extra price is valid."
            ],
            "rdfs:label": "validityPeriod",
            "unece:cefactElementMetadata": [
                {
                    "@id": "cefact:Cancellation_Price.Validity.TravelProduct_Period",
                    "@type": "unece:AssociationBIE",
                    "unece:cefactUNId": "UN01005081",
                    "unece:cefactBieDomainClass": "cefact:Cancellation_Price.Details",
                    "rdfs:comment": "A travel product period for which this cancellation price is valid."
                },
                {
                    "@id": "cefact:Basic_Price.Validity.TravelProduct_Period",
                    "@type": "unece:AssociationBIE",
                    "unece:cefactUNId": "UN01005011",
                    "unece:cefactBieDomainClass": "cefact:Basic_Price.Details",
                    "rdfs:comment": "A travel product period for which this basic price is valid."
                },
                {
                    "@id": "cefact:Discount_Price.Validity.Seasonal_Period",
                    "@type": "unece:AssociationBIE",
                    "unece:cefactUNId": "UN01005050",
                    "unece:cefactBieDomainClass": "cefact:Discount_Price.Details",
                    "rdfs:comment": "A seasonal period for which this discount price is valid."
                },
                {
                    "@id": "cefact:Basic_Price.Validity.Seasonal_Period",
                    "@type": "unece:AssociationBIE",
                    "unece:cefactUNId": "UN01005012",
                    "unece:cefactBieDomainClass": "cefact:Basic_Price.Details",
                    "rdfs:comment": "A seasonal period for which this basic price is valid."
                },
                {
                    "@id": "cefact:Cancellation_Price.Validity.Seasonal_Period",
                    "@type": "unece:AssociationBIE",
                    "unece:cefactUNId": "UN01005082",
                    "unece:cefactBieDomainClass": "cefact:Cancellation_Price.Details",
                    "rdfs:comment": "A seasonal period for which this cancellation price is valid."
                },
                {
                    "@id": "cefact:Extra_Price.Validity.TravelProduct_Period",
                    "@type": "unece:AssociationBIE",
                    "unece:cefactUNId": "UN01005030",
                    "unece:cefactBieDomainClass": "cefact:Extra_Price.Details",
                    "rdfs:comment": "A travel product period for which this extra price is valid."
                },
                {
                    "@id": "cefact:Discount_Price.Validity.TravelProduct_Period",
                    "@type": "unece:AssociationBIE",
                    "unece:cefactUNId": "UN01005049",
                    "unece:cefactBieDomainClass": "cefact:Discount_Price.Details",
                    "rdfs:comment": "A travel product period for which this discount price is valid."
                },
                {
                    "@id": "cefact:Extra_Price.Validity.Seasonal_Period",
                    "@type": "unece:AssociationBIE",
                    "unece:cefactUNId": "UN01005031",
                    "unece:cefactBieDomainClass": "cefact:Extra_Price.Details",
                    "rdfs:comment": "A seasonal period for which this extra price is valid."
                }
            ]
        }
    ]
}